@prefix owl:   <http://www.w3.org/2002/07/owl#> .
@prefix skos:  <http://www.w3.org/2004/02/skos/core#> .
@prefix rdfs:  <http://www.w3.org/2000/01/rdf-schema#> .
@prefix ns2:   <http://purl.org/dc/terms/> .
@prefix ns4:   <http://purl.org/dc/terms/> .
@prefix ns6:   <http://lemon-model.net/lemon#> .
@prefix ns5:   <http://publications.europa.eu/ontology/euvoc#> .
@prefix ns8:   <http://publications.europa.eu/ontology/authority/> .
@prefix ns7:   <http://www.w3.org/2008/05/skos-xl#> .
@prefix rdf:   <http://www.w3.org/1999/02/22-rdf-syntax-ns#> .
@prefix ns9:   <http://publications.europa.eu/ontology/authority/> .
@prefix ns10:  <http://publications.europa.eu/resource/authority/> .
@prefix dc:    <http://purl.org/dc/elements/1.1/> .

<http://publications.europa.eu/resource/authority/data-theme/ECON>
        a                   skos:Concept , ns5:DataTheme ;
        ns6:context         <http://publications.europa.eu/resource/authority/use-context/DCAT_AP> , <http://publications.europa.eu/resource/authority/use-context/ODP> , <http://publications.europa.eu/resource/authority/use-context/IMMC> ;
        ns9:authority-code  "ECON" ;
        ns9:deprecated      "false" ;
        ns9:op-code         "ECON" ;
        ns9:start.use       "2015-10-01" ;
        ns5:startDate       "2015-10-01"^^<http://www.w3.org/2001/XMLSchema#date> ;
        ns5:status          <http://publications.europa.eu/resource/authority/concept-status/CURRENT> ;
        ns5:xlDefinition    []  ;
        ns10:op-code        "ECON" ;
        dc:identifier       "ECON" ;
        ns4:created         "2015-10-01"^^<http://www.w3.org/2001/XMLSchema#date> ;
        ns4:dateAccepted    "2015-10-09"^^<http://www.w3.org/2001/XMLSchema#date> ;
        ns4:dateSubmitted   "2015-10-09"^^<http://www.w3.org/2001/XMLSchema#date> ;
        owl:versionInfo     "20200624-0" ;
        skos:definition     "This concept identifies datasets covering such domains as economy or finance. Economy is the area of the production, distribution and trade, as well as consumption of goods and services by different agents. In its broadest sense, the economy is defined as a social domain that emphasize the practices, discourses and material expressions associated with the production, use, and management of resources. Finance is the study of money and how it is used. Specifically, it deals with the questions of how an individual, company or government acquires the money needed and how they then spend or invest that money. Dataset examples: Tenders Electronic Daily (TED) - public procurement notices from the EU and beyond; General government deficit (-) and surplus (+) - quarterly data."@en ;
        skos:inScheme       ns10:data-theme ;
        skos:prefLabel      "Hospodářství a finance"@cs , "Gospodarstvo in finance"@sl , "Ekonomija i financije"@hr , "Økonomi og finanser"@da , "Ekonomi och finans"@sv , "Økonomi og finans"@no , "Geilleagar agus airgeadas"@ga , "Majandus ja rahandus"@et , "Οικονομία και χρηματοοικονομικά θέματα"@el , "Ekonomika ir finansai"@lt , "Économie et finances"@fr , "Talous ja raha-asiat"@fi , "Gospodarka i finanse"@pl , "Economia e finanças"@pt , "Economy and finance"@en , "Ekonomika un finanses"@lv , "Hospodárstvo a financie"@sk , "Economía y finanzas"@es , "Ekonomija u finanzi"@mt , "Economia e finanze"@it , "Gazdaság és pénzügy"@hu , "Economie en financiën"@nl , "Икономика и финанси"@bg , "Economie şi finanţe"@ro , "Wirtschaft und Finanzen"@de ;
        skos:topConceptOf   ns10:data-theme ;
        ns7:prefLabel       []  ;
        ns7:prefLabel       []  ;
        ns7:prefLabel       []  ;
        ns7:prefLabel       []  ;
        ns7:prefLabel       []  ;
        ns7:prefLabel       []  ;
        ns7:prefLabel       []  ;
        ns7:prefLabel       []  ;
        ns7:prefLabel       []  ;
        ns7:prefLabel       []  ;
        ns7:prefLabel       []  ;
        ns7:prefLabel       []  ;
        ns7:prefLabel       []  ;
        ns7:prefLabel       []  ;
        ns7:prefLabel       []  ;
        ns7:prefLabel       []  ;
        ns7:prefLabel       []  ;
        ns7:prefLabel       []  ;
        ns7:prefLabel       []  ;
        ns7:prefLabel       []  ;
        ns7:prefLabel       []  ;
        ns7:prefLabel       []  ;
        ns7:prefLabel       []  ;
        ns7:prefLabel       []  ;
        ns7:prefLabel       []  .

<http://publications.europa.eu/resource/authority/data-theme/GOVE>
        a                   ns5:DataTheme , skos:Concept ;
        ns6:context         <http://publications.europa.eu/resource/authority/use-context/IMMC> , <http://publications.europa.eu/resource/authority/use-context/ODP> , <http://publications.europa.eu/resource/authority/use-context/DCAT_AP> ;
        ns9:authority-code  "GOVE" ;
        ns9:deprecated      "false" ;
        ns9:op-code         "GOVE" ;
        ns9:start.use       "2015-10-01" ;
        ns5:startDate       "2015-10-01"^^<http://www.w3.org/2001/XMLSchema#date> ;
        ns5:status          <http://publications.europa.eu/resource/authority/concept-status/CURRENT> ;
        ns5:xlDefinition    []  ;
        ns10:op-code        "GOVE" ;
        dc:identifier       "GOVE" ;
        ns4:created         "2015-10-01"^^<http://www.w3.org/2001/XMLSchema#date> ;
        ns4:dateAccepted    "2015-10-09"^^<http://www.w3.org/2001/XMLSchema#date> ;
        ns4:dateSubmitted   "2015-10-09"^^<http://www.w3.org/2001/XMLSchema#date> ;
        owl:versionInfo     "20200624-0" ;
        skos:definition     "This concept identifies datasets covering such domains as government or public sector. A government is the system or group of people governing an organised community, often a state. The public sector is the part of the economy composed of both public services and public enterprises. Public sector services and enterprises can be controlled by central government, regional or local authorities. Organisations that are not part of the public sector are either a part of the private sector or voluntary sector. Dataset examples: Candidate countries and potential candidates: Government statistics; Transparency Register."@en ;
        skos:inScheme       ns10:data-theme ;
        skos:prefLabel      "Kormányzat és közszféra"@hu , "Governo e settore pubblico"@it , "Overheid en publieke sector"@nl , "Правителство и публичен сектор"@bg , "Rząd i sektor publiczny"@pl , "Government and public sector"@en , "Regeringen och den offentliga sektorn"@sv , "Valtioneuvosto ja julkinen sektori"@fi , "Vyriausybė ir viešasis sektorius"@lt , "Vlada i javni sektor"@hr , "Regierung und öffentlicher Sektor"@de , "Κυβέρνηση και δημόσιος τομέας"@el , "Vláda a veřejný sektor"@cs , "Valdība un sabiedriskais sektors"@lv , "Guvern şi sector public"@ro , "Vláda a verejný sektor"@sk , "Gobierno y sector público"@es , "Gouvernement et secteur public"@fr , "Regeringen og den offentlige sektor"@da , "Forvaltning og offentlig sektor"@no , "Gvern u settur pubbliku"@mt , "Rialtas agus earnáil phoiblí"@ga , "Vlada in javni sektor"@sl , "Valitsus ja avalik sektor"@et , "Governo e setor público"@pt ;
        skos:topConceptOf   ns10:data-theme ;
        ns7:prefLabel       []  ;
        ns7:prefLabel       []  ;
        ns7:prefLabel       []  ;
        ns7:prefLabel       []  ;
        ns7:prefLabel       []  ;
        ns7:prefLabel       []  ;
        ns7:prefLabel       []  ;
        ns7:prefLabel       []  ;
        ns7:prefLabel       []  ;
        ns7:prefLabel       []  ;
        ns7:prefLabel       []  ;
        ns7:prefLabel       []  ;
        ns7:prefLabel       []  ;
        ns7:prefLabel       []  ;
        ns7:prefLabel       []  ;
        ns7:prefLabel       []  ;
        ns7:prefLabel       []  ;
        ns7:prefLabel       []  ;
        ns7:prefLabel       []  ;
        ns7:prefLabel       []  ;
        ns7:prefLabel       []  ;
        ns7:prefLabel       []  ;
        ns7:prefLabel       []  ;
        ns7:prefLabel       []  ;
        ns7:prefLabel       []  .

<http://publications.europa.eu/resource/authority/data-theme/AGRI>
        a                   ns5:DataTheme , skos:Concept ;
        ns6:context         <http://publications.europa.eu/resource/authority/use-context/DCAT_AP> , <http://publications.europa.eu/resource/authority/use-context/ODP> , <http://publications.europa.eu/resource/authority/use-context/IMMC> ;
        ns9:authority-code  "AGRI" ;
        ns9:deprecated      "false" ;
        ns9:op-code         "AGRI" ;
        ns9:start.use       "2015-10-01" ;
        ns5:startDate       "2015-10-01"^^<http://www.w3.org/2001/XMLSchema#date> ;
        ns5:status          <http://publications.europa.eu/resource/authority/concept-status/CURRENT> ;
        ns5:xlDefinition    []  ;
        ns10:op-code        "AGRI" ;
        dc:identifier       "AGRI" ;
        ns4:created         "2015-10-01"^^<http://www.w3.org/2001/XMLSchema#date> ;
        ns4:dateAccepted    "2015-10-09"^^<http://www.w3.org/2001/XMLSchema#date> ;
        ns4:dateSubmitted   "2015-10-09"^^<http://www.w3.org/2001/XMLSchema#date> ;
        owl:versionInfo     "20200624-0" ;
        skos:definition     "This concept identifies datasets covering such domains as agriculture, fisheries, forestry or food. Agriculture is the science and art of cultivating plants and livestock. Fisheries are activities leading to harvesting of fish; may involve capture of wild fish or raising of fish through aquaculture. Forestry is the science and craft of creating, managing, using, conserving and repairing forests, woodlands and associated resources for human and environmental benefits. Food is any substance consumed to provide nutritional support for an organism. Dataset examples: Agricultural and Vegetable Catalogue; The Community Fishing Fleet Register; Pan-European Map of Forest Biomass Increment; Food composition database for nutrient intake: selected vitamins and minerals in selected European countries."@en ;
        skos:inScheme       ns10:data-theme ;
        skos:prefLabel      "Lauksaimniecība, zivsaimniecība, mežsaimniecība un pārtika"@lv , "Rolnictwo, rybołówstwo, leśnictwo i żywność"@pl , "Poľnohospodárstvo, rybné hospodárstvo, lesníctvo a potravinárstvo"@sk , "Agricultură, pescuit, silvicultură şi hrană"@ro , "Agricoltura, pesca, silvicoltura e prodotti alimentari"@it , "Jordbruk, fiskeri, skogbruk og mat"@no , "Селско стопанство, рибарство, горско стопанство и храни"@bg , "Poljoprivreda, ribarstvo, šumarstvo i hrana"@hr , "Mezőgazdaság, halászat, erdészet és élelmiszer"@hu , "Kmetijstvo, ribištvo, gozdarstvo in prehrana"@sl , "Zemědělství, rybolov, lesnictví a výživa"@cs , "Agriculture, fisheries, forestry and food"@en , "Talmhaíocht, iascach, foraoiseacht agus bia"@ga , "Agrikoltura, sajd, forestrija u ikel"@mt , "Agriculture, pêche, sylviculture et alimentation"@fr , "Landbouw, visserij, bosbouw en voeding"@nl , "Agricultura, pesca, silvicultura e alimentação"@pt , "Agricultura, pesca, silvicultura y alimentación"@es , "Γεωργία, αλιεία, δασοκομία και τρόφιμα"@el , "Põllumajandus, kalandus, metsandus ja toiduained"@et , "Jordbruk, fiske, skogsbruk och livsmedel"@sv , "Landbrug, fiskeri, skovbrug og fødevarer"@da , "Landwirtschaft, Fischerei, Forstwirtschaft und Nahrungsmittel"@de , "Žemės ūkis, žuvininkystė, miškininkystė ir maistas"@lt , "Maatalous, kalastus, metsätalous ja elintarvikkeet"@fi ;
        skos:topConceptOf   ns10:data-theme ;
        ns7:prefLabel       []  ;
        ns7:prefLabel       []  ;
        ns7:prefLabel       []  ;
        ns7:prefLabel       []  ;
        ns7:prefLabel       []  ;
        ns7:prefLabel       []  ;
        ns7:prefLabel       []  ;
        ns7:prefLabel       []  ;
        ns7:prefLabel       []  ;
        ns7:prefLabel       []  ;
        ns7:prefLabel       []  ;
        ns7:prefLabel       []  ;
        ns7:prefLabel       []  ;
        ns7:prefLabel       []  ;
        ns7:prefLabel       []  ;
        ns7:prefLabel       []  ;
        ns7:prefLabel       []  ;
        ns7:prefLabel       []  ;
        ns7:prefLabel       []  ;
        ns7:prefLabel       []  ;
        ns7:prefLabel       []  ;
        ns7:prefLabel       []  ;
        ns7:prefLabel       []  ;
        ns7:prefLabel       []  ;
        ns7:prefLabel       []  .

<http://publications.europa.eu/resource/authority/data-theme/ENVI>
        a                   ns5:DataTheme , skos:Concept ;
        ns6:context         <http://publications.europa.eu/resource/authority/use-context/IMMC> , <http://publications.europa.eu/resource/authority/use-context/ODP> , <http://publications.europa.eu/resource/authority/use-context/DCAT_AP> ;
        ns9:authority-code  "ENVI" ;
        ns9:deprecated      "false" ;
        ns9:op-code         "ENVI" ;
        ns9:start.use       "2015-10-01" ;
        ns5:startDate       "2015-10-01"^^<http://www.w3.org/2001/XMLSchema#date> ;
        ns5:status          <http://publications.europa.eu/resource/authority/concept-status/CURRENT> ;
        ns5:xlDefinition    []  ;
        ns10:op-code        "ENVI" ;
        dc:identifier       "ENVI" ;
        ns4:created         "2015-10-01"^^<http://www.w3.org/2001/XMLSchema#date> ;
        ns4:dateAccepted    "2015-10-09"^^<http://www.w3.org/2001/XMLSchema#date> ;
        ns4:dateSubmitted   "2015-10-09"^^<http://www.w3.org/2001/XMLSchema#date> ;
        owl:versionInfo     "20200624-0" ;
        skos:definition     "This concept identifies datasets covering the domain of environment. The natural environment encompasses the interaction of all living species, climate, weather and natural resources that affect human survival and economic activity. Dataset examples: Attitudes of European citizens towards the environment; Pollutant emissions from transport."@en ;
        skos:inScheme       ns10:data-theme ;
        skos:prefLabel      "Miljø"@no , "Miljø"@da , "Miljö"@sv , "Ambiente"@pt , "Ambiente"@it , "Okolje"@sl , "Περιβάλλον"@el , "Mediu"@ro , "Keskkond"@et , "Aplinka"@lt , "Životné prostredie"@sk , "Okoliš"@hr , "Околна среда"@bg , "Comhshaol"@ga , "Ympäristö"@fi , "Környezet"@hu , "Environnement"@fr , "Medio ambiente"@es , "Vide"@lv , "Ambjent"@mt , "Životní prostředí"@cs , "Umwelt"@de , "Środowisko"@pl , "Environment"@en , "Milieu"@nl ;
        skos:topConceptOf   ns10:data-theme ;
        ns7:prefLabel       []  ;
        ns7:prefLabel       []  ;
        ns7:prefLabel       []  ;
        ns7:prefLabel       []  ;
        ns7:prefLabel       []  ;
        ns7:prefLabel       []  ;
        ns7:prefLabel       []  ;
        ns7:prefLabel       []  ;
        ns7:prefLabel       []  ;
        ns7:prefLabel       []  ;
        ns7:prefLabel       []  ;
        ns7:prefLabel       []  ;
        ns7:prefLabel       []  ;
        ns7:prefLabel       []  ;
        ns7:prefLabel       []  ;
        ns7:prefLabel       []  ;
        ns7:prefLabel       []  ;
        ns7:prefLabel       []  ;
        ns7:prefLabel       []  ;
        ns7:prefLabel       []  ;
        ns7:prefLabel       []  ;
        ns7:prefLabel       []  ;
        ns7:prefLabel       []  ;
        ns7:prefLabel       []  ;
        ns7:prefLabel       []  .

<http://publications.europa.eu/resource/authority/data-theme/ENER>
        a                   skos:Concept , ns5:DataTheme ;
        ns6:context         <http://publications.europa.eu/resource/authority/use-context/IMMC> , <http://publications.europa.eu/resource/authority/use-context/ODP> , <http://publications.europa.eu/resource/authority/use-context/DCAT_AP> ;
        ns9:authority-code  "ENER" ;
        ns9:deprecated      "false" ;
        ns9:op-code         "ENER" ;
        ns9:start.use       "2015-10-01" ;
        ns5:startDate       "2015-10-01"^^<http://www.w3.org/2001/XMLSchema#date> ;
        ns5:status          <http://publications.europa.eu/resource/authority/concept-status/CURRENT> ;
        ns5:xlDefinition    []  ;
        ns10:op-code        "ENER" ;
        dc:identifier       "ENER" ;
        ns4:created         "2015-10-01"^^<http://www.w3.org/2001/XMLSchema#date> ;
        ns4:dateAccepted    "2015-10-09"^^<http://www.w3.org/2001/XMLSchema#date> ;
        ns4:dateSubmitted   "2015-10-09"^^<http://www.w3.org/2001/XMLSchema#date> ;
        owl:versionInfo     "20200624-0" ;
        skos:definition     "This concept identifies datasets covering the domain of energy. Energy is the quantitative property that must be transferred to an object in order to perform work on, or to heat, the object. Living organisms require energy to stay alive; human civilisation requires energy to function. Dataset examples: European gas market reports; Electricity prices by type of user."@en ;
        skos:inScheme       ns10:data-theme ;
        skos:prefLabel      "Fuinneamh"@ga , "Énergie"@fr , "Energy"@en , "Energía"@es , "Ενέργεια"@el , "Energie"@cs , "Energie"@de , "Energie"@ro , "Energie"@nl , "Energetika"@sk , "Energetika"@hr , "Energetika"@lt , "Energetika"@sl , "Enerġija"@mt , "Energeetika"@et , "Energia"@it , "Energia"@pl , "Energia"@pt , "Energia"@hu , "Energia"@fi , "Energi"@sv , "Energi"@da , "Energi"@no , "Enerģētika"@lv , "Енергетика"@bg ;
        skos:topConceptOf   ns10:data-theme ;
        ns7:prefLabel       []  ;
        ns7:prefLabel       []  ;
        ns7:prefLabel       []  ;
        ns7:prefLabel       []  ;
        ns7:prefLabel       []  ;
        ns7:prefLabel       []  ;
        ns7:prefLabel       []  ;
        ns7:prefLabel       []  ;
        ns7:prefLabel       []  ;
        ns7:prefLabel       []  ;
        ns7:prefLabel       []  ;
        ns7:prefLabel       []  ;
        ns7:prefLabel       []  ;
        ns7:prefLabel       []  ;
        ns7:prefLabel       []  ;
        ns7:prefLabel       []  ;
        ns7:prefLabel       []  ;
        ns7:prefLabel       []  ;
        ns7:prefLabel       []  ;
        ns7:prefLabel       []  ;
        ns7:prefLabel       []  ;
        ns7:prefLabel       []  ;
        ns7:prefLabel       []  ;
        ns7:prefLabel       []  ;
        ns7:prefLabel       []  .

<http://publications.europa.eu/resource/authority/data-theme/EDUC>
        a                   skos:Concept , ns5:DataTheme ;
        ns6:context         <http://publications.europa.eu/resource/authority/use-context/IMMC> , <http://publications.europa.eu/resource/authority/use-context/ODP> , <http://publications.europa.eu/resource/authority/use-context/DCAT_AP> ;
        ns9:authority-code  "EDUC" ;
        ns9:deprecated      "false" ;
        ns9:op-code         "EDUC" ;
        ns9:start.use       "2015-10-01" ;
        ns5:startDate       "2015-10-01"^^<http://www.w3.org/2001/XMLSchema#date> ;
        ns5:status          <http://publications.europa.eu/resource/authority/concept-status/CURRENT> ;
        ns5:xlDefinition    []  ;
        ns10:op-code        "EDUC" ;
        dc:identifier       "EDUC" ;
        ns4:created         "2015-10-01"^^<http://www.w3.org/2001/XMLSchema#date> ;
        ns4:dateAccepted    "2015-10-09"^^<http://www.w3.org/2001/XMLSchema#date> ;
        ns4:dateSubmitted   "2015-10-09"^^<http://www.w3.org/2001/XMLSchema#date> ;
        owl:versionInfo     "20200624-0" ;
        skos:definition     "This concept identifies datasets covering such domains as education, culture or sport. Education is the process of facilitating learning, or the acquisition of knowledge, skills, values, beliefs and habits. Culture encompasses the social behavior and norms found in human societies, as well as the knowledge, beliefs, arts, laws, customs, capabilities and habits of the individuals in these groups. Sport includes all forms of competitive physical activity or games which maintain or improve physical ability and skills while providing enjoyment to participants, and in some cases, entertainment for spectators. Dataset examples: European Skills, Competences, Qualifications and Occupations (ESCO); EU Member States and international human rights obligations; Participation in any cultural or sport activities in the last 12 months by sex, age and educational attainment level."@en ;
        skos:inScheme       ns10:data-theme ;
        skos:prefLabel      "Oktatás, kultúra és sport"@hu , "Vzdelávanie, kultúra a šport"@sk , "Bildung, Kultur und Sport"@de , "Koulutus, kulttuuri ja urheilu"@fi , "Vzdělávání, kultura a sport"@cs , "Uddannelse, kultur og sport"@da , "Παιδεία, πολιτιστικά θέματα και αθλητισμός"@el , "Švietimas, kultūra ir sportas"@lt , "Haridus, kultuur ja sport"@et , "Education, culture and sport"@en , "Onderwijs, cultuur en sport"@nl , "Educaţie, cultură şi sport"@ro , "Izglītība, kultūra un sports"@lv , "Izobraževanje, kultura in šport"@sl , "Utbildning, kultur och sport"@sv , "Éducation, culture et sport"@fr , "Istruzione, cultura e sport"@it , "Educación, cultura y deportes"@es , "Образование, култура и спорт"@bg , "Educação, cultura e desporto"@pt , "Utdanning, kultur og sport"@no , "Edukazzjoni, kultura u sport"@mt , "Edukacja, kultura i sport"@pl , "Oideachas, cultúr agus spórt"@ga , "Obrazovanje, kultura i sport"@hr ;
        skos:topConceptOf   ns10:data-theme ;
        ns7:prefLabel       []  ;
        ns7:prefLabel       []  ;
        ns7:prefLabel       []  ;
        ns7:prefLabel       []  ;
        ns7:prefLabel       []  ;
        ns7:prefLabel       []  ;
        ns7:prefLabel       []  ;
        ns7:prefLabel       []  ;
        ns7:prefLabel       []  ;
        ns7:prefLabel       []  ;
        ns7:prefLabel       []  ;
        ns7:prefLabel       []  ;
        ns7:prefLabel       []  ;
        ns7:prefLabel       []  ;
        ns7:prefLabel       []  ;
        ns7:prefLabel       []  ;
        ns7:prefLabel       []  ;
        ns7:prefLabel       []  ;
        ns7:prefLabel       []  ;
        ns7:prefLabel       []  ;
        ns7:prefLabel       []  ;
        ns7:prefLabel       []  ;
        ns7:prefLabel       []  ;
        ns7:prefLabel       []  ;
        ns7:prefLabel       []  .

<http://publications.europa.eu/resource/authority/data-theme/JUST>
        a                   ns5:DataTheme , skos:Concept ;
        ns6:context         <http://publications.europa.eu/resource/authority/use-context/DCAT_AP> , <http://publications.europa.eu/resource/authority/use-context/ODP> , <http://publications.europa.eu/resource/authority/use-context/IMMC> ;
        ns9:authority-code  "JUST" ;
        ns9:deprecated      "false" ;
        ns9:op-code         "JUST" ;
        ns9:start.use       "2015-10-01" ;
        ns5:startDate       "2015-10-01"^^<http://www.w3.org/2001/XMLSchema#date> ;
        ns5:status          <http://publications.europa.eu/resource/authority/concept-status/CURRENT> ;
        ns5:xlDefinition    []  ;
        ns10:op-code        "JUST" ;
        dc:identifier       "JUST" ;
        ns4:created         "2015-10-01"^^<http://www.w3.org/2001/XMLSchema#date> ;
        ns4:dateAccepted    "2015-10-09"^^<http://www.w3.org/2001/XMLSchema#date> ;
        ns4:dateSubmitted   "2015-10-09"^^<http://www.w3.org/2001/XMLSchema#date> ;
        owl:versionInfo     "20200624-0" ;
        skos:definition     "This concept identifies datasets covering such domains as justice, legal system or public safety. Justice includes both the attainment of that which is just and the philosophical discussion of that which is just; here it mainly means the procedural justice as found in the study and application of the law. The contemporary legal systems of the world are generally based on one of four basic systems: civil law, common law, statutory law, religious law or combinations of these. Public safety is the function of governments which ensures the protection of citizens, persons in their territory, organisations and institutions against threats to their well-being – and to the prosperity of their communities. Dataset examples: EU case-law; Information on Member States Law; European Data Protection Supervisor register of processing operations."@en ;
        skos:inScheme       ns10:data-theme ;
        skos:prefLabel      "Spravedlnost, právní systém a veřejná bezpečnost"@cs , "Spravodlivosť, právny systém a verejná bezpečnosť"@sk , "Igazságügy, jogrendszer és közbiztonság"@hu , "Justice, système juridique et sécurité publique"@fr , "Sprawiedliwość, ustrój sądów i bezpieczeństwo publiczne"@pl , "Ceartas, córas dlí agus sábháilteacht an phobail"@ga , "Õigusemõistmine, õigussüsteem ja avalik turvalisus"@et , "Ġustizzja, sistema legali u sigurtà pubblika"@mt , "Rättvisa, rättsliga system och allmän säkerhet"@sv , "Retfærdighed, retssystem og offentlig sikkerhed"@da , "Justicia, sistema judicial y seguridad pública"@es , "Justiție, sistem juridic și siguranță publică"@ro , "Justis, rettssystem og allmenn sikkerhet"@no , "Pravosuđe, pravni sustav i javna sigurnost"@hr , "Правосъдие, съдебна система и обществена безопасност"@bg , "Justitie, rechtsstelsel en openbare veiligheid"@nl , "Pravosodje, pravni sistem in javna varnost"@sl , "Teisingumas, teisės sistema ir visuomenės sauga"@lt , "Oikeus, oikeusjärjestelmä ja yleinen turvallisuus"@fi , "Tieslietas, tiesību sistēma un sabiedrības drošība"@lv , "Giustizia, sistema giuridico e sicurezza pubblica"@it , "Justiz, Rechtssystem und öffentliche Sicherheit"@de , "Justiça, sistema judiciário e segurança pública"@pt , "Justice, legal system and public safety"@en , "Δικαιoσύνη, νομικό σύστημα και δημόσια ασφάλεια"@el ;
        skos:topConceptOf   ns10:data-theme ;
        ns7:prefLabel       []  ;
        ns7:prefLabel       []  ;
        ns7:prefLabel       []  ;
        ns7:prefLabel       []  ;
        ns7:prefLabel       []  ;
        ns7:prefLabel       []  ;
        ns7:prefLabel       []  ;
        ns7:prefLabel       []  ;
        ns7:prefLabel       []  ;
        ns7:prefLabel       []  ;
        ns7:prefLabel       []  ;
        ns7:prefLabel       []  ;
        ns7:prefLabel       []  ;
        ns7:prefLabel       []  ;
        ns7:prefLabel       []  ;
        ns7:prefLabel       []  ;
        ns7:prefLabel       []  ;
        ns7:prefLabel       []  ;
        ns7:prefLabel       []  ;
        ns7:prefLabel       []  ;
        ns7:prefLabel       []  ;
        ns7:prefLabel       []  ;
        ns7:prefLabel       []  ;
        ns7:prefLabel       []  ;
        ns7:prefLabel       []  .

<http://publications.europa.eu/resource/authority/data-theme/REGI>
        a                   skos:Concept , ns5:DataTheme ;
        ns6:context         <http://publications.europa.eu/resource/authority/use-context/IMMC> , <http://publications.europa.eu/resource/authority/use-context/DCAT_AP> , <http://publications.europa.eu/resource/authority/use-context/ODP> ;
        ns9:authority-code  "REGI" ;
        ns9:deprecated      "false" ;
        ns9:op-code         "REGI" ;
        ns9:start.use       "2015-10-01" ;
        ns5:startDate       "2015-10-01"^^<http://www.w3.org/2001/XMLSchema#date> ;
        ns5:status          <http://publications.europa.eu/resource/authority/concept-status/CURRENT> ;
        ns5:xlDefinition    []  ;
        ns10:op-code        "REGI" ;
        dc:identifier       "REGI" ;
        ns4:created         "2015-10-01"^^<http://www.w3.org/2001/XMLSchema#date> ;
        ns4:dateAccepted    "2015-10-09"^^<http://www.w3.org/2001/XMLSchema#date> ;
        ns4:dateSubmitted   "2015-10-09"^^<http://www.w3.org/2001/XMLSchema#date> ;
        owl:versionInfo     "20200624-0" ;
        skos:definition     "This concept identifies datasets covering such domains as regions or cities. In the field of political geography, regions tend to be based on political units such as sovereign states; subnational units such as administrative regions, provinces, states, counties, townships, territories, etc.; and multinational groupings. A city is a large human settlement. Dataset examples: NUTS - Nomenclature of territorial units for statistics classification; UDP - GDP per capita by metro regions, 2000 - 2060."@en ;
        skos:inScheme       ns10:data-theme ;
        skos:prefLabel      "Περιφέρειες και πόλεις"@el , "Regions and cities"@en , "Regiões e cidades"@pt , "Regiuni şi orașe"@ro , "Réigiúin agus cathracha"@ga , "Piirkonnad ja linnad"@et , "Régiók és városok"@hu , "Alueet ja kaupungit"@fi , "Regionen und Städte"@de , "Regioni e città"@it , "Regioner og byer"@no , "Regioner og byer"@da , "Reġjuni u bliet"@mt , "Regiones y ciudades"@es , "Regije i gradovi"@hr , "Régions et villes"@fr , "Regiony i miasta"@pl , "Regióny a mestá"@sk , "Regioner och städer"@sv , "Regiony a města"@cs , "Regionai ir miestai"@lt , "Regije in mesta"@sl , "Regio's en steden"@nl , "Reģioni un pilsētas"@lv , "Региони и градове"@bg ;
        skos:topConceptOf   ns10:data-theme ;
        ns7:prefLabel       []  ;
        ns7:prefLabel       []  ;
        ns7:prefLabel       []  ;
        ns7:prefLabel       []  ;
        ns7:prefLabel       []  ;
        ns7:prefLabel       []  ;
        ns7:prefLabel       []  ;
        ns7:prefLabel       []  ;
        ns7:prefLabel       []  ;
        ns7:prefLabel       []  ;
        ns7:prefLabel       []  ;
        ns7:prefLabel       []  ;
        ns7:prefLabel       []  ;
        ns7:prefLabel       []  ;
        ns7:prefLabel       []  ;
        ns7:prefLabel       []  ;
        ns7:prefLabel       []  ;
        ns7:prefLabel       []  ;
        ns7:prefLabel       []  ;
        ns7:prefLabel       []  ;
        ns7:prefLabel       []  ;
        ns7:prefLabel       []  ;
        ns7:prefLabel       []  ;
        ns7:prefLabel       []  ;
        ns7:prefLabel       []  .

ns10:data-theme  a                skos:ConceptScheme , owl:Ontology ;
        rdfs:comment              "Data theme"^^rdfs:Literal ;
        rdfs:label                "Data theme"@en ;
        ns9:prefLabel             "Data theme"@en ;
        ns9:table.id              "data-theme" ;
        ns9:table.version.number  "20200624-0" ;
        ns4:identifier            "http://publications.europa.eu/resource/authority/data-theme" ;
        owl:imports               <http://publications.europa.eu/ontology/euvoc> ;
        owl:versionIRI            <http://publications.europa.eu/resource/authority/data-theme/20200624-0> ;
        owl:versionInfo           "20200624-0" ;
        skos:prefLabel            "Data theme"@en ;
        ns7:prefLabel             []  ;
        ns7:prefLabel             []  .

<http://publications.europa.eu/resource/authority/data-theme/INTR>
        a                   ns5:DataTheme , skos:Concept ;
        ns6:context         <http://publications.europa.eu/resource/authority/use-context/DCAT_AP> , <http://publications.europa.eu/resource/authority/use-context/ODP> , <http://publications.europa.eu/resource/authority/use-context/IMMC> ;
        ns9:authority-code  "INTR" ;
        ns9:deprecated      "false" ;
        ns9:op-code         "INTR" ;
        ns9:start.use       "2015-10-01" ;
        ns5:startDate       "2015-10-01"^^<http://www.w3.org/2001/XMLSchema#date> ;
        ns5:status          <http://publications.europa.eu/resource/authority/concept-status/CURRENT> ;
        ns5:xlDefinition    []  ;
        ns10:op-code        "INTR" ;
        dc:identifier       "INTR" ;
        ns4:created         "2015-10-01"^^<http://www.w3.org/2001/XMLSchema#date> ;
        ns4:dateAccepted    "2015-10-09"^^<http://www.w3.org/2001/XMLSchema#date> ;
        ns4:dateSubmitted   "2015-10-09"^^<http://www.w3.org/2001/XMLSchema#date> ;
        owl:versionInfo     "20200624-0" ;
        skos:definition     "This concept identifies datasets covering the domain of international issues. An issue – important topic or problem for debate or discussion – is international when the participants represent at least two countries. Dataset examples: Consolidated list of persons, groups and entities subject to EU financial sanctions; European Commission — DG DEVCO – development and humanitarian assistance to Afghanistan."@en ;
        skos:inScheme       ns10:data-theme ;
        skos:prefLabel      "Medzinárodné otázky"@sk , "Questions internationales"@fr , "Međunarodni pitanja"@hr , "Mezinárodní otázky"@cs , "Kwestie międzynarodowe"@pl , "Tarptautiniai klausimai"@lt , "Διεθνή θέματα"@el , "International issues"@en , "Tematiche internazionali"@it , "Международни въпроси"@bg , "Questões internacionais"@pt , "Asuntos internacionales"@es , "Saincheisteanna idirnáisiúnta"@ga , "Internationale Themen"@de , "Chestiuni internaționale"@ro , "Internationale vraagstukken"@nl , "Kwistjonijiet internazzjonali"@mt , "Mednarodna vprašanja"@sl , "Internationella frågor"@sv , "Starptautiski jautājumi"@lv , "Internasjonale temaer"@no , "Rahvusvahelised küsimused"@et , "Internationale spørgsmål"@da , "Nemzetközi ügyek"@hu , "Kansainväliset kysymykset"@fi ;
        skos:topConceptOf   ns10:data-theme ;
        ns7:prefLabel       []  ;
        ns7:prefLabel       []  ;
        ns7:prefLabel       []  ;
        ns7:prefLabel       []  ;
        ns7:prefLabel       []  ;
        ns7:prefLabel       []  ;
        ns7:prefLabel       []  ;
        ns7:prefLabel       []  ;
        ns7:prefLabel       []  ;
        ns7:prefLabel       []  ;
        ns7:prefLabel       []  ;
        ns7:prefLabel       []  ;
        ns7:prefLabel       []  ;
        ns7:prefLabel       []  ;
        ns7:prefLabel       []  ;
        ns7:prefLabel       []  ;
        ns7:prefLabel       []  ;
        ns7:prefLabel       []  ;
        ns7:prefLabel       []  ;
        ns7:prefLabel       []  ;
        ns7:prefLabel       []  ;
        ns7:prefLabel       []  ;
        ns7:prefLabel       []  ;
        ns7:prefLabel       []  ;
        ns7:prefLabel       []  .

<http://publications.europa.eu/resource/authority/data-theme/HEAL>
        a                   ns5:DataTheme , skos:Concept ;
        ns6:context         <http://publications.europa.eu/resource/authority/use-context/ODP> , <http://publications.europa.eu/resource/authority/use-context/DCAT_AP> , <http://publications.europa.eu/resource/authority/use-context/IMMC> ;
        ns9:authority-code  "HEAL" ;
        ns9:deprecated      "false" ;
        ns9:op-code         "HEAL" ;
        ns9:start.use       "2015-10-01" ;
        ns5:startDate       "2015-10-01"^^<http://www.w3.org/2001/XMLSchema#date> ;
        ns5:status          <http://publications.europa.eu/resource/authority/concept-status/CURRENT> ;
        ns5:xlDefinition    []  ;
        ns10:op-code        "HEAL" ;
        dc:identifier       "HEAL" ;
        ns4:created         "2015-10-01"^^<http://www.w3.org/2001/XMLSchema#date> ;
        ns4:dateAccepted    "2015-10-09"^^<http://www.w3.org/2001/XMLSchema#date> ;
        ns4:dateSubmitted   "2015-10-09"^^<http://www.w3.org/2001/XMLSchema#date> ;
        owl:versionInfo     "20200624-0" ;
        skos:definition     "This concept identifies datasets covering the domain of health. Health is a state of physical, mental and social well-being in which disease and infirmity are absent. Dataset examples: COVID-19 Coronavirus data; European Cancer Information System."@en ;
        skos:inScheme       ns10:data-theme ;
        skos:prefLabel      "Υγεία"@el , "Zdrowie"@pl , "Sveikata"@lt , "Salud"@es , "Saúde"@pt , "Zdraví"@cs , "Gezondheid"@nl , "Sláinte"@ga , "Gesundheit"@de , "Hälsa"@sv , "Sundhed"@da , "Zdravje"@sl , "Zdravotníctvo"@sk , "Salute"@it , "Helse"@no , "Zdravlje"@hr , "Здраве"@bg , "Saħħa"@mt , "Santé"@fr , "Sănătate"@ro , "Terveys"@fi , "Veselība"@lv , "Egészségügy"@hu , "Tervis"@et , "Health"@en ;
        skos:topConceptOf   ns10:data-theme ;
        ns7:prefLabel       []  ;
        ns7:prefLabel       []  ;
        ns7:prefLabel       []  ;
        ns7:prefLabel       []  ;
        ns7:prefLabel       []  ;
        ns7:prefLabel       []  ;
        ns7:prefLabel       []  ;
        ns7:prefLabel       []  ;
        ns7:prefLabel       []  ;
        ns7:prefLabel       []  ;
        ns7:prefLabel       []  ;
        ns7:prefLabel       []  ;
        ns7:prefLabel       []  ;
        ns7:prefLabel       []  ;
        ns7:prefLabel       []  ;
        ns7:prefLabel       []  ;
        ns7:prefLabel       []  ;
        ns7:prefLabel       []  ;
        ns7:prefLabel       []  ;
        ns7:prefLabel       []  ;
        ns7:prefLabel       []  ;
        ns7:prefLabel       []  ;
        ns7:prefLabel       []  ;
        ns7:prefLabel       []  ;
        ns7:prefLabel       []  .

<http://publications.europa.eu/resource/authority/data-theme/SOCI>
        a                   skos:Concept , ns5:DataTheme ;
        ns6:context         <http://publications.europa.eu/resource/authority/use-context/IMMC> , <http://publications.europa.eu/resource/authority/use-context/DCAT_AP> , <http://publications.europa.eu/resource/authority/use-context/ODP> ;
        ns9:authority-code  "SOCI" ;
        ns9:deprecated      "false" ;
        ns9:op-code         "SOCI" ;
        ns9:start.use       "2015-10-01" ;
        ns5:startDate       "2015-10-01"^^<http://www.w3.org/2001/XMLSchema#date> ;
        ns5:status          <http://publications.europa.eu/resource/authority/concept-status/CURRENT> ;
        ns5:xlDefinition    []  ;
        ns10:op-code        "SOCI" ;
        dc:identifier       "SOCI" ;
        ns4:created         "2015-10-01"^^<http://www.w3.org/2001/XMLSchema#date> ;
        ns4:dateAccepted    "2015-10-09"^^<http://www.w3.org/2001/XMLSchema#date> ;
        ns4:dateSubmitted   "2015-10-09"^^<http://www.w3.org/2001/XMLSchema#date> ;
        owl:versionInfo     "20200624-0" ;
        skos:definition     "This concept identifies datasets covering such domains as population or society. Population is a collection of humans and their entire race; it is the number of people in a city or town, region, country or world. A society is a group of individuals involved in persistent social interaction, or a large social group sharing the same spatial or social territory, typically subject to the same political authority and dominant cultural expectations. Dataset examples: Population density by NUTS 2 region; Violence against Women: An EU-wide survey."@en ;
        skos:inScheme       ns10:data-theme ;
        skos:prefLabel      "Befolkning og samfund"@da , "Iedzīvotāji un sabiedrība"@lv , "Population et société"@fr , "Populace a společnost"@cs , "Bevölkerung und Gesellschaft"@de , "Daonra agus sochaí"@ga , "População e sociedade"@pt , "Népesség és társadalom"@hu , "Elanikkond ja ühiskond"@et , "Prebivalstvo in družba"@sl , "Population and society"@en , "Popolazione e società"@it , "Население и общество"@bg , "Πληθυσμός και κοινωνία"@el , "Gyventojų skaičius ir visuomenė"@lt , "Población y sociedad"@es , "Befolkning och samhälle"@sv , "Bevolking en samenleving"@nl , "Befolkning og samfunn"@no , "Stanovništvo i društvo"@hr , "Väestö ja yhteiskunta"@fi , "Obyvateľstvo a spoločnosť"@sk , "Populaţie şi societate"@ro , "Popolazzjoni u soċjetà"@mt , "Ludność i społeczeństwo"@pl ;
        skos:topConceptOf   ns10:data-theme ;
        ns7:prefLabel       []  ;
        ns7:prefLabel       []  ;
        ns7:prefLabel       []  ;
        ns7:prefLabel       []  ;
        ns7:prefLabel       []  ;
        ns7:prefLabel       []  ;
        ns7:prefLabel       []  ;
        ns7:prefLabel       []  ;
        ns7:prefLabel       []  ;
        ns7:prefLabel       []  ;
        ns7:prefLabel       []  ;
        ns7:prefLabel       []  ;
        ns7:prefLabel       []  ;
        ns7:prefLabel       []  ;
        ns7:prefLabel       []  ;
        ns7:prefLabel       []  ;
        ns7:prefLabel       []  ;
        ns7:prefLabel       []  ;
        ns7:prefLabel       []  ;
        ns7:prefLabel       []  ;
        ns7:prefLabel       []  ;
        ns7:prefLabel       []  ;
        ns7:prefLabel       []  ;
        ns7:prefLabel       []  ;
        ns7:prefLabel       []  .

<http://publications.europa.eu/resource/authority/data-theme/OP_DATPRO>
        a                  skos:Concept , ns5:DataTheme ;
        ns9:op-code        "OP_DATPRO" ;
        ns5:status         <http://publications.europa.eu/resource/authority/concept-status/CURRENT> ;
        ns10:op-code       "OP_DATPRO" ;
        dc:identifier      "OP_DATPRO" ;
        ns4:created        "2015-10-01"^^<http://www.w3.org/2001/XMLSchema#date> ;
        owl:versionInfo    "20200624-0" ;
        skos:inScheme      ns10:data-theme ;
        skos:prefLabel     "Midlertidige data"@da , "Données provisoires"@fr , "Provisional data"@en , "Predbežné údaje"@sk , "НЕОКОНЧАТЕЛНИ ДАННИ"@bg , "Datos provisionales"@es , "Esialgsed andmed"@et , "Dados provisórios"@pt , "Privremeni podaci"@hr , "Začasni podatki"@sl , "Sonraí sealadacha"@ga , "Dane tymczasowe"@pl , "Dejta provviżorja"@mt , "Tillfälliga uppgifter"@sv , "Date provizorii"@ro , "Provizoriski dati"@lv , "Ideiglenes adatok"@hu , "Předběžné údaje"@cs , "Dati provvisori"@it , "Vorläufige Daten"@de , "Voorlopige gegevens"@nl , "Alustavat tiedot"@fi , "Προσωρινά δεδομένα"@el , "Laikinieji duomenys"@lt ;
        skos:topConceptOf  ns10:data-theme ;
        ns7:prefLabel      []  ;
        ns7:prefLabel      []  ;
        ns7:prefLabel      []  ;
        ns7:prefLabel      []  ;
        ns7:prefLabel      []  ;
        ns7:prefLabel      []  ;
        ns7:prefLabel      []  ;
        ns7:prefLabel      []  ;
        ns7:prefLabel      []  ;
        ns7:prefLabel      []  ;
        ns7:prefLabel      []  ;
        ns7:prefLabel      []  ;
        ns7:prefLabel      []  ;
        ns7:prefLabel      []  ;
        ns7:prefLabel      []  ;
        ns7:prefLabel      []  ;
        ns7:prefLabel      []  ;
        ns7:prefLabel      []  ;
        ns7:prefLabel      []  ;
        ns7:prefLabel      []  ;
        ns7:prefLabel      []  ;
        ns7:prefLabel      []  ;
        ns7:prefLabel      []  ;
        ns7:prefLabel      []  .

<http://publications.europa.eu/resource/authority/data-theme/TECH>
        a                   skos:Concept , ns5:DataTheme ;
        ns6:context         <http://publications.europa.eu/resource/authority/use-context/IMMC> , <http://publications.europa.eu/resource/authority/use-context/DCAT_AP> , <http://publications.europa.eu/resource/authority/use-context/ODP> ;
        ns9:authority-code  "TECH" ;
        ns9:deprecated      "false" ;
        ns9:op-code         "TECH" ;
        ns9:start.use       "2015-10-01" ;
        ns5:startDate       "2015-10-01"^^<http://www.w3.org/2001/XMLSchema#date> ;
        ns5:status          <http://publications.europa.eu/resource/authority/concept-status/CURRENT> ;
        ns5:xlDefinition    []  ;
        ns10:op-code        "TECH" ;
        dc:identifier       "TECH" ;
        ns4:created         "2015-10-01"^^<http://www.w3.org/2001/XMLSchema#date> ;
        ns4:dateAccepted    "2015-10-09"^^<http://www.w3.org/2001/XMLSchema#date> ;
        ns4:dateSubmitted   "2015-10-09"^^<http://www.w3.org/2001/XMLSchema#date> ;
        owl:versionInfo     "20200624-0" ;
        skos:definition     "This concept identifies datasets covering such domains as science or technology. Science is a systematic enterprise that builds and organises knowledge in the form of testable explanations and predictions. Modern science is typically divided into three major branches that consist of the natural sciences, which study nature in the broadest sense; the social sciences, which study individuals and societies; and the formal sciences, which study abstract concepts. Technology is the sum of techniques, skills, methods and processes used in the production of goods or services or in the accomplishment of objectives, such as scientific investigation. Dataset examples: CORDIS - EU research projects under Horizon 2020 (2014-2020); Take-up of mobile broadband (subscriptions/100 people)."@en ;
        skos:inScheme       ns10:data-theme ;
        skos:prefLabel      "Xjenza u teknoloġija"@mt , "Mokslas ir technologijos"@lt , "Ştiinţă şi tehnologie"@ro , "Tiede ja teknologia"@fi , "Scienza e tecnologia"@it , "Teadus ja tehnoloogia"@et , "Science et technologie"@fr , "Vitenskap og teknologi"@no , "Vetenskap och teknik"@sv , "Wetenschap en technologie"@nl , "Eolaíocht agus teicneolaíocht"@ga , "Znanost in tehnologija"@sl , "Veda a technika"@sk , "Ciencia y tecnología"@es , "Επιστήμη και τεχνολογία"@el , "Nauka i technologia"@pl , "Zinātne un tehnoloģija"@lv , "Ciência e tecnologia"@pt , "Wissenschaft und Technologie"@de , "Наука и tехнологии"@bg , "Science and technology"@en , "Videnskab og teknologi"@da , "Tudomány és technológia"@hu , "Znanost i tehnologija"@hr , "Věda a technika"@cs ;
        skos:topConceptOf   ns10:data-theme ;
        ns7:prefLabel       []  ;
        ns7:prefLabel       []  ;
        ns7:prefLabel       []  ;
        ns7:prefLabel       []  ;
        ns7:prefLabel       []  ;
        ns7:prefLabel       []  ;
        ns7:prefLabel       []  ;
        ns7:prefLabel       []  ;
        ns7:prefLabel       []  ;
        ns7:prefLabel       []  ;
        ns7:prefLabel       []  ;
        ns7:prefLabel       []  ;
        ns7:prefLabel       []  ;
        ns7:prefLabel       []  ;
        ns7:prefLabel       []  ;
        ns7:prefLabel       []  ;
        ns7:prefLabel       []  ;
        ns7:prefLabel       []  ;
        ns7:prefLabel       []  ;
        ns7:prefLabel       []  ;
        ns7:prefLabel       []  ;
        ns7:prefLabel       []  ;
        ns7:prefLabel       []  ;
        ns7:prefLabel       []  ;
        ns7:prefLabel       []  .

<http://publications.europa.eu/resource/authority/data-theme/TRAN>
        a                   ns5:DataTheme , skos:Concept ;
        ns6:context         <http://publications.europa.eu/resource/authority/use-context/IMMC> , <http://publications.europa.eu/resource/authority/use-context/ODP> , <http://publications.europa.eu/resource/authority/use-context/DCAT_AP> ;
        ns9:authority-code  "TRAN" ;
        ns9:deprecated      "false" ;
        ns9:op-code         "TRAN" ;
        ns9:start.use       "2015-10-01" ;
        ns5:startDate       "2015-10-01"^^<http://www.w3.org/2001/XMLSchema#date> ;
        ns5:status          <http://publications.europa.eu/resource/authority/concept-status/CURRENT> ;
        ns5:xlDefinition    []  ;
        ns10:op-code        "TRAN" ;
        dc:identifier       "TRAN" ;
        ns4:created         "2015-10-01"^^<http://www.w3.org/2001/XMLSchema#date> ;
        ns4:dateAccepted    "2015-10-09"^^<http://www.w3.org/2001/XMLSchema#date> ;
        ns4:dateSubmitted   "2015-10-09"^^<http://www.w3.org/2001/XMLSchema#date> ;
        owl:versionInfo     "20200624-0" ;
        skos:definition     "This concept identifies datasets covering the domain of transport. Transport is the movement of humans, animals and goods from one location to another. Modes of transport include air, land (rail and road), water, cable, pipeline and space. Dataset examples: Total length of motorways; Airport traffic data by reporting airport and airlines."@en ;
        skos:inScheme       ns10:data-theme ;
        skos:prefLabel      "Transporte"@es , "Vervoer"@nl , "Közlekedés"@hu , "Promet"@hr , "Transportas"@lt , "Transports"@fr , "Transports"@lv , "Transportes"@pt , "Μεταφορές"@el , "Liikenne"@fi , "Trasport"@mt , "Iompar"@ga , "Транспорт"@bg , "Doprava"@cs , "Doprava"@sk , "Transport"@ro , "Transport"@et , "Transport"@sv , "Transport"@no , "Trasporti"@it , "Transport"@pl , "Transport"@en , "Transport"@sl , "Transport"@da , "Verkehr"@de ;
        skos:topConceptOf   ns10:data-theme ;
        ns7:prefLabel       []  ;
        ns7:prefLabel       []  ;
        ns7:prefLabel       []  ;
        ns7:prefLabel       []  ;
        ns7:prefLabel       []  ;
        ns7:prefLabel       []  ;
        ns7:prefLabel       []  ;
        ns7:prefLabel       []  ;
        ns7:prefLabel       []  ;
        ns7:prefLabel       []  ;
        ns7:prefLabel       []  ;
        ns7:prefLabel       []  ;
        ns7:prefLabel       []  ;
        ns7:prefLabel       []  ;
        ns7:prefLabel       []  ;
        ns7:prefLabel       []  ;
        ns7:prefLabel       []  ;
        ns7:prefLabel       []  ;
        ns7:prefLabel       []  ;
        ns7:prefLabel       []  ;
        ns7:prefLabel       []  ;
        ns7:prefLabel       []  ;
        ns7:prefLabel       []  ;
        ns7:prefLabel       []  ;
        ns7:prefLabel       []  .
