@prefix owl:   <http://www.w3.org/2002/07/owl#> .
@prefix skos:  <http://www.w3.org/2004/02/skos/core#> .
@prefix rdfs:  <http://www.w3.org/2000/01/rdf-schema#> .
@prefix ns2:   <http://purl.org/dc/terms/> .
@prefix ns4:   <http://purl.org/dc/terms/> .
@prefix ns6:   <http://lemon-model.net/lemon#> .
@prefix ns5:   <http://publications.europa.eu/ontology/euvoc#> .
@prefix ns8:   <http://publications.europa.eu/ontology/authority/> .
@prefix ns7:   <http://www.w3.org/2008/05/skos-xl#> .
@prefix rdf:   <http://www.w3.org/1999/02/22-rdf-syntax-ns#> .
@prefix ns9:   <http://publications.europa.eu/ontology/authority/> .
@prefix ns10:  <http://publications.europa.eu/resource/authority/> .
@prefix dc:    <http://purl.org/dc/elements/1.1/> .

<http://publications.europa.eu/resource/authority/file-type/EXE>
        a                   ns5:FileType , skos:Concept ;
        ns6:context         <http://publications.europa.eu/resource/authority/use-context/IMMC> , <http://publications.europa.eu/resource/authority/use-context/DCAT_AP> , <http://publications.europa.eu/resource/authority/use-context/ODP> ;
        ns9:authority-code  "EXE" ;
        ns9:deprecated      "false" ;
        ns9:op-code         "EXE" ;
        ns9:op-mapped-code  []  ;
        ns9:start.use       "1978-01-01" ;
        ns5:startDate       "1978-01-01"^^<http://www.w3.org/2001/XMLSchema#date> ;
        ns5:status          <http://publications.europa.eu/resource/authority/concept-status/CURRENT> ;
        ns5:xlDefinition    []  ;
        ns5:xlNotation      []  ;
        ns5:xlNotation      []  ;
        ns10:op-code        "EXE" ;
        dc:identifier       "EXE" ;
        ns4:created         "2018-11-06"^^<http://www.w3.org/2001/XMLSchema#date> ;
        ns4:dateAccepted    "2018-11-28"^^<http://www.w3.org/2001/XMLSchema#date> ;
        ns4:dateSubmitted   "2018-11-14"^^<http://www.w3.org/2001/XMLSchema#date> ;
        owl:versionInfo     "20200624-0" ;
        skos:definition     "An executable file (the main execution point of a computer program) for DOS, OpenVMS, Microsoft Windows, Symbian or OS/2. Besides the executable program, many .exe files contain other components called resources, such as bitmap graphics and icons which the executable program may use for its graphical user interface."@en ;
        skos:inScheme       ns10:file-type ;
        skos:prefLabel      "EXE"@en ;
        skos:topConceptOf   ns10:file-type ;
        ns7:altLabel        []  ;
        ns7:prefLabel       []  .

<http://publications.europa.eu/resource/authority/file-type/FMX3>
        a                   ns5:FileType , skos:Concept ;
        ns6:context         <http://publications.europa.eu/resource/authority/use-context/IMMC> , <http://publications.europa.eu/resource/authority/use-context/EUDOR> , <http://publications.europa.eu/resource/authority/use-context/CELLAR> , <http://publications.europa.eu/resource/authority/use-context/ODP> ;
        ns9:authority-code  "FMX3" ;
        ns9:deprecated      "true" ;
        ns9:end.use         "2004-04-30" ;
        ns9:op-code         "FMX3" ;
        ns9:op-mapped-code  []  ;
        ns9:op-mapped-code  []  ;
        ns9:op-mapped-code  []  ;
        ns9:op-mapped-code  []  ;
        ns9:op-mapped-code  []  ;
        ns9:op-mapped-code  []  ;
        ns9:op-mapped-code  []  ;
        ns9:start.use       "1999-04-01" ;
        ns5:endDate         "2004-04-30"^^<http://www.w3.org/2001/XMLSchema#date> ;
        ns5:isTextual       true ;
        ns5:order           175 ;
        ns5:startDate       "1999-04-01"^^<http://www.w3.org/2001/XMLSchema#date> ;
        ns5:status          <http://publications.europa.eu/resource/authority/concept-status/DEPRECATED> ;
        ns5:xlDefinition    []  ;
        ns5:xlNotation      []  ;
        ns5:xlNotation      []  ;
        ns5:xlNotation      []  ;
        ns5:xlNotation      []  ;
        ns5:xlNotation      []  ;
        ns5:xlNotation      []  ;
        ns10:op-code        "FMX3" ;
        dc:identifier       "FMX3" ;
        ns4:created         "2012-03-19"^^<http://www.w3.org/2001/XMLSchema#date> ;
        ns4:dateAccepted    "2012-11-27"^^<http://www.w3.org/2001/XMLSchema#date> ;
        ns4:dateSubmitted   "2012-09-27"^^<http://www.w3.org/2001/XMLSchema#date> ;
        owl:versionInfo     "20200624-0" ;
        skos:definition     "Formex describes the format for the exchange of data between the Publication Office and its contractors. In particular, it defines the logical markup for documents which are published in the different series of the Offical Journal of the European Union. Formex 3 was a previous version of Formex actually used."@en ;
        skos:inScheme       ns10:file-type ;
        skos:prefLabel      "Formex 3"@en ;
        skos:topConceptOf   ns10:file-type ;
        ns7:altLabel        []  ;
        ns7:prefLabel       []  .

<http://publications.europa.eu/resource/authority/file-type/TXT>
        a                   ns5:FileType , skos:Concept ;
        ns6:context         <http://publications.europa.eu/resource/authority/use-context/CELLAR> , <http://publications.europa.eu/resource/authority/use-context/DCAT_AP> , <http://publications.europa.eu/resource/authority/use-context/ODP> , <http://publications.europa.eu/resource/authority/use-context/IMMC> , <http://publications.europa.eu/resource/authority/use-context/EUDOR> ;
        ns9:authority-code  "TXT" ;
        ns9:deprecated      "false" ;
        ns9:op-code         "TXT" ;
        ns9:op-mapped-code  []  ;
        ns9:op-mapped-code  []  ;
        ns9:op-mapped-code  []  ;
        ns9:op-mapped-code  []  ;
        ns9:op-mapped-code  []  ;
        ns9:op-mapped-code  []  ;
        ns9:op-mapped-code  []  ;
        ns9:start.use       "2012-09-01" ;
        ns5:isTextual       true ;
        ns5:nonPropExt      true ;
        ns5:order           300 ;
        ns5:startDate       "2012-09-01"^^<http://www.w3.org/2001/XMLSchema#date> ;
        ns5:status          <http://publications.europa.eu/resource/authority/concept-status/CURRENT> ;
        ns5:xlDefinition    []  ;
        ns5:xlNotation      []  ;
        ns5:xlNotation      []  ;
        ns5:xlNotation      []  ;
        ns5:xlNotation      []  ;
        ns5:xlNotation      []  ;
        ns10:op-code        "TXT" ;
        dc:identifier       "TXT" ;
        ns4:created         "2012-03-19"^^<http://www.w3.org/2001/XMLSchema#date> ;
        ns4:dateAccepted    "2012-11-27"^^<http://www.w3.org/2001/XMLSchema#date> ;
        ns4:dateSubmitted   "2012-09-27"^^<http://www.w3.org/2001/XMLSchema#date> ;
        owl:versionInfo     "20200624-0" ;
        skos:definition     "Plain text is the data (e.g. file contents) that represent only characters of readable material but not its graphical representation nor other objects. It may also include a limited number of characters that control simple arrangement of text, such as line breaks or tabulation characters. Plain text is different from formatted text, where style information is included, and from ‘binary files’ in which some portions must be interpreted as binary objects (encoded integers, real numbers, images, etc.)."@en ;
        skos:inScheme       ns10:file-type ;
        skos:prefLabel      "Plain text"@en ;
        skos:topConceptOf   ns10:file-type ;
        ns7:altLabel        []  ;
        ns7:prefLabel       []  .

<http://publications.europa.eu/resource/authority/file-type/MPEG2>
        a                   ns5:FileType , skos:Concept ;
        ns6:context         <http://publications.europa.eu/resource/authority/use-context/IMMC> ;
        ns9:authority-code  "MPEG2" ;
        ns9:deprecated      "false" ;
        ns9:op-code         "MPEG2" ;
        ns9:op-mapped-code  []  ;
        ns9:op-mapped-code  []  ;
        ns9:op-mapped-code  []  ;
        ns9:op-mapped-code  []  ;
        ns9:op-mapped-code  []  ;
        ns9:start.use       "2000-12-01" ;
        ns5:startDate       "2000-12-01"^^<http://www.w3.org/2001/XMLSchema#date> ;
        ns5:status          <http://publications.europa.eu/resource/authority/concept-status/CURRENT> ;
        ns5:xlDefinition    []  ;
        ns5:xlNotation      []  ;
        ns5:xlNotation      []  ;
        ns5:xlNotation      []  ;
        ns5:xlNotation      []  ;
        ns5:xlNotation      []  ;
        ns5:xlNotation      []  ;
        ns5:xlNotation      []  ;
        ns10:op-code        "MPEG2" ;
        dc:identifier       "MPEG2" ;
        ns4:created         "2016-08-18"^^<http://www.w3.org/2001/XMLSchema#date> ;
        ns4:dateAccepted    "2016-09-09"^^<http://www.w3.org/2001/XMLSchema#date> ;
        ns4:dateSubmitted   "2016-08-22"^^<http://www.w3.org/2001/XMLSchema#date> ;
        owl:versionInfo     "20200624-0" ;
        skos:definition     "MPEG-2 – Moving Picture Experts Group – is a standard for the generic coding of moving pictures and associated audio information. It describes a combination of lossy video compression and lossy audio data compression methods, which permit storage and transmission of movies using currently available storage media and transmission bandwidth."@en ;
        skos:inScheme       ns10:file-type ;
        skos:prefLabel      "MPEG-2"@en ;
        skos:topConceptOf   ns10:file-type ;
        ns7:altLabel        []  ;
        ns7:prefLabel       []  .

<http://publications.europa.eu/resource/authority/file-type/XLS>
        a                    skos:Concept , ns5:FileType ;
        ns6:context          <http://publications.europa.eu/resource/authority/use-context/OJEEP> , <http://publications.europa.eu/resource/authority/use-context/CELLAR> , <http://publications.europa.eu/resource/authority/use-context/DCAT_AP> , <http://publications.europa.eu/resource/authority/use-context/IMMC> , <http://publications.europa.eu/resource/authority/use-context/ODP> ;
        ns9:authority-code   "XLS" ;
        ns9:deprecated       "false" ;
        ns9:op-code          "XLS" ;
        ns9:op-mapped-code   []  ;
        ns9:op-mapped-code   []  ;
        ns9:op-mapped-code   []  ;
        ns9:op-mapped-code   []  ;
        ns9:op-mapped-code   []  ;
        ns9:op-mapped-code   []  ;
        ns9:op-mapped-code   []  ;
        ns9:start.use        "2012-09-01" ;
        ns5:isTextual        false ;
        ns5:machineReadable  true ;
        ns5:order            60 ;
        ns5:startDate        "2012-09-01"^^<http://www.w3.org/2001/XMLSchema#date> ;
        ns5:status           <http://publications.europa.eu/resource/authority/concept-status/CURRENT> ;
        ns5:xlDefinition     []  ;
        ns5:xlNotation       []  ;
        ns5:xlNotation       []  ;
        ns5:xlNotation       []  ;
        ns5:xlNotation       []  ;
        ns5:xlNotation       []  ;
        ns10:op-code         "XLS" ;
        dc:identifier        "XLS" ;
        ns4:created          "2012-03-19"^^<http://www.w3.org/2001/XMLSchema#date> ;
        ns4:dateAccepted     "2012-11-27"^^<http://www.w3.org/2001/XMLSchema#date> ;
        ns4:dateSubmitted    "2012-09-27"^^<http://www.w3.org/2001/XMLSchema#date> ;
        owl:versionInfo      "20200624-0" ;
        skos:definition      "XLS is a proprietary binary file format used for Microsoft Excel spreadsheet which features calculation, graphing tools, pivot tables and a macro programming language."@en ;
        skos:inScheme        ns10:file-type ;
        skos:prefLabel       "Excel XLS"@en ;
        skos:topConceptOf    ns10:file-type ;
        ns7:altLabel         []  ;
        ns7:prefLabel        []  .

<http://publications.europa.eu/resource/authority/file-type/PDFA2B>
        a                   ns5:FileType , skos:Concept ;
        ns6:context         <http://publications.europa.eu/resource/authority/use-context/IMMC> ;
        ns9:authority-code  "PDFA2B" ;
        ns9:deprecated      "false" ;
        ns9:op-code         "PDFA2B" ;
        ns9:op-mapped-code  []  ;
        ns9:op-mapped-code  []  ;
        ns9:op-mapped-code  []  ;
        ns9:op-mapped-code  []  ;
        ns9:op-mapped-code  []  ;
        ns9:op-mapped-code  []  ;
        ns9:start.use       "2011-07-01" ;
        ns5:isTextual       false ;
        ns5:order           246 ;
        ns5:startDate       "2011-07-01"^^<http://www.w3.org/2001/XMLSchema#date> ;
        ns5:status          <http://publications.europa.eu/resource/authority/concept-status/CURRENT> ;
        ns5:xlDefinition    []  ;
        ns5:xlNotation      []  ;
        ns5:xlNotation      []  ;
        ns5:xlNotation      []  ;
        ns5:xlNotation      []  ;
        ns5:xlNotation      []  ;
        ns10:op-code        "PDFA2B" ;
        dc:identifier       "PDFA2B" ;
        ns4:created         "2016-08-18"^^<http://www.w3.org/2001/XMLSchema#date> ;
        ns4:dateAccepted    "2016-09-09"^^<http://www.w3.org/2001/XMLSchema#date> ;
        ns4:dateSubmitted   "2016-08-22"^^<http://www.w3.org/2001/XMLSchema#date> ;
        owl:versionInfo     "20200624-0" ;
        skos:definition     "PDF/A-2 is the Part 2 of the PDF standard and specifies three levels of conformance for PDF files. PDF/A-2a corresponds to conformance level a in PDF/A-2 (basic)."@en ;
        skos:inScheme       ns10:file-type ;
        skos:prefLabel      "PDF/A-2b"@en ;
        skos:topConceptOf   ns10:file-type ;
        ns7:altLabel        []  ;
        ns7:prefLabel       []  .

<http://publications.europa.eu/resource/authority/file-type/XLSM>
        a                   ns5:FileType , skos:Concept ;
        ns6:context         <http://publications.europa.eu/resource/authority/use-context/ODP> , <http://publications.europa.eu/resource/authority/use-context/IMMC> ;
        ns9:authority-code  "XLSM" ;
        ns9:deprecated      "false" ;
        ns9:op-code         "XLSM" ;
        ns9:op-mapped-code  []  ;
        ns9:start.use       "2007-01-30" ;
        ns5:startDate       "2007-01-30"^^<http://www.w3.org/2001/XMLSchema#date> ;
        ns5:status          <http://publications.europa.eu/resource/authority/concept-status/CURRENT> ;
        ns5:xlDefinition    []  ;
        ns5:xlNotation      []  ;
        ns5:xlNotation      []  ;
        ns10:op-code        "XLSM" ;
        dc:identifier       "XLSM" ;
        ns4:created         "2019-08-05"^^<http://www.w3.org/2001/XMLSchema#date> ;
        ns4:dateAccepted    "2019-08-27"^^<http://www.w3.org/2001/XMLSchema#date> ;
        ns4:dateSubmitted   "2019-08-13"^^<http://www.w3.org/2001/XMLSchema#date> ;
        owl:versionInfo     "20200624-0" ;
        skos:definition     "An Excel Macro-enabled Workbook contains worksheets of cells arranged by rows and columns as well as embedded macros programmed in the Visual Basic for Applications (VBA) language. XLSM files are saved in the Open XML format introduced in Microsoft Office 2007. XLSM files are XLSX files, but with macros enabled."@en ;
        skos:inScheme       ns10:file-type ;
        skos:prefLabel      "XLSM"@en ;
        skos:topConceptOf   ns10:file-type ;
        ns7:altLabel        []  ;
        ns7:prefLabel       []  .

<http://publications.europa.eu/resource/authority/file-type/OWL>
        a                   ns5:FileType , skos:Concept ;
        ns6:context         <http://publications.europa.eu/resource/authority/use-context/ODP> , <http://publications.europa.eu/resource/authority/use-context/IMMC> , <http://publications.europa.eu/resource/authority/use-context/CELLAR> ;
        ns9:authority-code  "OWL" ;
        ns9:deprecated      "false" ;
        ns9:op-code         "OWL" ;
        ns9:op-mapped-code  []  ;
        ns9:op-mapped-code  []  ;
        ns9:op-mapped-code  []  ;
        ns9:start.use       "2012-09-01" ;
        ns5:startDate       "2012-09-01"^^<http://www.w3.org/2001/XMLSchema#date> ;
        ns5:status          <http://publications.europa.eu/resource/authority/concept-status/CURRENT> ;
        ns5:xlDefinition    []  ;
        ns5:xlNotation      []  ;
        ns5:xlNotation      []  ;
        ns5:xlNotation      []  ;
        ns5:xlNotation      []  ;
        ns10:op-code        "OWL" ;
        dc:identifier       "OWL" ;
        ns4:created         "2012-09-01"^^<http://www.w3.org/2001/XMLSchema#date> ;
        ns4:dateAccepted    "2014-03-12"^^<http://www.w3.org/2001/XMLSchema#date> ;
        ns4:dateSubmitted   "2014-02-19"^^<http://www.w3.org/2001/XMLSchema#date> ;
        owl:versionInfo     "20200624-0" ;
        skos:definition     "OWL – Web Ontology Language – is a family of knowledge representation languages for authoring ontologies."@en ;
        skos:inScheme       ns10:file-type ;
        skos:prefLabel      "OWL"@en ;
        skos:topConceptOf   ns10:file-type ;
        ns7:altLabel        []  ;
        ns7:prefLabel       []  .

<http://publications.europa.eu/resource/authority/file-type/RDF_XML>
        a                    skos:Concept , ns5:FileType ;
        ns6:context          <http://publications.europa.eu/resource/authority/use-context/IMMC> , <http://publications.europa.eu/resource/authority/use-context/CELLAR> , <http://publications.europa.eu/resource/authority/use-context/ODP> , <http://publications.europa.eu/resource/authority/use-context/DCAT_AP> ;
        ns9:authority-code   "RDF_XML" ;
        ns9:deprecated       "false" ;
        ns9:op-code          "RDF_XML" ;
        ns9:op-mapped-code   []  ;
        ns9:op-mapped-code   []  ;
        ns9:op-mapped-code   []  ;
        ns9:op-mapped-code   []  ;
        ns9:op-mapped-code   []  ;
        ns9:op-mapped-code   []  ;
        ns9:op-mapped-code   []  ;
        ns9:op-mapped-code   []  ;
        ns9:start.use        "2012-09-01" ;
        ns5:isTextual        true ;
        ns5:machineReadable  true ;
        ns5:nonPropExt       true ;
        ns5:order            120 ;
        ns5:startDate        "2012-09-01"^^<http://www.w3.org/2001/XMLSchema#date> ;
        ns5:status           <http://publications.europa.eu/resource/authority/concept-status/CURRENT> ;
        ns5:xlDefinition     []  ;
        ns5:xlNotation       []  ;
        ns5:xlNotation       []  ;
        ns5:xlNotation       []  ;
        ns5:xlNotation       []  ;
        ns5:xlNotation       []  ;
        ns10:op-code         "RDF_XML" ;
        dc:identifier        "RDF_XML" ;
        ns4:created          "2012-03-19"^^<http://www.w3.org/2001/XMLSchema#date> ;
        ns4:dateAccepted     "2012-11-27"^^<http://www.w3.org/2001/XMLSchema#date> ;
        ns4:dateSubmitted    "2012-09-27"^^<http://www.w3.org/2001/XMLSchema#date> ;
        owl:versionInfo      "20200624-0" ;
        skos:definition      "RDF XML is a syntax, defined by the W3C, to express (i.e. serialize) an RDF graph as an XML document."@en ;
        skos:inScheme        ns10:file-type ;
        skos:prefLabel       "RDF XML"@en ;
        skos:topConceptOf    ns10:file-type ;
        ns7:altLabel         []  ;
        ns7:prefLabel        []  .

<http://publications.europa.eu/resource/authority/file-type/MOP>
        a                   skos:Concept , ns5:FileType ;
        ns6:context         <http://publications.europa.eu/resource/authority/use-context/CELLAR> , <http://publications.europa.eu/resource/authority/use-context/DCAT_AP> , <http://publications.europa.eu/resource/authority/use-context/ODP> , <http://publications.europa.eu/resource/authority/use-context/IMMC> ;
        ns9:authority-code  "MOP" ;
        ns9:deprecated      "false" ;
        ns9:op-code         "MOP" ;
        ns9:op-mapped-code  []  ;
        ns9:start.use       "2013-09-18" ;
        ns5:startDate       "2013-09-18"^^<http://www.w3.org/2001/XMLSchema#date> ;
        ns5:status          <http://publications.europa.eu/resource/authority/concept-status/CURRENT> ;
        ns5:xlDefinition    []  ;
        ns5:xlNotation      []  ;
        ns5:xlNotation      []  ;
        ns10:op-code        "MOP" ;
        dc:identifier       "MOP" ;
        ns4:created         "2013-09-18"^^<http://www.w3.org/2001/XMLSchema#date> ;
        ns4:dateSubmitted   "2013-09-26"^^<http://www.w3.org/2001/XMLSchema#date> ;
        owl:versionInfo     "20200624-0" ;
        skos:definition     "MOP is a chemical file format used by MOPAC. MOPAC is a popular computer program used in computational chemistry. It is designed to implement semi-empirical quantum chemistry algorithms."@en ;
        skos:inScheme       ns10:file-type ;
        skos:prefLabel      "MOP"@en ;
        skos:topConceptOf   ns10:file-type ;
        ns7:altLabel        []  ;
        ns7:prefLabel       []  .

<http://publications.europa.eu/resource/authority/file-type/OP_DATPRO>
        a                  skos:Concept , ns5:FileType ;
        ns9:op-code        "OP_DATPRO" ;
        ns5:status         <http://publications.europa.eu/resource/authority/concept-status/CURRENT> ;
        ns10:op-code       "OP_DATPRO" ;
        dc:identifier      "OP_DATPRO" ;
        ns4:created        "2012-03-19"^^<http://www.w3.org/2001/XMLSchema#date> ;
        owl:versionInfo    "20200624-0" ;
        skos:inScheme      ns10:file-type ;
        skos:prefLabel     "НЕОКОНЧАТЕЛНИ ДАННИ"@bg , "Tillfälliga uppgifter"@sv , "Dejta provviżorja"@mt , "Laikinieji duomenys"@lt , "Midlertidige data"@da , "Ideiglenes adatok"@hu , "Προσωρινά δεδομένα"@el , "Provisional data"@en , "Sonraí sealadacha"@ga , "Dati provvisori"@it , "Dados provisórios"@pt , "Začasni podatki"@sl , "Privremeni podaci"@hr , "Datos provisionales"@es , "Alustavat tiedot"@fi , "Voorlopige gegevens"@nl , "Predbežné údaje"@sk , "Esialgsed andmed"@et , "Vorläufige Daten"@de , "Dane tymczasowe"@pl , "Date provizorii"@ro , "Provizoriski dati"@lv , "Données provisoires"@fr , "Předběžné údaje"@cs ;
        skos:topConceptOf  ns10:file-type ;
        ns7:prefLabel      []  ;
        ns7:prefLabel      []  ;
        ns7:prefLabel      []  ;
        ns7:prefLabel      []  ;
        ns7:prefLabel      []  ;
        ns7:prefLabel      []  ;
        ns7:prefLabel      []  ;
        ns7:prefLabel      []  ;
        ns7:prefLabel      []  ;
        ns7:prefLabel      []  ;
        ns7:prefLabel      []  ;
        ns7:prefLabel      []  ;
        ns7:prefLabel      []  ;
        ns7:prefLabel      []  ;
        ns7:prefLabel      []  ;
        ns7:prefLabel      []  ;
        ns7:prefLabel      []  ;
        ns7:prefLabel      []  ;
        ns7:prefLabel      []  ;
        ns7:prefLabel      []  ;
        ns7:prefLabel      []  ;
        ns7:prefLabel      []  ;
        ns7:prefLabel      []  ;
        ns7:prefLabel      []  .

<http://publications.europa.eu/resource/authority/file-type/LZMA>
        a                   skos:Concept , ns5:FileType ;
        ns6:context         <http://publications.europa.eu/resource/authority/use-context/IMMC> , <http://publications.europa.eu/resource/authority/use-context/DCAT_AP> ;
        ns9:authority-code  "LZMA" ;
        ns9:deprecated      "false" ;
        ns9:op-code         "LZMA" ;
        ns9:op-mapped-code  []  ;
        ns9:start.use       "2000-01-01" ;
        ns5:startDate       "2000-01-01"^^<http://www.w3.org/2001/XMLSchema#date> ;
        ns5:status          <http://publications.europa.eu/resource/authority/concept-status/CURRENT> ;
        ns5:xlDefinition    []  ;
        ns5:xlNotation      []  ;
        ns5:xlNotation      []  ;
        ns10:op-code        "LZMA" ;
        dc:identifier       "LZMA" ;
        ns4:created         "2020-05-15"^^<http://www.w3.org/2001/XMLSchema#date> ;
        ns4:dateAccepted    "2020-06-04"^^<http://www.w3.org/2001/XMLSchema#date> ;
        ns4:dateSubmitted   "2020-05-19"^^<http://www.w3.org/2001/XMLSchema#date> ;
        owl:versionInfo     "20200624-0" ;
        skos:definition     "Compressed file produced using LZMA (Lempel-Ziv-Markov) chain algorithm."@en ;
        skos:inScheme       ns10:file-type ;
        skos:prefLabel      "lzma"@en ;
        skos:topConceptOf   ns10:file-type ;
        ns7:altLabel        []  ;
        ns7:prefLabel       []  .

<http://publications.europa.eu/resource/authority/file-type/PPS>
        a                   skos:Concept , ns5:FileType ;
        ns6:context         <http://publications.europa.eu/resource/authority/use-context/ODP> , <http://publications.europa.eu/resource/authority/use-context/CELLAR> , <http://publications.europa.eu/resource/authority/use-context/IMMC> ;
        ns9:authority-code  "PPS" ;
        ns9:deprecated      "false" ;
        ns9:op-code         "PPS" ;
        ns9:op-mapped-code  []  ;
        ns9:op-mapped-code  []  ;
        ns9:start.use       "2012-09-01" ;
        ns5:startDate       "2012-09-01"^^<http://www.w3.org/2001/XMLSchema#date> ;
        ns5:status          <http://publications.europa.eu/resource/authority/concept-status/CURRENT> ;
        ns5:xlDefinition    []  ;
        ns5:xlNotation      []  ;
        ns5:xlNotation      []  ;
        ns5:xlNotation      []  ;
        ns10:op-code        "PPS" ;
        dc:identifier       "PPS" ;
        ns4:created         "2012-09-01"^^<http://www.w3.org/2001/XMLSchema#date> ;
        ns4:dateAccepted    "2014-03-12"^^<http://www.w3.org/2001/XMLSchema#date> ;
        ns4:dateSubmitted   "2014-02-19"^^<http://www.w3.org/2001/XMLSchema#date> ;
        owl:versionInfo     "20200624-0" ;
        skos:definition     "PPS – PowerPoint 97–2003 binary slide show – is a binary filaname extension of Microsoft PowerPoint presentation program. PowerPoint was originally designed to provide visuals for group presentations within business organizations, but has come to be very widely used in many other communication situations, both in business and beyond."@en ;
        skos:inScheme       ns10:file-type ;
        skos:prefLabel      "PowerPoint Slide Show"@en ;
        skos:topConceptOf   ns10:file-type ;
        ns7:altLabel        []  ;
        ns7:prefLabel       []  .

<http://publications.europa.eu/resource/authority/file-type/BZIP2>
        a                   skos:Concept , ns5:FileType ;
        ns6:context         <http://publications.europa.eu/resource/authority/use-context/IMMC> , <http://publications.europa.eu/resource/authority/use-context/DCAT_AP> ;
        ns9:authority-code  "BZIP2" ;
        ns9:deprecated      "false" ;
        ns9:op-code         "BZIP2" ;
        ns9:op-mapped-code  []  ;
        ns9:start.use       "1996-07-18" ;
        ns5:startDate       "1996-07-18"^^<http://www.w3.org/2001/XMLSchema#date> ;
        ns5:status          <http://publications.europa.eu/resource/authority/concept-status/CURRENT> ;
        ns5:xlDefinition    []  ;
        ns5:xlNotation      []  ;
        ns5:xlNotation      []  ;
        ns10:op-code        "BZIP2" ;
        dc:identifier       "BZIP2" ;
        ns4:created         "2020-05-15"^^<http://www.w3.org/2001/XMLSchema#date> ;
        ns4:dateAccepted    "2020-06-04"^^<http://www.w3.org/2001/XMLSchema#date> ;
        ns4:dateSubmitted   "2020-05-19"^^<http://www.w3.org/2001/XMLSchema#date> ;
        owl:versionInfo     "20200624-0" ;
        skos:definition     "An open source, patent- and royalty-free compression format. The compression algorithm is a Burrows-Wheeler transform followed by a move-to-front transform and finally Huffman coding."@en ;
        skos:inScheme       ns10:file-type ;
        skos:prefLabel      "bzip2"@en ;
        skos:topConceptOf   ns10:file-type ;
        ns7:altLabel        []  ;
        ns7:prefLabel       []  .

<http://publications.europa.eu/resource/authority/file-type/DTD_XML>
        a                   ns5:FileType , skos:Concept ;
        ns6:context         <http://publications.europa.eu/resource/authority/use-context/CELLAR> , <http://publications.europa.eu/resource/authority/use-context/IMMC> , <http://publications.europa.eu/resource/authority/use-context/ODP> ;
        ns9:authority-code  "DTD_XML" ;
        ns9:deprecated      "false" ;
        ns9:op-code         "DTD_XML" ;
        ns9:op-mapped-code  []  ;
        ns9:op-mapped-code  []  ;
        ns9:start.use       "2012-09-01" ;
        ns5:startDate       "2012-09-01"^^<http://www.w3.org/2001/XMLSchema#date> ;
        ns5:status          <http://publications.europa.eu/resource/authority/concept-status/CURRENT> ;
        ns5:xlDefinition    []  ;
        ns5:xlNotation      []  ;
        ns5:xlNotation      []  ;
        ns5:xlNotation      []  ;
        ns10:op-code        "DTD_XML" ;
        dc:identifier       "DTD_XML" ;
        ns4:created         "2012-09-01"^^<http://www.w3.org/2001/XMLSchema#date> ;
        ns4:dateAccepted    "2014-03-12"^^<http://www.w3.org/2001/XMLSchema#date> ;
        ns4:dateSubmitted   "2014-02-19"^^<http://www.w3.org/2001/XMLSchema#date> ;
        owl:versionInfo     "20200624-0" ;
        skos:definition     "XML – Extensible Markup Language – is a markup language that defines a set of rules for encoding documents in a format that is both human-readable and machine-readable. DTD – document type definition – is a set of markup declarations that define a document type for an SGML-family markup language (SGML, XML, HTML). It defines the legal building blocks of an XML document, the document structure with a list of legal elements and attributes. XML uses a subset of SGML DTD."@en ;
        skos:inScheme       ns10:file-type ;
        skos:prefLabel      "XML DTD"@en ;
        skos:topConceptOf   ns10:file-type ;
        ns7:altLabel        []  ;
        ns7:prefLabel       []  .

<http://publications.europa.eu/resource/authority/file-type/MRSID>
        a                   ns5:FileType , skos:Concept ;
        ns6:context         <http://publications.europa.eu/resource/authority/use-context/DCAT_AP> , <http://publications.europa.eu/resource/authority/use-context/ODP> , <http://publications.europa.eu/resource/authority/use-context/IMMC> ;
        ns9:authority-code  "MRSID" ;
        ns9:deprecated      "false" ;
        ns9:op-code         "MRSID" ;
        ns9:op-mapped-code  []  ;
        ns9:start.use       "1996-01-01" ;
        ns5:startDate       "1996-01-01"^^<http://www.w3.org/2001/XMLSchema#date> ;
        ns5:status          <http://publications.europa.eu/resource/authority/concept-status/CURRENT> ;
        ns5:xlDefinition    []  ;
        ns5:xlNotation      []  ;
        ns5:xlNotation      []  ;
        ns5:xlNotation      []  ;
        ns5:xlNotation      []  ;
        ns10:op-code        "MRSID" ;
        dc:identifier       "MRSID" ;
        ns4:created         "2018-11-06"^^<http://www.w3.org/2001/XMLSchema#date> ;
        ns4:dateAccepted    "2018-11-28"^^<http://www.w3.org/2001/XMLSchema#date> ;
        ns4:dateSubmitted   "2018-11-14"^^<http://www.w3.org/2001/XMLSchema#date> ;
        owl:versionInfo     "20200624-0" ;
        skos:definition     "Multiresolution seamless image database (MrSID) is a file format developed and patented by LizardTech for encoding of georeferenced raster graphics, such as orthophotos. With this format, large raster image files such as aerial photographs or satellite imagery are compressed and can be quickly viewed without having to decompress the entire file."@en ;
        skos:inScheme       ns10:file-type ;
        skos:prefLabel      "MrSID"@en ;
        skos:topConceptOf   ns10:file-type ;
        ns7:altLabel        []  ;
        ns7:prefLabel       []  .

<http://publications.europa.eu/resource/authority/file-type/HTML>
        a                   ns5:FileType , skos:Concept ;
        ns6:context         <http://publications.europa.eu/resource/authority/use-context/DCAT_AP> , <http://publications.europa.eu/resource/authority/use-context/CELLAR> , <http://publications.europa.eu/resource/authority/use-context/IMMC> , <http://publications.europa.eu/resource/authority/use-context/ODP> ;
        ns9:authority-code  "HTML" ;
        ns9:deprecated      "false" ;
        ns9:op-code         "HTML" ;
        ns9:op-mapped-code  []  ;
        ns9:op-mapped-code  []  ;
        ns9:op-mapped-code  []  ;
        ns9:op-mapped-code  []  ;
        ns9:op-mapped-code  []  ;
        ns9:op-mapped-code  []  ;
        ns9:op-mapped-code  []  ;
        ns9:op-mapped-code  []  ;
        ns9:start.use       "2012-09-01" ;
        ns5:isTextual       true ;
        ns5:nonPropExt      true ;
        ns5:order           320 ;
        ns5:startDate       "2012-09-01"^^<http://www.w3.org/2001/XMLSchema#date> ;
        ns5:status          <http://publications.europa.eu/resource/authority/concept-status/CURRENT> ;
        ns5:xlDefinition    []  ;
        ns5:xlNotation      []  ;
        ns5:xlNotation      []  ;
        ns5:xlNotation      []  ;
        ns5:xlNotation      []  ;
        ns5:xlNotation      []  ;
        ns5:xlNotation      []  ;
        ns10:op-code        "HTML" ;
        dc:identifier       "HTML" ;
        ns4:created         "2012-03-19"^^<http://www.w3.org/2001/XMLSchema#date> ;
        ns4:dateAccepted    "2012-11-27"^^<http://www.w3.org/2001/XMLSchema#date> ;
        ns4:dateSubmitted   "2012-09-27"^^<http://www.w3.org/2001/XMLSchema#date> ;
        owl:versionInfo     "20200624-0" ;
        skos:definition     "HTML is the standard markup language used to create web pages and its elements form the building blocks of all websites."@en ;
        skos:inScheme       ns10:file-type ;
        skos:prefLabel      "HTML"@en ;
        skos:topConceptOf   ns10:file-type ;
        ns7:altLabel        []  ;
        ns7:prefLabel       []  .

<http://publications.europa.eu/resource/authority/file-type/PPSX>
        a                   ns5:FileType , skos:Concept ;
        ns6:context         <http://publications.europa.eu/resource/authority/use-context/CELLAR> , <http://publications.europa.eu/resource/authority/use-context/IMMC> ;
        ns9:authority-code  "PPSX" ;
        ns9:deprecated      "false" ;
        ns9:op-code         "PPSX" ;
        ns9:op-mapped-code  []  ;
        ns9:op-mapped-code  []  ;
        ns9:op-mapped-code  []  ;
        ns9:op-mapped-code  []  ;
        ns9:op-mapped-code  []  ;
        ns9:op-mapped-code  []  ;
        ns9:start.use       "2012-09-01" ;
        ns5:isTextual       false ;
        ns5:order           150 ;
        ns5:startDate       "2012-09-01"^^<http://www.w3.org/2001/XMLSchema#date> ;
        ns5:status          <http://publications.europa.eu/resource/authority/concept-status/CURRENT> ;
        ns5:xlDefinition    []  ;
        ns5:xlNotation      []  ;
        ns5:xlNotation      []  ;
        ns5:xlNotation      []  ;
        ns5:xlNotation      []  ;
        ns5:xlNotation      []  ;
        ns10:op-code        "PPSX" ;
        dc:identifier       "PPSX" ;
        ns4:created         "2012-03-19"^^<http://www.w3.org/2001/XMLSchema#date> ;
        ns4:dateAccepted    "2012-11-27"^^<http://www.w3.org/2001/XMLSchema#date> ;
        ns4:dateSubmitted   "2012-09-27"^^<http://www.w3.org/2001/XMLSchema#date> ;
        owl:versionInfo     "20200624-0" ;
        skos:definition     "PPSX – PowerPoint 2007 XML slide show – is an XML filename extension of Microsoft PowerPoint presentation program. PowerPoint was originally designed to provide visuals for group presentations within business organizations, but has come to be very widely used in many other communication situations, both in business and beyond."@en ;
        skos:inScheme       ns10:file-type ;
        skos:prefLabel      "PowerPoint PPSX"@en ;
        skos:topConceptOf   ns10:file-type ;
        ns7:altLabel        []  ;
        ns7:prefLabel       []  .

<http://publications.europa.eu/resource/authority/file-type/TAB_RSTR>
        a                   ns5:FileType , skos:Concept ;
        ns6:context         <http://publications.europa.eu/resource/authority/use-context/IMMC> , <http://publications.europa.eu/resource/authority/use-context/CELLAR> ;
        ns9:authority-code  "TAB_RSTR" ;
        ns9:deprecated      "false" ;
        ns9:op-code         "TAB_RSTR" ;
        ns9:op-mapped-code  []  ;
        ns9:start.use       "2000-03-26" ;
        ns5:startDate       "2000-03-26"^^<http://www.w3.org/2001/XMLSchema#date> ;
        ns5:status          <http://publications.europa.eu/resource/authority/concept-status/CURRENT> ;
        ns5:xlDefinition    []  ;
        ns5:xlNotation      []  ;
        ns5:xlNotation      []  ;
        ns10:op-code        "TAB_RSTR" ;
        dc:identifier       "TAB_RSTR" ;
        ns4:created         "2015-04-20"^^<http://www.w3.org/2001/XMLSchema#date> ;
        ns4:dateSubmitted   "2015-04-22"^^<http://www.w3.org/2001/XMLSchema#date> ;
        owl:versionInfo     "20200624-0" ;
        skos:definition     "MapInfo TAB raster file is the media type which shall be used for the MapInfo Raster TAB format. This media type is incomplete as it lacks a reference to the specification of the format."@en ;
        skos:inScheme       ns10:file-type ;
        skos:prefLabel      "MapInfo TAB raster file"@en ;
        skos:topConceptOf   ns10:file-type ;
        ns7:altLabel        []  ;
        ns7:prefLabel       []  .

<http://publications.europa.eu/resource/authority/file-type/XLIFF>
        a                   skos:Concept , ns5:FileType ;
        ns6:context         <http://publications.europa.eu/resource/authority/use-context/ODP> , <http://publications.europa.eu/resource/authority/use-context/DCAT_AP> , <http://publications.europa.eu/resource/authority/use-context/IMMC> , <http://publications.europa.eu/resource/authority/use-context/PUB> , <http://publications.europa.eu/resource/authority/use-context/CELLAR> ;
        ns9:authority-code  "XLIFF" ;
        ns9:deprecated      "false" ;
        ns9:op-code         "XLIFF" ;
        ns9:op-mapped-code  []  ;
        ns9:start.use       "2001-05-30" ;
        ns5:startDate       "2001-05-30"^^<http://www.w3.org/2001/XMLSchema#date> ;
        ns5:status          <http://publications.europa.eu/resource/authority/concept-status/CURRENT> ;
        ns5:xlDefinition    []  ;
        ns5:xlNotation      []  ;
        ns5:xlNotation      []  ;
        ns10:op-code        "XLIFF" ;
        dc:identifier       "XLIFF" ;
        ns4:created         "2015-03-23"^^<http://www.w3.org/2001/XMLSchema#date> ;
        ns4:dateSubmitted   "2015-04-22"^^<http://www.w3.org/2001/XMLSchema#date> ;
        owl:versionInfo     "20200624-0" ;
        skos:definition     "XLIFF is the XML Localisation Interchange File Format designed by a group of multilingual content publishers, software providers, localization service providers, localization tools providers and researchers. It is intended to give any multilingual content owner a single interchange file format that can be understood by any localization provider, using any conformant localization tool. While the primary focus is on being a lossless interchange format, usage of XLIFF as a processing format is neither encouraged nor discouraged or prohibited."@en ;
        skos:inScheme       ns10:file-type ;
        skos:prefLabel      "XLIFF"@en ;
        skos:topConceptOf   ns10:file-type ;
        ns7:altLabel        []  ;
        ns7:prefLabel       []  .

<http://publications.europa.eu/resource/authority/file-type/MAP_SRVC>
        a                   skos:Concept , ns5:FileType ;
        ns6:context         <http://publications.europa.eu/resource/authority/use-context/IMMC> , <http://publications.europa.eu/resource/authority/use-context/CELLAR> , <http://publications.europa.eu/resource/authority/use-context/ODP> ;
        ns9:authority-code  "MAP_SRVC" ;
        ns9:deprecated      "false" ;
        ns9:op-code         "MAP_SRVC" ;
        ns9:start.use       "2010-01-01" ;
        ns5:startDate       "2010-01-01"^^<http://www.w3.org/2001/XMLSchema#date> ;
        ns5:status          <http://publications.europa.eu/resource/authority/concept-status/CURRENT> ;
        ns5:xlDefinition    []  ;
        ns5:xlNotation      []  ;
        ns10:op-code        "MAP_SRVC" ;
        dc:identifier       "MAP_SRVC" ;
        ns4:created         "2015-04-21"^^<http://www.w3.org/2001/XMLSchema#date> ;
        ns4:dateSubmitted   "2015-04-22"^^<http://www.w3.org/2001/XMLSchema#date> ;
        owl:versionInfo     "20200624-0" ;
        skos:definition     "Esri's ArcGIS is a geographic information system (GIS) for working with maps and geographic information. Map services offer access to map and layer content."@en ;
        skos:inScheme       ns10:file-type ;
        skos:prefLabel      "ArcGIS Map Service"@en ;
        skos:topConceptOf   ns10:file-type ;
        ns7:altLabel        []  ;
        ns7:prefLabel       []  .

<http://publications.europa.eu/resource/authority/file-type/GRID>
        a                   ns5:FileType , skos:Concept ;
        ns6:context         <http://publications.europa.eu/resource/authority/use-context/CELLAR> , <http://publications.europa.eu/resource/authority/use-context/ODP> , <http://publications.europa.eu/resource/authority/use-context/IMMC> ;
        ns9:authority-code  "GRID" ;
        ns9:deprecated      "false" ;
        ns9:op-code         "GRID" ;
        ns9:start.use       "2013-08-21" ;
        ns5:startDate       "2013-08-21"^^<http://www.w3.org/2001/XMLSchema#date> ;
        ns5:status          <http://publications.europa.eu/resource/authority/concept-status/CURRENT> ;
        ns5:xlDefinition    []  ;
        ns5:xlNotation      []  ;
        ns5:xlNotation      []  ;
        ns10:op-code        "GRID" ;
        dc:identifier       "GRID" ;
        ns4:created         "2017-11-16"^^<http://www.w3.org/2001/XMLSchema#date> ;
        ns4:dateAccepted    "2017-11-20"^^<http://www.w3.org/2001/XMLSchema#date> ;
        ns4:dateSubmitted   "2017-11-13"^^<http://www.w3.org/2001/XMLSchema#date> ;
        owl:versionInfo     "20200624-0" ;
        skos:definition     "Esri binary grid is a proprietary binary variation of an Esri grid, a raster GIS file format developed by Esri. It is also known as an ARC/INFO GRID or ARC GRID. It differs from the other Esri grid variation, a non-proprietary ASCII format."@en ;
        skos:inScheme       ns10:file-type ;
        skos:prefLabel      "Esri binary grid"@en ;
        skos:topConceptOf   ns10:file-type ;
        ns7:altLabel        []  ;
        ns7:prefLabel       []  .

<http://publications.europa.eu/resource/authority/file-type/PDFX2A>
        a                   ns5:FileType , skos:Concept ;
        ns6:context         <http://publications.europa.eu/resource/authority/use-context/CELLAR> , <http://publications.europa.eu/resource/authority/use-context/IMMC> , <http://publications.europa.eu/resource/authority/use-context/EUDOR> ;
        ns9:authority-code  "PDFX2A" ;
        ns9:deprecated      "false" ;
        ns9:op-code         "PDFX2A" ;
        ns9:op-mapped-code  []  ;
        ns9:op-mapped-code  []  ;
        ns9:op-mapped-code  []  ;
        ns9:op-mapped-code  []  ;
        ns9:op-mapped-code  []  ;
        ns9:op-mapped-code  []  ;
        ns9:start.use       "2003-12-01" ;
        ns5:isTextual       false ;
        ns5:order           242 ;
        ns5:startDate       "2003-12-01"^^<http://www.w3.org/2001/XMLSchema#date> ;
        ns5:status          <http://publications.europa.eu/resource/authority/concept-status/CURRENT> ;
        ns5:xlDefinition    []  ;
        ns5:xlNotation      []  ;
        ns5:xlNotation      []  ;
        ns5:xlNotation      []  ;
        ns5:xlNotation      []  ;
        ns5:xlNotation      []  ;
        ns10:op-code        "PDFX2A" ;
        dc:identifier       "PDFX2A" ;
        ns4:created         "2017-08-22"^^<http://www.w3.org/2001/XMLSchema#date> ;
        ns4:dateAccepted    "2017-09-05"^^<http://www.w3.org/2001/XMLSchema#date> ;
        ns4:dateSubmitted   "2017-08-22"^^<http://www.w3.org/2001/XMLSchema#date> ;
        owl:versionInfo     "20200624-0" ;
        skos:definition     "PDF/X-2a is a PDF specification in which colour-managed, CMYK and spot colour data are supported in any combination."@en ;
        skos:inScheme       ns10:file-type ;
        skos:prefLabel      "PDF/X-2a"@en ;
        skos:topConceptOf   ns10:file-type ;
        ns7:altLabel        []  ;
        ns7:prefLabel       []  .

<http://publications.europa.eu/resource/authority/file-type/GMZ>
        a                   ns5:FileType , skos:Concept ;
        ns6:context         <http://publications.europa.eu/resource/authority/use-context/IMMC> , <http://publications.europa.eu/resource/authority/use-context/ODP> , <http://publications.europa.eu/resource/authority/use-context/CELLAR> ;
        ns9:authority-code  "GMZ" ;
        ns9:deprecated      "false" ;
        ns9:op-code         "GMZ" ;
        ns9:op-mapped-code  []  ;
        ns9:start.use       "2013-09-03" ;
        ns5:startDate       "2013-09-03"^^<http://www.w3.org/2001/XMLSchema#date> ;
        ns5:status          <http://publications.europa.eu/resource/authority/concept-status/CURRENT> ;
        ns5:xlDefinition    []  ;
        ns5:xlNotation      []  ;
        ns5:xlNotation      []  ;
        ns10:op-code        "GMZ" ;
        dc:identifier       "GMZ" ;
        ns4:created         "2015-04-20"^^<http://www.w3.org/2001/XMLSchema#date> ;
        ns4:dateSubmitted   "2015-04-22"^^<http://www.w3.org/2001/XMLSchema#date> ;
        owl:versionInfo     "20200624-0" ;
        skos:definition     "GMZ is the media type which shall be used for a zip archive that contains one or more GML documents."@en ;
        skos:inScheme       ns10:file-type ;
        skos:prefLabel      "Zipped GML"@en ;
        skos:topConceptOf   ns10:file-type ;
        ns7:altLabel        []  ;
        ns7:prefLabel       []  .

<http://publications.europa.eu/resource/authority/file-type/XML>
        a                    ns5:FileType , skos:Concept ;
        ns6:context          <http://publications.europa.eu/resource/authority/use-context/DCAT_AP> , <http://publications.europa.eu/resource/authority/use-context/CELLAR> , <http://publications.europa.eu/resource/authority/use-context/EUDOR> , <http://publications.europa.eu/resource/authority/use-context/ODP> , <http://publications.europa.eu/resource/authority/use-context/OJEEP> , <http://publications.europa.eu/resource/authority/use-context/IMMC> ;
        ns9:authority-code   "XML" ;
        ns9:deprecated       "false" ;
        ns9:op-code          "XML" ;
        ns9:op-mapped-code   []  ;
        ns9:op-mapped-code   []  ;
        ns9:op-mapped-code   []  ;
        ns9:op-mapped-code   []  ;
        ns9:op-mapped-code   []  ;
        ns9:op-mapped-code   []  ;
        ns9:op-mapped-code   []  ;
        ns9:op-mapped-code   []  ;
        ns9:start.use        "2012-09-01" ;
        ns5:isTextual        true ;
        ns5:machineReadable  true ;
        ns5:nonPropExt       true ;
        ns5:order            5 ;
        ns5:startDate        "2012-09-01"^^<http://www.w3.org/2001/XMLSchema#date> ;
        ns5:status           <http://publications.europa.eu/resource/authority/concept-status/CURRENT> ;
        ns5:xlDefinition     []  ;
        ns5:xlNotation       []  ;
        ns5:xlNotation       []  ;
        ns5:xlNotation       []  ;
        ns5:xlNotation       []  ;
        ns5:xlNotation       []  ;
        ns10:op-code         "XML" ;
        dc:identifier        "XML" ;
        ns4:created          "2012-03-19"^^<http://www.w3.org/2001/XMLSchema#date> ;
        ns4:dateAccepted     "2012-11-27"^^<http://www.w3.org/2001/XMLSchema#date> ;
        ns4:dateSubmitted    "2012-09-27"^^<http://www.w3.org/2001/XMLSchema#date> ;
        owl:versionInfo      "20200624-0" ;
        skos:definition      "XML – Extensible Markup Language – is a markup language that defines a set of rules for encoding documents in a format that is both human-readable and machine-readable. The design goals of XML emphasize simplicity, generality and usability across the Internet."@en ;
        skos:inScheme        ns10:file-type ;
        skos:prefLabel       "XML"@en ;
        skos:topConceptOf    ns10:file-type ;
        ns7:altLabel         []  ;
        ns7:prefLabel        []  .

<http://publications.europa.eu/resource/authority/file-type/XSLFO>
        a                   skos:Concept , ns5:FileType ;
        ns6:context         <http://publications.europa.eu/resource/authority/use-context/IMMC> , <http://publications.europa.eu/resource/authority/use-context/CELLAR> ;
        ns9:authority-code  "XSLFO" ;
        ns9:deprecated      "false" ;
        ns9:op-code         "XSLFO" ;
        ns9:op-mapped-code  []  ;
        ns9:start.use       "2012-09-01" ;
        ns5:startDate       "2012-09-01"^^<http://www.w3.org/2001/XMLSchema#date> ;
        ns5:status          <http://publications.europa.eu/resource/authority/concept-status/CURRENT> ;
        ns5:xlDefinition    []  ;
        ns5:xlNotation      []  ;
        ns5:xlNotation      []  ;
        ns10:op-code        "XSLFO" ;
        dc:identifier       "XSLFO" ;
        ns4:created         "2012-09-01"^^<http://www.w3.org/2001/XMLSchema#date> ;
        ns4:dateAccepted    "2014-03-12"^^<http://www.w3.org/2001/XMLSchema#date> ;
        ns4:dateSubmitted   "2014-02-19"^^<http://www.w3.org/2001/XMLSchema#date> ;
        owl:versionInfo     "20200624-0" ;
        skos:definition     "XSL-FO – XSL Formatting Objects – is a markup language for XML document formatting that is most often used to generate PDF files. XSL-FO is part of XSL (Extensible Stylesheet Language), a set of W3C technologies designed for the transformation and formatting of XML data."@en ;
        skos:inScheme       ns10:file-type ;
        skos:prefLabel      "XSL-FO"@en ;
        skos:topConceptOf   ns10:file-type ;
        ns7:altLabel        []  ;
        ns7:prefLabel       []  .

<http://publications.europa.eu/resource/authority/file-type/XYZ>
        a                   skos:Concept , ns5:FileType ;
        ns6:context         <http://publications.europa.eu/resource/authority/use-context/CELLAR> , <http://publications.europa.eu/resource/authority/use-context/IMMC> , <http://publications.europa.eu/resource/authority/use-context/ODP> ;
        ns9:authority-code  "XYZ" ;
        ns9:deprecated      "false" ;
        ns9:op-code         "XYZ" ;
        ns9:op-mapped-code  []  ;
        ns9:op-mapped-code  []  ;
        ns9:start.use       "2010-10-10" ;
        ns5:startDate       "2010-10-10"^^<http://www.w3.org/2001/XMLSchema#date> ;
        ns5:status          <http://publications.europa.eu/resource/authority/concept-status/CURRENT> ;
        ns5:xlDefinition    []  ;
        ns5:xlNotation      []  ;
        ns5:xlNotation      []  ;
        ns5:xlNotation      []  ;
        ns10:op-code        "XYZ" ;
        dc:identifier       "XYZ" ;
        ns4:created         "2015-04-21"^^<http://www.w3.org/2001/XMLSchema#date> ;
        ns4:dateSubmitted   "2015-04-22"^^<http://www.w3.org/2001/XMLSchema#date> ;
        owl:versionInfo     "20200624-0" ;
        skos:definition     "The XYZ file format is a chemical file format. There is no formal standard and several variations exist, but a typical XYZ format specifies the molecule geometry by giving the number of atoms with Cartesian coordinates that will be read on the first line, a comment on the second, and the lines of atomic coordinates in the following lines."@en ;
        skos:inScheme       ns10:file-type ;
        skos:prefLabel      "XYZ Chemical File"@en ;
        skos:topConceptOf   ns10:file-type ;
        ns7:altLabel        []  ;
        ns7:prefLabel       []  .

<http://publications.europa.eu/resource/authority/file-type/XSLT>
        a                   skos:Concept , ns5:FileType ;
        ns6:context         <http://publications.europa.eu/resource/authority/use-context/IMMC> , <http://publications.europa.eu/resource/authority/use-context/CELLAR> , <http://publications.europa.eu/resource/authority/use-context/ODP> , <http://publications.europa.eu/resource/authority/use-context/DCAT_AP> ;
        ns9:authority-code  "XSLT" ;
        ns9:deprecated      "false" ;
        ns9:op-code         "XSLT" ;
        ns9:op-mapped-code  []  ;
        ns9:op-mapped-code  []  ;
        ns9:op-mapped-code  []  ;
        ns9:op-mapped-code  []  ;
        ns9:op-mapped-code  []  ;
        ns9:op-mapped-code  []  ;
        ns9:op-mapped-code  []  ;
        ns9:start.use       "2012-09-01" ;
        ns5:isTextual       true ;
        ns5:order           40 ;
        ns5:startDate       "2012-09-01"^^<http://www.w3.org/2001/XMLSchema#date> ;
        ns5:status          <http://publications.europa.eu/resource/authority/concept-status/CURRENT> ;
        ns5:xlDefinition    []  ;
        ns5:xlNotation      []  ;
        ns5:xlNotation      []  ;
        ns5:xlNotation      []  ;
        ns5:xlNotation      []  ;
        ns5:xlNotation      []  ;
        ns5:xlNotation      []  ;
        ns10:op-code        "XSLT" ;
        dc:identifier       "XSLT" ;
        ns4:created         "2012-03-19"^^<http://www.w3.org/2001/XMLSchema#date> ;
        ns4:dateAccepted    "2012-11-27"^^<http://www.w3.org/2001/XMLSchema#date> ;
        ns4:dateSubmitted   "2012-09-27"^^<http://www.w3.org/2001/XMLSchema#date> ;
        owl:versionInfo     "20200624-0" ;
        skos:definition     "XSLT – Extensible Stylesheet Language Transformations – is a language for transforming XML documents into other XML documents or other formats such as HTML for web pages, plain text or XSL Formatting Objects, which may subsequently be converted to other formats, such as PDF, PostScript and PNG."@en ;
        skos:inScheme       ns10:file-type ;
        skos:prefLabel      "XSLT"@en ;
        skos:topConceptOf   ns10:file-type ;
        ns7:altLabel        []  ;
        ns7:prefLabel       []  .

<http://publications.europa.eu/resource/authority/file-type/TIFF>
        a                   ns5:FileType , skos:Concept ;
        ns6:context         <http://publications.europa.eu/resource/authority/use-context/IMMC> , <http://publications.europa.eu/resource/authority/use-context/EUDOR> , <http://publications.europa.eu/resource/authority/use-context/OJEEP> , <http://publications.europa.eu/resource/authority/use-context/ODP> , <http://publications.europa.eu/resource/authority/use-context/DCAT_AP> , <http://publications.europa.eu/resource/authority/use-context/CELLAR> ;
        ns9:authority-code  "TIFF" ;
        ns9:deprecated      "false" ;
        ns9:op-code         "TIFF" ;
        ns9:op-mapped-code  []  ;
        ns9:op-mapped-code  []  ;
        ns9:op-mapped-code  []  ;
        ns9:op-mapped-code  []  ;
        ns9:op-mapped-code  []  ;
        ns9:op-mapped-code  []  ;
        ns9:op-mapped-code  []  ;
        ns9:op-mapped-code  []  ;
        ns9:op-mapped-code  []  ;
        ns9:start.use       "2012-09-01" ;
        ns5:isTextual       false ;
        ns5:nonPropExt      true ;
        ns5:order           70 ;
        ns5:startDate       "2012-09-01"^^<http://www.w3.org/2001/XMLSchema#date> ;
        ns5:status          <http://publications.europa.eu/resource/authority/concept-status/CURRENT> ;
        ns5:xlDefinition    []  ;
        ns5:xlNotation      []  ;
        ns5:xlNotation      []  ;
        ns5:xlNotation      []  ;
        ns5:xlNotation      []  ;
        ns5:xlNotation      []  ;
        ns5:xlNotation      []  ;
        ns5:xlNotation      []  ;
        ns10:op-code        "TIFF" ;
        dc:identifier       "TIFF" ;
        ns4:created         "2012-03-19"^^<http://www.w3.org/2001/XMLSchema#date> ;
        ns4:dateAccepted    "2012-11-27"^^<http://www.w3.org/2001/XMLSchema#date> ;
        ns4:dateSubmitted   "2012-09-27"^^<http://www.w3.org/2001/XMLSchema#date> ;
        owl:versionInfo     "20200624-0" ;
        skos:definition     "TIFF – Tagged Image File Format – is a computer file format for storing raster graphics images, popular among graphic artists, the publishing industry and photographers. TIFF is widely supported by scanning, faxing, word processing, optical character recognition, image manipulation, desktop publishing and page-layout applications. The format was created by Aldus Corporation for use in desktop publishing."@en ;
        skos:inScheme       ns10:file-type ;
        skos:prefLabel      "TIFF"@en ;
        skos:topConceptOf   ns10:file-type ;
        ns7:altLabel        []  ;
        ns7:prefLabel       []  .

<http://publications.europa.eu/resource/authority/file-type/PS>
        a                   skos:Concept , ns5:FileType ;
        ns6:context         <http://publications.europa.eu/resource/authority/use-context/CELLAR> , <http://publications.europa.eu/resource/authority/use-context/IMMC> , <http://publications.europa.eu/resource/authority/use-context/OJEEP> ;
        ns9:authority-code  "PS" ;
        ns9:deprecated      "false" ;
        ns9:op-code         "PS" ;
        ns9:op-mapped-code  []  ;
        ns9:start.use       "2012-09-01" ;
        ns5:startDate       "2012-09-01"^^<http://www.w3.org/2001/XMLSchema#date> ;
        ns5:status          <http://publications.europa.eu/resource/authority/concept-status/CURRENT> ;
        ns5:xlDefinition    []  ;
        ns5:xlNotation      []  ;
        ns5:xlNotation      []  ;
        ns10:op-code        "PS" ;
        dc:identifier       "PS" ;
        ns4:created         "2014-03-04"^^<http://www.w3.org/2001/XMLSchema#date> ;
        ns4:dateAccepted    "2014-03-12"^^<http://www.w3.org/2001/XMLSchema#date> ;
        ns4:dateSubmitted   "2014-02-19"^^<http://www.w3.org/2001/XMLSchema#date> ;
        owl:versionInfo     "20200624-0" ;
        skos:definition     "PS – PostScript – is a page description language in the electronic publishing and desktop publishing business. It is a dynamically typed, concatenative programming language."@en ;
        skos:inScheme       ns10:file-type ;
        skos:prefLabel      "PS"@en ;
        skos:topConceptOf   ns10:file-type ;
        ns7:altLabel        []  ;
        ns7:prefLabel       []  .

<http://publications.europa.eu/resource/authority/file-type/PDFA1B>
        a                   ns5:FileType , skos:Concept ;
        ns6:context         <http://publications.europa.eu/resource/authority/use-context/IMMC> , <http://publications.europa.eu/resource/authority/use-context/CELLAR> , <http://publications.europa.eu/resource/authority/use-context/EUDOR> , <http://publications.europa.eu/resource/authority/use-context/PUB> ;
        ns9:authority-code  "PDFA1B" ;
        ns9:deprecated      "false" ;
        ns9:op-code         "PDFA1B" ;
        ns9:op-mapped-code  []  ;
        ns9:op-mapped-code  []  ;
        ns9:op-mapped-code  []  ;
        ns9:op-mapped-code  []  ;
        ns9:op-mapped-code  []  ;
        ns9:op-mapped-code  []  ;
        ns9:start.use       "2012-09-01" ;
        ns5:isTextual       false ;
        ns5:order           260 ;
        ns5:startDate       "2012-09-01"^^<http://www.w3.org/2001/XMLSchema#date> ;
        ns5:status          <http://publications.europa.eu/resource/authority/concept-status/CURRENT> ;
        ns5:xlDefinition    []  ;
        ns5:xlNotation      []  ;
        ns5:xlNotation      []  ;
        ns5:xlNotation      []  ;
        ns5:xlNotation      []  ;
        ns5:xlNotation      []  ;
        ns10:op-code        "PDFA1B" ;
        dc:identifier       "PDFA1B" ;
        ns4:created         "2012-03-19"^^<http://www.w3.org/2001/XMLSchema#date> ;
        ns4:dateAccepted    "2012-11-27"^^<http://www.w3.org/2001/XMLSchema#date> ;
        ns4:dateSubmitted   "2012-09-27"^^<http://www.w3.org/2001/XMLSchema#date> ;
        owl:versionInfo     "20200624-0" ;
        skos:definition     "PDF/A-1 is the Part 1 of the PDF standard and specifies two levels of conformance for PDF files. Level B (basic) conformance requires only that standards necessary for the reliable reproduction of a document's visual appearance be followed."@en ;
        skos:inScheme       ns10:file-type ;
        skos:prefLabel      "PDF/A-1b"@en ;
        skos:topConceptOf   ns10:file-type ;
        ns7:altLabel        []  ;
        ns7:prefLabel       []  .

<http://publications.europa.eu/resource/authority/file-type/BMP>
        a                   skos:Concept , ns5:FileType ;
        ns6:context         <http://publications.europa.eu/resource/authority/use-context/IMMC> , <http://publications.europa.eu/resource/authority/use-context/CELLAR> , <http://publications.europa.eu/resource/authority/use-context/ODP> ;
        ns9:authority-code  "BMP" ;
        ns9:deprecated      "false" ;
        ns9:op-code         "BMP" ;
        ns9:op-mapped-code  []  ;
        ns9:op-mapped-code  []  ;
        ns9:op-mapped-code  []  ;
        ns9:op-mapped-code  []  ;
        ns9:op-mapped-code  []  ;
        ns9:start.use       "1996-04-01" ;
        ns5:nonPropExt      true ;
        ns5:startDate       "1996-04-01"^^<http://www.w3.org/2001/XMLSchema#date> ;
        ns5:status          <http://publications.europa.eu/resource/authority/concept-status/CURRENT> ;
        ns5:xlDefinition    []  ;
        ns5:xlNotation      []  ;
        ns5:xlNotation      []  ;
        ns5:xlNotation      []  ;
        ns5:xlNotation      []  ;
        ns5:xlNotation      []  ;
        ns10:op-code        "BMP" ;
        dc:identifier       "BMP" ;
        ns4:created         "2015-04-21"^^<http://www.w3.org/2001/XMLSchema#date> ;
        ns4:dateSubmitted   "2015-04-22"^^<http://www.w3.org/2001/XMLSchema#date> ;
        owl:versionInfo     "20200624-0" ;
        skos:definition     "The bitmap image (BMP) or device independent bitmap (DIB) is a raster graphics image file format used to store bitmap digital images, independently of the display device."@en ;
        skos:inScheme       ns10:file-type ;
        skos:prefLabel      "Bitmap Image File"@en ;
        skos:topConceptOf   ns10:file-type ;
        ns7:altLabel        []  ;
        ns7:prefLabel       []  .

<http://publications.europa.eu/resource/authority/file-type/KMZ>
        a                    skos:Concept , ns5:FileType ;
        ns6:context          <http://publications.europa.eu/resource/authority/use-context/ODP> , <http://publications.europa.eu/resource/authority/use-context/CELLAR> , <http://publications.europa.eu/resource/authority/use-context/DCAT_AP> , <http://publications.europa.eu/resource/authority/use-context/IMMC> ;
        ns9:authority-code   "KMZ" ;
        ns9:deprecated       "false" ;
        ns9:op-code          "KMZ" ;
        ns9:op-mapped-code   []  ;
        ns9:op-mapped-code   []  ;
        ns9:op-mapped-code   []  ;
        ns9:start.use        "2013-11-27" ;
        ns5:machineReadable  true ;
        ns5:nonPropExt       true ;
        ns5:startDate        "2013-11-27"^^<http://www.w3.org/2001/XMLSchema#date> ;
        ns5:status           <http://publications.europa.eu/resource/authority/concept-status/CURRENT> ;
        ns5:xlDefinition     []  ;
        ns5:xlNotation       []  ;
        ns5:xlNotation       []  ;
        ns10:op-code         "KMZ" ;
        dc:identifier        "KMZ" ;
        ns4:created          "2012-09-01"^^<http://www.w3.org/2001/XMLSchema#date> ;
        ns4:dateAccepted     "2014-03-12"^^<http://www.w3.org/2001/XMLSchema#date> ;
        ns4:dateSubmitted    "2014-02-19"^^<http://www.w3.org/2001/XMLSchema#date> ;
        owl:versionInfo      "20200624-0" ;
        skos:definition      "A KMZ file consists of a main KML file and zero or more supporting files that are packaged using a Zip utility into one unit, called an archive. The KMZ file can then be stored and emailed as a single entity. A NetworkLink can fetch a KMZ file from a web server. When the KMZ file is unzipped, the main .kml file and its supporting files are separated into their original formats and directory structure, with their original filenames and extensions. In addition to being an archive format, the Zip format is also compressed, so an archive can include only a single large KML file. Depending on the content of the KML file, this process typically results in 10:1 compression. Your 10 Kbyte KML file can be served with a 1 Kbyte KMZ file."@en ;
        skos:inScheme        ns10:file-type ;
        skos:prefLabel       "KMZ"@en ;
        skos:topConceptOf    ns10:file-type ;
        ns7:altLabel         []  ;
        ns7:prefLabel        []  .

<http://publications.europa.eu/resource/authority/file-type/PDFX4>
        a                   ns5:FileType , skos:Concept ;
        ns6:context         <http://publications.europa.eu/resource/authority/use-context/IMMC> , <http://publications.europa.eu/resource/authority/use-context/EUDOR> , <http://publications.europa.eu/resource/authority/use-context/CELLAR> ;
        ns9:authority-code  "PDFX4" ;
        ns9:deprecated      "false" ;
        ns9:op-code         "PDFX4" ;
        ns9:op-mapped-code  []  ;
        ns9:op-mapped-code  []  ;
        ns9:op-mapped-code  []  ;
        ns9:op-mapped-code  []  ;
        ns9:op-mapped-code  []  ;
        ns9:op-mapped-code  []  ;
        ns9:start.use       "2008-03-01" ;
        ns5:isTextual       false ;
        ns5:order           241 ;
        ns5:startDate       "2008-03-01"^^<http://www.w3.org/2001/XMLSchema#date> ;
        ns5:status          <http://publications.europa.eu/resource/authority/concept-status/CURRENT> ;
        ns5:xlDefinition    []  ;
        ns5:xlNotation      []  ;
        ns5:xlNotation      []  ;
        ns5:xlNotation      []  ;
        ns5:xlNotation      []  ;
        ns5:xlNotation      []  ;
        ns10:op-code        "PDFX4" ;
        dc:identifier       "PDFX4" ;
        ns4:created         "2017-08-22"^^<http://www.w3.org/2001/XMLSchema#date> ;
        ns4:dateAccepted    "2017-09-05"^^<http://www.w3.org/2001/XMLSchema#date> ;
        ns4:dateSubmitted   "2017-08-22"^^<http://www.w3.org/2001/XMLSchema#date> ;
        owl:versionInfo     "20200624-0" ;
        skos:definition     "PDF/X-4 is a PDF specification in which colour-managed, CMYK, gray, RGB or spot colour data are supported, as are PDF transparency and optional content."@en ;
        skos:inScheme       ns10:file-type ;
        skos:prefLabel      "PDF/X-4"@en ;
        skos:topConceptOf   ns10:file-type ;
        ns7:altLabel        []  ;
        ns7:prefLabel       []  .

<http://publications.europa.eu/resource/authority/file-type/CSS>
        a                   ns5:FileType , skos:Concept ;
        ns6:context         <http://publications.europa.eu/resource/authority/use-context/CELLAR> , <http://publications.europa.eu/resource/authority/use-context/ODP> , <http://publications.europa.eu/resource/authority/use-context/IMMC> , <http://publications.europa.eu/resource/authority/use-context/DCAT_AP> ;
        ns9:authority-code  "CSS" ;
        ns9:deprecated      "false" ;
        ns9:op-code         "CSS" ;
        ns9:op-mapped-code  []  ;
        ns9:op-mapped-code  []  ;
        ns9:op-mapped-code  []  ;
        ns9:op-mapped-code  []  ;
        ns9:op-mapped-code  []  ;
        ns9:start.use       "2012-09-01" ;
        ns5:isTextual       true ;
        ns5:order           7 ;
        ns5:startDate       "2012-09-01"^^<http://www.w3.org/2001/XMLSchema#date> ;
        ns5:status          <http://publications.europa.eu/resource/authority/concept-status/CURRENT> ;
        ns5:xlDefinition    []  ;
        ns5:xlNotation      []  ;
        ns5:xlNotation      []  ;
        ns5:xlNotation      []  ;
        ns5:xlNotation      []  ;
        ns10:op-code        "CSS" ;
        dc:identifier       "CSS" ;
        ns4:created         "2012-09-01"^^<http://www.w3.org/2001/XMLSchema#date> ;
        ns4:dateAccepted    "2014-03-12"^^<http://www.w3.org/2001/XMLSchema#date> ;
        ns4:dateSubmitted   "2014-02-19"^^<http://www.w3.org/2001/XMLSchema#date> ;
        owl:versionInfo     "20200624-0" ;
        skos:definition     "CSS – Cascading Style Sheets – is a style sheet language used for describing the presentation of a document written in a markup language."@en ;
        skos:inScheme       ns10:file-type ;
        skos:prefLabel      "CSS"@en ;
        skos:topConceptOf   ns10:file-type ;
        ns7:altLabel        []  ;
        ns7:prefLabel       []  .

<http://publications.europa.eu/resource/authority/file-type/ODP>
        a                   skos:Concept , ns5:FileType ;
        ns6:context         <http://publications.europa.eu/resource/authority/use-context/IMMC> ;
        ns9:authority-code  "ODP" ;
        ns9:deprecated      "false" ;
        ns9:op-code         "ODP" ;
        ns9:op-mapped-code  []  ;
        ns9:op-mapped-code  []  ;
        ns9:start.use       "2005-05-01" ;
        ns5:startDate       "2005-05-01"^^<http://www.w3.org/2001/XMLSchema#date> ;
        ns5:status          <http://publications.europa.eu/resource/authority/concept-status/CURRENT> ;
        ns5:xlDefinition    []  ;
        ns5:xlNotation      []  ;
        ns5:xlNotation      []  ;
        ns5:xlNotation      []  ;
        ns10:op-code        "ODP" ;
        dc:identifier       "ODP" ;
        ns4:created         "2020-05-12"^^<http://www.w3.org/2001/XMLSchema#date> ;
        ns4:dateAccepted    "2020-06-04"^^<http://www.w3.org/2001/XMLSchema#date> ;
        ns4:dateSubmitted   "2020-05-19"^^<http://www.w3.org/2001/XMLSchema#date> ;
        owl:versionInfo     "20200624-0" ;
        skos:definition     "ODP is an OpenDocument file format for presentations. OpenDocument was developed with the aim of providing an open, XML-based file format specification for office applications."@en ;
        skos:inScheme       ns10:file-type ;
        skos:prefLabel      "ODP"@en ;
        skos:topConceptOf   ns10:file-type ;
        ns7:altLabel        []  ;
        ns7:prefLabel       []  .

<http://publications.europa.eu/resource/authority/file-type/XLSX>
        a                    ns5:FileType , skos:Concept ;
        ns6:context          <http://publications.europa.eu/resource/authority/use-context/CELLAR> , <http://publications.europa.eu/resource/authority/use-context/ODP> , <http://publications.europa.eu/resource/authority/use-context/IMMC> , <http://publications.europa.eu/resource/authority/use-context/DCAT_AP> , <http://publications.europa.eu/resource/authority/use-context/OJEEP> ;
        ns9:authority-code   "XLSX" ;
        ns9:deprecated       "false" ;
        ns9:op-code          "XLSX" ;
        ns9:op-mapped-code   []  ;
        ns9:op-mapped-code   []  ;
        ns9:op-mapped-code   []  ;
        ns9:op-mapped-code   []  ;
        ns9:op-mapped-code   []  ;
        ns9:op-mapped-code   []  ;
        ns9:op-mapped-code   []  ;
        ns9:start.use        "2012-09-01" ;
        ns5:isTextual        false ;
        ns5:machineReadable  true ;
        ns5:order            50 ;
        ns5:startDate        "2012-09-01"^^<http://www.w3.org/2001/XMLSchema#date> ;
        ns5:status           <http://publications.europa.eu/resource/authority/concept-status/CURRENT> ;
        ns5:xlDefinition     []  ;
        ns5:xlNotation       []  ;
        ns5:xlNotation       []  ;
        ns5:xlNotation       []  ;
        ns5:xlNotation       []  ;
        ns5:xlNotation       []  ;
        ns10:op-code         "XLSX" ;
        dc:identifier        "XLSX" ;
        ns4:created          "2012-03-19"^^<http://www.w3.org/2001/XMLSchema#date> ;
        ns4:dateAccepted     "2012-11-27"^^<http://www.w3.org/2001/XMLSchema#date> ;
        ns4:dateSubmitted    "2012-09-27"^^<http://www.w3.org/2001/XMLSchema#date> ;
        owl:versionInfo      "20200624-0" ;
        skos:definition      "XLSX is the default file format for Excel 2007 and later workbook used for Microsoft Excel spreadsheet which features calculation, graphing tools, pivot tables and a macro programming language. XLSX is in reality a ZIP compressed archive with a directory structure of XML text documents."@en ;
        skos:inScheme        ns10:file-type ;
        skos:prefLabel       "Excel XLSX"@en ;
        skos:topConceptOf    ns10:file-type ;
        ns7:altLabel         []  ;
        ns7:prefLabel        []  .

<http://publications.europa.eu/resource/authority/file-type/BIN>
        a                   ns5:FileType , skos:Concept ;
        ns6:context         <http://publications.europa.eu/resource/authority/use-context/IMMC> , <http://publications.europa.eu/resource/authority/use-context/CELLAR> , <http://publications.europa.eu/resource/authority/use-context/ODP> ;
        ns9:authority-code  "BIN" ;
        ns9:deprecated      "false" ;
        ns9:op-code         "BIN" ;
        ns9:op-mapped-code  []  ;
        ns9:op-mapped-code  []  ;
        ns9:start.use       "1996-11-01" ;
        ns5:startDate       "1996-11-01"^^<http://www.w3.org/2001/XMLSchema#date> ;
        ns5:status          <http://publications.europa.eu/resource/authority/concept-status/CURRENT> ;
        ns5:xlDefinition    []  ;
        ns5:xlNotation      []  ;
        ns5:xlNotation      []  ;
        ns5:xlNotation      []  ;
        ns10:op-code        "BIN" ;
        dc:identifier       "BIN" ;
        ns4:created         "2015-04-21"^^<http://www.w3.org/2001/XMLSchema#date> ;
        ns4:dateSubmitted   "2015-04-22"^^<http://www.w3.org/2001/XMLSchema#date> ;
        owl:versionInfo     "20200624-0" ;
        skos:definition     "A binary file is a computer file that is not a text file."@en ;
        skos:inScheme       ns10:file-type ;
        skos:prefLabel      "Binary Data"@en ;
        skos:topConceptOf   ns10:file-type ;
        ns7:altLabel        []  ;
        ns7:prefLabel       []  .

ns10:file-type  a                 owl:Ontology , skos:ConceptScheme ;
        rdfs:comment              "File type"^^rdfs:Literal ;
        rdfs:label                "File type"@en ;
        ns9:prefLabel             "File type"@en ;
        ns9:table.id              "file-type" ;
        ns9:table.version.number  "20200624-0" ;
        ns4:identifier            "http://publications.europa.eu/resource/authority/file-type" ;
        owl:imports               <http://publications.europa.eu/ontology/euvoc> ;
        owl:versionIRI            <http://publications.europa.eu/resource/authority/file-type/20200624-0> ;
        owl:versionInfo           "20200624-0" ;
        skos:prefLabel            "File type"@en ;
        ns7:prefLabel             []  ;
        ns7:prefLabel             []  .

<http://publications.europa.eu/resource/authority/file-type/GRID_ASCII>
        a                   skos:Concept , ns5:FileType ;
        ns6:context         <http://publications.europa.eu/resource/authority/use-context/IMMC> , <http://publications.europa.eu/resource/authority/use-context/ODP> , <http://publications.europa.eu/resource/authority/use-context/CELLAR> ;
        ns9:authority-code  "GRID_ASCII" ;
        ns9:deprecated      "false" ;
        ns9:op-code         "GRID_ASCII" ;
        ns9:op-mapped-code  []  ;
        ns9:start.use       "2013-08-21" ;
        ns5:startDate       "2013-08-21"^^<http://www.w3.org/2001/XMLSchema#date> ;
        ns5:status          <http://publications.europa.eu/resource/authority/concept-status/CURRENT> ;
        ns5:xlDefinition    []  ;
        ns5:xlNotation      []  ;
        ns5:xlNotation      []  ;
        ns10:op-code        "GRID_ASCII" ;
        dc:identifier       "GRID_ASCII" ;
        ns4:created         "2015-04-20"^^<http://www.w3.org/2001/XMLSchema#date> ;
        ns4:dateSubmitted   "2015-04-22"^^<http://www.w3.org/2001/XMLSchema#date> ;
        owl:versionInfo     "20200624-0" ;
        skos:definition     "Esri ASCII grid is the media type which shall be used for ASCII GRID files. ASCII GRID is one of the two formats of Esri grid, a raster GIS file format, a non-proprietary ASCII format, also known as an ArcInfo ASCII GRID."@en ;
        skos:inScheme       ns10:file-type ;
        skos:prefLabel      "Esri ASCII grid"@en ;
        skos:topConceptOf   ns10:file-type ;
        ns7:altLabel        []  ;
        ns7:prefLabel       []  .

<http://publications.europa.eu/resource/authority/file-type/BITS>
        a                   skos:Concept , ns5:FileType ;
        ns6:context         <http://publications.europa.eu/resource/authority/use-context/IMMC> , <http://publications.europa.eu/resource/authority/use-context/CELLAR> ;
        ns9:authority-code  "BITS" ;
        ns9:deprecated      "false" ;
        ns9:op-code         "BITS" ;
        ns9:op-mapped-code  []  ;
        ns9:start.use       "2012-08-22" ;
        ns5:startDate       "2012-08-22"^^<http://www.w3.org/2001/XMLSchema#date> ;
        ns5:status          <http://publications.europa.eu/resource/authority/concept-status/CURRENT> ;
        ns5:xlDefinition    []  ;
        ns5:xlNotation      []  ;
        ns5:xlNotation      []  ;
        ns10:op-code        "BITS" ;
        dc:identifier       "BITS" ;
        ns4:created         "2018-01-05"^^<http://www.w3.org/2001/XMLSchema#date> ;
        ns4:dateAccepted    "2018-03-06"^^<http://www.w3.org/2001/XMLSchema#date> ;
        ns4:dateSubmitted   "2018-02-20"^^<http://www.w3.org/2001/XMLSchema#date> ;
        owl:versionInfo     "20200624-0" ;
        skos:definition     "BITS – Book Interchange Tag Suite – is the ‘book version’ of Journal Article Tag Suite (JATS); an XML format used to describe books published online. BITS provides a common XML format in which publishers and archivists can describe textual and graphical content elements. In order to facilitate the reusability, BITS makes a tag set adequate for supporting interchange, archiving, format-conversion and publishing."@en ;
        skos:inScheme       ns10:file-type ;
        skos:prefLabel      "BITS XML"@en ;
        skos:topConceptOf   ns10:file-type ;
        ns7:altLabel        []  ;
        ns7:prefLabel       []  .

<http://publications.europa.eu/resource/authority/file-type/DMP>
        a                   ns5:FileType , skos:Concept ;
        ns6:context         <http://publications.europa.eu/resource/authority/use-context/CELLAR> , <http://publications.europa.eu/resource/authority/use-context/IMMC> ;
        ns9:authority-code  "DMP" ;
        ns9:deprecated      "false" ;
        ns9:op-code         "DMP" ;
        ns9:op-mapped-code  []  ;
        ns9:start.use       "2004-01-01" ;
        ns5:startDate       "2004-01-01"^^<http://www.w3.org/2001/XMLSchema#date> ;
        ns5:status          <http://publications.europa.eu/resource/authority/concept-status/CURRENT> ;
        ns5:xlDefinition    []  ;
        ns5:xlNotation      []  ;
        ns5:xlNotation      []  ;
        ns10:op-code        "DMP" ;
        dc:identifier       "DMP" ;
        ns4:created         "2015-04-20"^^<http://www.w3.org/2001/XMLSchema#date> ;
        ns4:dateSubmitted   "2015-04-22"^^<http://www.w3.org/2001/XMLSchema#date> ;
        owl:versionInfo     "20200624-0" ;
        skos:definition     "DMP is the media type which shall be used for Oracle dumps. This media type is incomplete as it lacks a reference to the specification of the format."@en ;
        skos:inScheme       ns10:file-type ;
        skos:prefLabel      "Oracle Dump"@en ;
        skos:topConceptOf   ns10:file-type ;
        ns7:altLabel        []  ;
        ns7:prefLabel       []  .

<http://publications.europa.eu/resource/authority/file-type/XHTML_SIMPL>
        a                   skos:Concept , ns5:FileType ;
        ns6:context         <http://publications.europa.eu/resource/authority/use-context/IMMC> , <http://publications.europa.eu/resource/authority/use-context/CELLAR> ;
        ns9:authority-code  "XHTML_SIMPL" ;
        ns9:deprecated      "false" ;
        ns9:op-code         "XHTML_SIMPL" ;
        ns9:op-mapped-code  []  ;
        ns9:op-mapped-code  []  ;
        ns9:op-mapped-code  []  ;
        ns9:op-mapped-code  []  ;
        ns9:op-mapped-code  []  ;
        ns9:op-mapped-code  []  ;
        ns9:op-mapped-code  []  ;
        ns9:op-mapped-code  []  ;
        ns9:op-mapped-code  []  ;
        ns9:start.use       "2012-09-01" ;
        ns5:isTextual       true ;
        ns5:order           350 ;
        ns5:startDate       "2012-09-01"^^<http://www.w3.org/2001/XMLSchema#date> ;
        ns5:status          <http://publications.europa.eu/resource/authority/concept-status/CURRENT> ;
        ns5:xlDefinition    []  ;
        ns5:xlNotation      []  ;
        ns5:xlNotation      []  ;
        ns5:xlNotation      []  ;
        ns5:xlNotation      []  ;
        ns5:xlNotation      []  ;
        ns5:xlNotation      []  ;
        ns5:xlNotation      []  ;
        ns5:xlNotation      []  ;
        ns10:op-code        "XHTML_SIMPL" ;
        dc:identifier       "XHTML_SIMPL" ;
        ns4:created         "2016-05-12"^^<http://www.w3.org/2001/XMLSchema#date> ;
        ns4:dateAccepted    "2016-06-01"^^<http://www.w3.org/2001/XMLSchema#date> ;
        ns4:dateSubmitted   "2016-05-18"^^<http://www.w3.org/2001/XMLSchema#date> ;
        owl:versionInfo     "20200624-0" ;
        skos:definition     "XHTML is HTML written as XML. Its simplified version is used for storage in the Publications Office."@en ;
        skos:inScheme       ns10:file-type ;
        skos:prefLabel      "XHTML simplified"@en ;
        skos:topConceptOf   ns10:file-type ;
        ns7:altLabel        []  ;
        ns7:prefLabel       []  .

<http://publications.europa.eu/resource/authority/file-type/HDF>
        a                   skos:Concept , ns5:FileType ;
        ns6:context         <http://publications.europa.eu/resource/authority/use-context/IMMC> , <http://publications.europa.eu/resource/authority/use-context/CELLAR> ;
        ns9:authority-code  "HDF" ;
        ns9:deprecated      "false" ;
        ns9:op-code         "HDF" ;
        ns9:op-mapped-code  []  ;
        ns9:op-mapped-code  []  ;
        ns9:op-mapped-code  []  ;
        ns9:op-mapped-code  []  ;
        ns9:op-mapped-code  []  ;
        ns9:op-mapped-code  []  ;
        ns9:op-mapped-code  []  ;
        ns9:op-mapped-code  []  ;
        ns9:start.use       "1990-01-01" ;
        ns5:startDate       "1990-01-01"^^<http://www.w3.org/2001/XMLSchema#date> ;
        ns5:status          <http://publications.europa.eu/resource/authority/concept-status/CURRENT> ;
        ns5:xlDefinition    []  ;
        ns5:xlNotation      []  ;
        ns5:xlNotation      []  ;
        ns5:xlNotation      []  ;
        ns5:xlNotation      []  ;
        ns5:xlNotation      []  ;
        ns5:xlNotation      []  ;
        ns5:xlNotation      []  ;
        ns5:xlNotation      []  ;
        ns5:xlNotation      []  ;
        ns10:op-code        "HDF" ;
        dc:identifier       "HDF" ;
        ns4:created         "2015-04-07"^^<http://www.w3.org/2001/XMLSchema#date> ;
        ns4:dateSubmitted   "2015-04-22"^^<http://www.w3.org/2001/XMLSchema#date> ;
        owl:versionInfo     "20200624-0" ;
        skos:definition     "HDF is a set of file formats (HDF4, HDF5) designed to store and organize large amounts of numerical data."@en ;
        skos:inScheme       ns10:file-type ;
        skos:prefLabel      "HDF"@en ;
        skos:topConceptOf   ns10:file-type ;
        ns7:altLabel        []  ;
        ns7:prefLabel       []  .

<http://publications.europa.eu/resource/authority/file-type/PDFA3>
        a                   ns5:FileType , skos:Concept ;
        ns6:context         <http://publications.europa.eu/resource/authority/use-context/IMMC> ;
        ns9:authority-code  "PDFA3" ;
        ns9:deprecated      "false" ;
        ns9:op-code         "PDFA3" ;
        ns9:op-mapped-code  []  ;
        ns9:op-mapped-code  []  ;
        ns9:op-mapped-code  []  ;
        ns9:op-mapped-code  []  ;
        ns9:op-mapped-code  []  ;
        ns9:op-mapped-code  []  ;
        ns9:start.use       "2012-12-15" ;
        ns5:isTextual       false ;
        ns5:order           244 ;
        ns5:startDate       "2012-12-15"^^<http://www.w3.org/2001/XMLSchema#date> ;
        ns5:status          <http://publications.europa.eu/resource/authority/concept-status/CURRENT> ;
        ns5:xlDefinition    []  ;
        ns5:xlNotation      []  ;
        ns5:xlNotation      []  ;
        ns5:xlNotation      []  ;
        ns5:xlNotation      []  ;
        ns5:xlNotation      []  ;
        ns10:op-code        "PDFA3" ;
        dc:identifier       "PDFA3" ;
        ns4:created         "2016-08-18"^^<http://www.w3.org/2001/XMLSchema#date> ;
        ns4:dateAccepted    "2016-09-09"^^<http://www.w3.org/2001/XMLSchema#date> ;
        ns4:dateSubmitted   "2016-08-22"^^<http://www.w3.org/2001/XMLSchema#date> ;
        owl:versionInfo     "20200624-0" ;
        skos:definition     "PDFA-3 is the Part 3 of the standard which differs from PDF/A-2 in only one regard – it allows embedding of arbitrary file formats (such as XML, CSV, CAD, word-processing documents, spreadsheet documents and others) into PDF/A conforming documents."@en ;
        skos:inScheme       ns10:file-type ;
        skos:prefLabel      "PDFA-3"@en ;
        skos:topConceptOf   ns10:file-type ;
        ns7:altLabel        []  ;
        ns7:prefLabel       []  .

<http://publications.europa.eu/resource/authority/file-type/ODC>
        a                   ns5:FileType , skos:Concept ;
        ns6:context         <http://publications.europa.eu/resource/authority/use-context/IMMC> , <http://publications.europa.eu/resource/authority/use-context/CELLAR> , <http://publications.europa.eu/resource/authority/use-context/ODP> ;
        ns9:authority-code  "ODC" ;
        ns9:deprecated      "false" ;
        ns9:op-code         "ODC" ;
        ns9:op-mapped-code  []  ;
        ns9:start.use       "2005-05-01" ;
        ns5:startDate       "2005-05-01"^^<http://www.w3.org/2001/XMLSchema#date> ;
        ns5:status          <http://publications.europa.eu/resource/authority/concept-status/CURRENT> ;
        ns5:xlDefinition    []  ;
        ns5:xlNotation      []  ;
        ns5:xlNotation      []  ;
        ns10:op-code        "ODC" ;
        dc:identifier       "ODC" ;
        ns4:created         "2015-04-21"^^<http://www.w3.org/2001/XMLSchema#date> ;
        ns4:dateSubmitted   "2015-04-22"^^<http://www.w3.org/2001/XMLSchema#date> ;
        owl:versionInfo     "20200624-0" ;
        skos:definition     "OpenDocument is a standardized Open Document Format for Office Applications. Charts define how to create graphical displays from numerical data."@en ;
        skos:inScheme       ns10:file-type ;
        skos:prefLabel      "OpenDocument Chart"@en ;
        skos:topConceptOf   ns10:file-type ;
        ns7:altLabel        []  ;
        ns7:prefLabel       []  .

<http://publications.europa.eu/resource/authority/file-type/SQL>
        a                   ns5:FileType , skos:Concept ;
        ns6:context         <http://publications.europa.eu/resource/authority/use-context/IMMC> ;
        ns9:authority-code  "SQL" ;
        ns9:deprecated      "false" ;
        ns9:op-code         "SQL" ;
        ns9:op-mapped-code  []  ;
        ns9:start.use       "1974-01-01" ;
        ns5:startDate       "1974-01-01"^^<http://www.w3.org/2001/XMLSchema#date> ;
        ns5:status          <http://publications.europa.eu/resource/authority/concept-status/CURRENT> ;
        ns5:xlDefinition    []  ;
        ns5:xlNotation      []  ;
        ns5:xlNotation      []  ;
        ns10:op-code        "SQL" ;
        dc:identifier       "SQL" ;
        ns4:created         "2016-08-18"^^<http://www.w3.org/2001/XMLSchema#date> ;
        ns4:dateAccepted    "2016-09-09"^^<http://www.w3.org/2001/XMLSchema#date> ;
        ns4:dateSubmitted   "2016-08-22"^^<http://www.w3.org/2001/XMLSchema#date> ;
        owl:versionInfo     "20200624-0" ;
        skos:definition     "SQL – Structured Query Language – is a domain-specific language used in programming and designed for managing data held in a relational database management system (RDBMS) or for stream processing in a relational data stream management system (RDSMS)."@en ;
        skos:inScheme       ns10:file-type ;
        skos:prefLabel      "SQL"@en ;
        skos:topConceptOf   ns10:file-type ;
        ns7:altLabel        []  ;
        ns7:prefLabel       []  .

<http://publications.europa.eu/resource/authority/file-type/ARC>
        a                   ns5:FileType , skos:Concept ;
        ns6:context         <http://publications.europa.eu/resource/authority/use-context/IMMC> , <http://publications.europa.eu/resource/authority/use-context/ODP> , <http://publications.europa.eu/resource/authority/use-context/CELLAR> ;
        ns9:authority-code  "ARC" ;
        ns9:deprecated      "false" ;
        ns9:op-code         "ARC" ;
        ns9:op-mapped-code  []  ;
        ns9:start.use       "1996-05-12" ;
        ns5:startDate       "1996-05-12"^^<http://www.w3.org/2001/XMLSchema#date> ;
        ns5:status          <http://publications.europa.eu/resource/authority/concept-status/CURRENT> ;
        ns5:xlDefinition    []  ;
        ns5:xlNotation      []  ;
        ns5:xlNotation      []  ;
        ns10:op-code        "ARC" ;
        dc:identifier       "ARC" ;
        ns4:created         "2016-02-10"^^<http://www.w3.org/2001/XMLSchema#date> ;
        ns4:dateAccepted    "2016-03-02"^^<http://www.w3.org/2001/XMLSchema#date> ;
        ns4:dateSubmitted   "2016-02-16"^^<http://www.w3.org/2001/XMLSchema#date> ;
        owl:versionInfo     "20200624-0" ;
        skos:definition     "ARC is the archive file format of Internet Archive. ARC files are large aggregate files."@en ;
        skos:inScheme       ns10:file-type ;
        skos:prefLabel      "ARC"@en ;
        skos:topConceptOf   ns10:file-type ;
        ns7:altLabel        []  ;
        ns7:prefLabel       []  .

<http://publications.europa.eu/resource/authority/file-type/IMMC_XML>
        a                   skos:Concept , ns5:FileType ;
        ns6:context         <http://publications.europa.eu/resource/authority/use-context/IMMC> , <http://publications.europa.eu/resource/authority/use-context/CELLAR> , <http://publications.europa.eu/resource/authority/use-context/EUDOR> ;
        ns9:authority-code  "IMMC_XML" ;
        ns9:deprecated      "false" ;
        ns9:op-code         "IMMC_XML" ;
        ns9:op-mapped-code  []  ;
        ns9:op-mapped-code  []  ;
        ns9:op-mapped-code  []  ;
        ns9:op-mapped-code  []  ;
        ns9:op-mapped-code  []  ;
        ns9:start.use       "2016-04-08" ;
        ns5:isTextual       true ;
        ns5:startDate       "2016-04-08"^^<http://www.w3.org/2001/XMLSchema#date> ;
        ns5:status          <http://publications.europa.eu/resource/authority/concept-status/CURRENT> ;
        ns5:xlDefinition    []  ;
        ns5:xlNotation      []  ;
        ns5:xlNotation      []  ;
        ns5:xlNotation      []  ;
        ns5:xlNotation      []  ;
        ns5:xlNotation      []  ;
        ns10:op-code        "IMMC_XML" ;
        dc:identifier       "IMMC_XML" ;
        ns4:created         "2019-07-11"^^<http://www.w3.org/2001/XMLSchema#date> ;
        ns4:dateAccepted    "2019-08-27"^^<http://www.w3.org/2001/XMLSchema#date> ;
        ns4:dateSubmitted   "2019-08-13"^^<http://www.w3.org/2001/XMLSchema#date> ;
        owl:versionInfo     "20200624-0" ;
        skos:definition     "Files exchanged within the context of the Interinstitutional Metadata Maintenance Committee (IMMC) communication protocol."@en ;
        skos:inScheme       ns10:file-type ;
        skos:prefLabel      "IMMC XML message"@en ;
        skos:topConceptOf   ns10:file-type ;
        ns7:altLabel        []  ;
        ns7:prefLabel       []  .

<http://publications.europa.eu/resource/authority/file-type/GIF>
        a                   skos:Concept , ns5:FileType ;
        ns6:context         <http://publications.europa.eu/resource/authority/use-context/CELLAR> , <http://publications.europa.eu/resource/authority/use-context/OJEEP> , <http://publications.europa.eu/resource/authority/use-context/ODP> , <http://publications.europa.eu/resource/authority/use-context/IMMC> ;
        ns9:authority-code  "GIF" ;
        ns9:deprecated      "false" ;
        ns9:op-code         "GIF" ;
        ns9:op-mapped-code  []  ;
        ns9:op-mapped-code  []  ;
        ns9:op-mapped-code  []  ;
        ns9:op-mapped-code  []  ;
        ns9:op-mapped-code  []  ;
        ns9:op-mapped-code  []  ;
        ns9:start.use       "2012-09-01" ;
        ns5:isTextual       false ;
        ns5:order           20 ;
        ns5:startDate       "2012-09-01"^^<http://www.w3.org/2001/XMLSchema#date> ;
        ns5:status          <http://publications.europa.eu/resource/authority/concept-status/CURRENT> ;
        ns5:xlDefinition    []  ;
        ns5:xlNotation      []  ;
        ns5:xlNotation      []  ;
        ns5:xlNotation      []  ;
        ns5:xlNotation      []  ;
        ns5:xlNotation      []  ;
        ns10:op-code        "GIF" ;
        dc:identifier       "GIF" ;
        ns4:created         "2012-03-19"^^<http://www.w3.org/2001/XMLSchema#date> ;
        ns4:dateAccepted    "2012-11-27"^^<http://www.w3.org/2001/XMLSchema#date> ;
        ns4:dateSubmitted   "2012-09-27"^^<http://www.w3.org/2001/XMLSchema#date> ;
        owl:versionInfo     "20200624-0" ;
        skos:definition     "GIF – Graphics Interchange Format – is a bitmap image format that was developed by a team at the bulletin board service (BBS) provider CompuServe."@en ;
        skos:inScheme       ns10:file-type ;
        skos:prefLabel      "GIF"@en ;
        skos:topConceptOf   ns10:file-type ;
        ns7:altLabel        []  ;
        ns7:prefLabel       []  .

<http://publications.europa.eu/resource/authority/file-type/WIM>
        a                   ns5:FileType , skos:Concept ;
        ns6:context         <http://publications.europa.eu/resource/authority/use-context/DCAT_AP> , <http://publications.europa.eu/resource/authority/use-context/IMMC> ;
        ns9:authority-code  "WIM" ;
        ns9:deprecated      "false" ;
        ns9:op-code         "WIM" ;
        ns9:op-mapped-code  []  ;
        ns9:start.use       "2007-01-30" ;
        ns5:startDate       "2007-01-30"^^<http://www.w3.org/2001/XMLSchema#date> ;
        ns5:status          <http://publications.europa.eu/resource/authority/concept-status/CURRENT> ;
        ns5:xlDefinition    []  ;
        ns5:xlNotation      []  ;
        ns5:xlNotation      []  ;
        ns10:op-code        "WIM" ;
        dc:identifier       "WIM" ;
        ns4:created         "2020-05-15"^^<http://www.w3.org/2001/XMLSchema#date> ;
        ns4:dateAccepted    "2020-06-04"^^<http://www.w3.org/2001/XMLSchema#date> ;
        ns4:dateSubmitted   "2020-05-19"^^<http://www.w3.org/2001/XMLSchema#date> ;
        owl:versionInfo     "20200624-0" ;
        skos:definition     "The Windows Imaging Format (WIM) is a file-based disk image format."@en ;
        skos:inScheme       ns10:file-type ;
        skos:prefLabel      "WIM"@en ;
        skos:topConceptOf   ns10:file-type ;
        ns7:altLabel        []  ;
        ns7:prefLabel       []  .

<http://publications.europa.eu/resource/authority/file-type/INDD>
        a                   skos:Concept , ns5:FileType ;
        ns6:context         <http://publications.europa.eu/resource/authority/use-context/IMMC> , <http://publications.europa.eu/resource/authority/use-context/CELLAR> , <http://publications.europa.eu/resource/authority/use-context/OJEEP> ;
        ns9:authority-code  "INDD" ;
        ns9:deprecated      "false" ;
        ns9:op-code         "INDD" ;
        ns9:op-mapped-code  []  ;
        ns9:start.use       "2012-09-01" ;
        ns5:startDate       "2012-09-01"^^<http://www.w3.org/2001/XMLSchema#date> ;
        ns5:status          <http://publications.europa.eu/resource/authority/concept-status/CURRENT> ;
        ns5:xlDefinition    []  ;
        ns5:xlNotation      []  ;
        ns5:xlNotation      []  ;
        ns10:op-code        "INDD" ;
        dc:identifier       "INDD" ;
        ns4:created         "2014-03-03"^^<http://www.w3.org/2001/XMLSchema#date> ;
        ns4:dateAccepted    "2014-03-12"^^<http://www.w3.org/2001/XMLSchema#date> ;
        ns4:dateSubmitted   "2014-02-19"^^<http://www.w3.org/2001/XMLSchema#date> ;
        owl:versionInfo     "20200624-0" ;
        skos:definition     "INDD is a file format for a page layout file used by Adobe InDesign. InDesign is a desktop publishing software application."@en ;
        skos:inScheme       ns10:file-type ;
        skos:prefLabel      "INDD"@en ;
        skos:topConceptOf   ns10:file-type ;
        ns7:altLabel        []  ;
        ns7:prefLabel       []  .

<http://publications.europa.eu/resource/authority/file-type/JATS>
        a                   ns5:FileType , skos:Concept ;
        ns6:context         <http://publications.europa.eu/resource/authority/use-context/IMMC> ;
        ns9:authority-code  "JATS" ;
        ns9:deprecated      "false" ;
        ns9:op-code         "JATS" ;
        ns9:op-mapped-code  []  ;
        ns9:start.use       "2003-03-31" ;
        ns5:startDate       "2003-03-31"^^<http://www.w3.org/2001/XMLSchema#date> ;
        ns5:status          <http://publications.europa.eu/resource/authority/concept-status/CURRENT> ;
        ns5:xlDefinition    []  ;
        ns5:xlNotation      []  ;
        ns5:xlNotation      []  ;
        ns10:op-code        "JATS" ;
        dc:identifier       "JATS" ;
        ns4:created         "2018-01-05"^^<http://www.w3.org/2001/XMLSchema#date> ;
        ns4:dateAccepted    "2018-03-06"^^<http://www.w3.org/2001/XMLSchema#date> ;
        ns4:dateSubmitted   "2018-02-20"^^<http://www.w3.org/2001/XMLSchema#date> ;
        owl:versionInfo     "20200624-0" ;
        skos:definition     "JATS – Journal Article Tag Suite – is an XML format used to describe scientific literature published online. It is a technical standard developed by the National Information Standards Organization (NISO)."@en ;
        skos:inScheme       ns10:file-type ;
        skos:prefLabel      "JATS XML"@en ;
        skos:topConceptOf   ns10:file-type ;
        ns7:altLabel        []  ;
        ns7:prefLabel       []  .

<http://publications.europa.eu/resource/authority/file-type/PDFX1A>
        a                   ns5:FileType , skos:Concept ;
        ns6:context         <http://publications.europa.eu/resource/authority/use-context/CELLAR> , <http://publications.europa.eu/resource/authority/use-context/EUDOR> , <http://publications.europa.eu/resource/authority/use-context/IMMC> ;
        ns9:authority-code  "PDFX1A" ;
        ns9:deprecated      "false" ;
        ns9:op-code         "PDFX1A" ;
        ns9:op-mapped-code  []  ;
        ns9:op-mapped-code  []  ;
        ns9:op-mapped-code  []  ;
        ns9:op-mapped-code  []  ;
        ns9:op-mapped-code  []  ;
        ns9:op-mapped-code  []  ;
        ns9:start.use       "2001-12-01" ;
        ns5:isTextual       false ;
        ns5:order           243 ;
        ns5:startDate       "2001-12-01"^^<http://www.w3.org/2001/XMLSchema#date> ;
        ns5:status          <http://publications.europa.eu/resource/authority/concept-status/CURRENT> ;
        ns5:xlDefinition    []  ;
        ns5:xlNotation      []  ;
        ns5:xlNotation      []  ;
        ns5:xlNotation      []  ;
        ns5:xlNotation      []  ;
        ns5:xlNotation      []  ;
        ns10:op-code        "PDFX1A" ;
        dc:identifier       "PDFX1A" ;
        ns4:created         "2017-08-22"^^<http://www.w3.org/2001/XMLSchema#date> ;
        ns4:dateAccepted    "2017-09-05"^^<http://www.w3.org/2001/XMLSchema#date> ;
        ns4:dateSubmitted   "2017-08-22"^^<http://www.w3.org/2001/XMLSchema#date> ;
        owl:versionInfo     "20200624-0" ;
        skos:definition     "PDF/X-1a is a PDF specification which completes exchange using CMYK data and spots colour printing data."@en ;
        skos:inScheme       ns10:file-type ;
        skos:prefLabel      "PDF/X-1a"@en ;
        skos:topConceptOf   ns10:file-type ;
        ns7:altLabel        []  ;
        ns7:prefLabel       []  .

<http://publications.europa.eu/resource/authority/file-type/MAP_PRVW>
        a                   ns5:FileType , skos:Concept ;
        ns6:context         <http://publications.europa.eu/resource/authority/use-context/ODP> , <http://publications.europa.eu/resource/authority/use-context/IMMC> , <http://publications.europa.eu/resource/authority/use-context/CELLAR> ;
        ns9:authority-code  "MAP_PRVW" ;
        ns9:deprecated      "false" ;
        ns9:op-code         "MAP_PRVW" ;
        ns9:start.use       "2010-01-01" ;
        ns5:startDate       "2010-01-01"^^<http://www.w3.org/2001/XMLSchema#date> ;
        ns5:status          <http://publications.europa.eu/resource/authority/concept-status/CURRENT> ;
        ns5:xlDefinition    []  ;
        ns5:xlNotation      []  ;
        ns10:op-code        "MAP_PRVW" ;
        dc:identifier       "MAP_PRVW" ;
        ns4:created         "2015-04-21"^^<http://www.w3.org/2001/XMLSchema#date> ;
        ns4:dateSubmitted   "2015-04-22"^^<http://www.w3.org/2001/XMLSchema#date> ;
        owl:versionInfo     "20200624-0" ;
        skos:definition     "Esri's ArcGIS is a geographic information system (GIS) for working with maps and geographic information. Map previews are normal raster background maps."@en ;
        skos:inScheme       ns10:file-type ;
        skos:prefLabel      "ArcGIS Map Preview"@en ;
        skos:topConceptOf   ns10:file-type ;
        ns7:altLabel        []  ;
        ns7:prefLabel       []  .

<http://publications.europa.eu/resource/authority/file-type/XZ>
        a                   skos:Concept , ns5:FileType ;
        ns6:context         <http://publications.europa.eu/resource/authority/use-context/DCAT_AP> , <http://publications.europa.eu/resource/authority/use-context/IMMC> ;
        ns9:authority-code  "XZ" ;
        ns9:deprecated      "false" ;
        ns9:op-code         "XZ" ;
        ns9:op-mapped-code  []  ;
        ns9:start.use       "2010-10-23" ;
        ns5:startDate       "2010-10-23"^^<http://www.w3.org/2001/XMLSchema#date> ;
        ns5:status          <http://publications.europa.eu/resource/authority/concept-status/CURRENT> ;
        ns5:xlDefinition    []  ;
        ns5:xlNotation      []  ;
        ns5:xlNotation      []  ;
        ns10:op-code        "XZ" ;
        dc:identifier       "XZ" ;
        ns4:created         "2020-05-15"^^<http://www.w3.org/2001/XMLSchema#date> ;
        ns4:dateAccepted    "2020-06-04"^^<http://www.w3.org/2001/XMLSchema#date> ;
        ns4:dateSubmitted   "2020-05-19"^^<http://www.w3.org/2001/XMLSchema#date> ;
        owl:versionInfo     "20200624-0" ;
        skos:definition     "Compressed file produced using XZ Utils (free software command-line lossless data compressors, including LZMA and xz)."@en ;
        skos:inScheme       ns10:file-type ;
        skos:prefLabel      "xz"@en ;
        skos:topConceptOf   ns10:file-type ;
        ns7:altLabel        []  ;
        ns7:prefLabel       []  .

<http://publications.europa.eu/resource/authority/file-type/WFS_SRVC>
        a                   skos:Concept , ns5:FileType ;
        ns6:context         <http://publications.europa.eu/resource/authority/use-context/DCAT_AP> , <http://publications.europa.eu/resource/authority/use-context/ODP> , <http://publications.europa.eu/resource/authority/use-context/IMMC> ;
        ns9:authority-code  "WFS_SRVC" ;
        ns9:deprecated      "false" ;
        ns9:op-code         "WFS_SRVC" ;
        ns9:start.use       "2006-01-01" ;
        ns5:startDate       "2006-01-01"^^<http://www.w3.org/2001/XMLSchema#date> ;
        ns5:status          <http://publications.europa.eu/resource/authority/concept-status/CURRENT> ;
        ns5:xlDefinition    []  ;
        ns5:xlNotation      []  ;
        ns5:xlNotation      []  ;
        ns10:op-code        "WFS_SRVC" ;
        dc:identifier       "WFS_SRVC" ;
        ns4:created         "2018-11-12"^^<http://www.w3.org/2001/XMLSchema#date> ;
        ns4:dateAccepted    "2018-11-28"^^<http://www.w3.org/2001/XMLSchema#date> ;
        ns4:dateSubmitted   "2018-11-14"^^<http://www.w3.org/2001/XMLSchema#date> ;
        owl:versionInfo     "20200624-0" ;
        skos:definition     "The Open Geospatial Consortium Web Feature Service (WFS) Interface Standard provides an interface allowing requests for geospatial features across the web using platform-independent mechanisms and is independent of the underlying data store."@en ;
        skos:inScheme       ns10:file-type ;
        skos:prefLabel      "WFS"@en ;
        skos:topConceptOf   ns10:file-type ;
        ns7:altLabel        []  ;
        ns7:prefLabel       []  .

<http://publications.europa.eu/resource/authority/file-type/TAR_XZ>
        a                   ns5:FileType , skos:Concept ;
        ns6:context         <http://publications.europa.eu/resource/authority/use-context/CELLAR> , <http://publications.europa.eu/resource/authority/use-context/IMMC> ;
        ns9:authority-code  "TAR_XZ" ;
        ns9:deprecated      "false" ;
        ns9:op-code         "TAR_XZ" ;
        ns9:op-mapped-code  []  ;
        ns9:start.use       "2012-09-01" ;
        ns5:startDate       "2012-09-01"^^<http://www.w3.org/2001/XMLSchema#date> ;
        ns5:status          <http://publications.europa.eu/resource/authority/concept-status/CURRENT> ;
        ns5:xlDefinition    []  ;
        ns5:xlNotation      []  ;
        ns5:xlNotation      []  ;
        ns10:op-code        "TAR_XZ" ;
        dc:identifier       "TAR_XZ" ;
        ns4:created         "2014-03-04"^^<http://www.w3.org/2001/XMLSchema#date> ;
        ns4:dateAccepted    "2014-03-12"^^<http://www.w3.org/2001/XMLSchema#date> ;
        ns4:dateSubmitted   "2014-02-19"^^<http://www.w3.org/2001/XMLSchema#date> ;
        owl:versionInfo     "20200624-0" ;
        skos:definition     "TAR – tape archive – is a computer software utility for collecting many files into one archive file, often referred to as a tarball, for distribution or backup purposes. XZ is a lossless compression program and file format."@en ;
        skos:inScheme       ns10:file-type ;
        skos:prefLabel      "TAR XZ"@en ;
        skos:topConceptOf   ns10:file-type ;
        ns7:altLabel        []  ;
        ns7:prefLabel       []  .

<http://publications.europa.eu/resource/authority/file-type/ISO_ZIP>
        a                   skos:Concept , ns5:FileType ;
        ns6:context         <http://publications.europa.eu/resource/authority/use-context/IMMC> ;
        ns9:authority-code  "ISO_ZIP" ;
        ns9:deprecated      "false" ;
        ns9:op-code         "ISO_ZIP" ;
        ns9:op-mapped-code  []  ;
        ns9:start.use       "2012-09-01" ;
        ns5:startDate       "2012-09-01"^^<http://www.w3.org/2001/XMLSchema#date> ;
        ns5:status          <http://publications.europa.eu/resource/authority/concept-status/CURRENT> ;
        ns5:xlDefinition    []  ;
        ns5:xlNotation      []  ;
        ns5:xlNotation      []  ;
        ns10:op-code        "ISO_ZIP" ;
        dc:identifier       "ISO_ZIP" ;
        ns4:created         "2018-08-17"^^<http://www.w3.org/2001/XMLSchema#date> ;
        ns4:dateAccepted    "2018-09-12"^^<http://www.w3.org/2001/XMLSchema#date> ;
        ns4:dateSubmitted   "2018-08-29"^^<http://www.w3.org/2001/XMLSchema#date> ;
        owl:versionInfo     "20200624-0" ;
        skos:definition     "ZIP archive containing an ISO disc image file."@en ;
        skos:inScheme       ns10:file-type ;
        skos:prefLabel      "Zipped ISO image"@en ;
        skos:topConceptOf   ns10:file-type ;
        ns7:altLabel        []  ;
        ns7:prefLabel       []  .

<http://publications.europa.eu/resource/authority/file-type/PDFX>
        a                   skos:Concept , ns5:FileType ;
        ns6:context         <http://publications.europa.eu/resource/authority/use-context/CELLAR> , <http://publications.europa.eu/resource/authority/use-context/EUDOR> , <http://publications.europa.eu/resource/authority/use-context/IMMC> , <http://publications.europa.eu/resource/authority/use-context/PUB> ;
        ns9:authority-code  "PDFX" ;
        ns9:deprecated      "false" ;
        ns9:op-code         "PDFX" ;
        ns9:op-mapped-code  []  ;
        ns9:op-mapped-code  []  ;
        ns9:op-mapped-code  []  ;
        ns9:op-mapped-code  []  ;
        ns9:op-mapped-code  []  ;
        ns9:op-mapped-code  []  ;
        ns9:start.use       "2001-12-01" ;
        ns5:isTextual       false ;
        ns5:order           250 ;
        ns5:startDate       "2001-12-01"^^<http://www.w3.org/2001/XMLSchema#date> ;
        ns5:status          <http://publications.europa.eu/resource/authority/concept-status/CURRENT> ;
        ns5:xlDefinition    []  ;
        ns5:xlNotation      []  ;
        ns5:xlNotation      []  ;
        ns5:xlNotation      []  ;
        ns5:xlNotation      []  ;
        ns5:xlNotation      []  ;
        ns10:op-code        "PDFX" ;
        dc:identifier       "PDFX" ;
        ns4:created         "2012-03-19"^^<http://www.w3.org/2001/XMLSchema#date> ;
        ns4:dateAccepted    "2012-11-27"^^<http://www.w3.org/2001/XMLSchema#date> ;
        ns4:dateSubmitted   "2012-09-27"^^<http://www.w3.org/2001/XMLSchema#date> ;
        owl:versionInfo     "20200624-0" ;
        skos:definition     "PDF/X is a subset of the PDF standard. The purpose of PDF/X is to facilitate graphics exchange, and it therefore has a series of printing related requirements which do not apply to standard PDF files."@en ;
        skos:inScheme       ns10:file-type ;
        skos:prefLabel      "PDF/X"@en ;
        skos:topConceptOf   ns10:file-type ;
        ns7:altLabel        []  ;
        ns7:prefLabel       []  .

<http://publications.europa.eu/resource/authority/file-type/AZW>
        a                   skos:Concept , ns5:FileType ;
        ns6:context         <http://publications.europa.eu/resource/authority/use-context/CELLAR> , <http://publications.europa.eu/resource/authority/use-context/IMMC> ;
        ns9:authority-code  "AZW" ;
        ns9:deprecated      "false" ;
        ns9:op-code         "AZW" ;
        ns9:op-mapped-code  []  ;
        ns9:op-mapped-code  []  ;
        ns9:op-mapped-code  []  ;
        ns9:op-mapped-code  []  ;
        ns9:op-mapped-code  []  ;
        ns9:op-mapped-code  []  ;
        ns9:start.use       "2012-09-01" ;
        ns5:isTextual       false ;
        ns5:order           240 ;
        ns5:startDate       "2012-09-01"^^<http://www.w3.org/2001/XMLSchema#date> ;
        ns5:status          <http://publications.europa.eu/resource/authority/concept-status/CURRENT> ;
        ns5:xlDefinition    []  ;
        ns5:xlNotation      []  ;
        ns5:xlNotation      []  ;
        ns5:xlNotation      []  ;
        ns5:xlNotation      []  ;
        ns5:xlNotation      []  ;
        ns10:op-code        "AZW" ;
        dc:identifier       "AZW" ;
        ns4:created         "2012-03-19"^^<http://www.w3.org/2001/XMLSchema#date> ;
        ns4:dateAccepted    "2012-11-27"^^<http://www.w3.org/2001/XMLSchema#date> ;
        ns4:dateSubmitted   "2012-09-27"^^<http://www.w3.org/2001/XMLSchema#date> ;
        owl:versionInfo     "20200624-0" ;
        skos:definition     "AZW Kindle File Format is a proprietary e-book file format created by Amazon.com that can be downloaded and read on devices like smartphones, tablets, computers or e-readers that have Amazon's Kindle application."@en ;
        skos:inScheme       ns10:file-type ;
        skos:prefLabel      "Amazon Kindle eBook"@en ;
        skos:topConceptOf   ns10:file-type ;
        ns7:altLabel        []  ;
        ns7:prefLabel       []  .

<http://publications.europa.eu/resource/authority/file-type/EAR>
        a                   skos:Concept , ns5:FileType ;
        ns6:context         <http://publications.europa.eu/resource/authority/use-context/DCAT_AP> , <http://publications.europa.eu/resource/authority/use-context/IMMC> ;
        ns9:authority-code  "EAR" ;
        ns9:deprecated      "false" ;
        ns9:op-code         "EAR" ;
        ns9:op-mapped-code  []  ;
        ns9:start.use       "2006-05-11" ;
        ns5:startDate       "2006-05-11"^^<http://www.w3.org/2001/XMLSchema#date> ;
        ns5:status          <http://publications.europa.eu/resource/authority/concept-status/CURRENT> ;
        ns5:xlDefinition    []  ;
        ns5:xlNotation      []  ;
        ns5:xlNotation      []  ;
        ns10:op-code        "EAR" ;
        dc:identifier       "EAR" ;
        ns4:created         "2020-05-15"^^<http://www.w3.org/2001/XMLSchema#date> ;
        ns4:dateAccepted    "2020-06-04"^^<http://www.w3.org/2001/XMLSchema#date> ;
        ns4:dateSubmitted   "2020-05-19"^^<http://www.w3.org/2001/XMLSchema#date> ;
        owl:versionInfo     "20200624-0" ;
        skos:definition     "EAR (Enterprise Application aRchive) is a file format used by Java EE for packaging one or more modules into a single archive."@en ;
        skos:inScheme       ns10:file-type ;
        skos:prefLabel      "EAR"@en ;
        skos:topConceptOf   ns10:file-type ;
        ns7:altLabel        []  ;
        ns7:prefLabel       []  .

<http://publications.europa.eu/resource/authority/file-type/JS>
        a                   ns5:FileType , skos:Concept ;
        ns6:context         <http://publications.europa.eu/resource/authority/use-context/ODP> , <http://publications.europa.eu/resource/authority/use-context/DCAT_AP> , <http://publications.europa.eu/resource/authority/use-context/IMMC> ;
        ns9:authority-code  "JS" ;
        ns9:deprecated      "false" ;
        ns9:op-code         "JS" ;
        ns9:op-mapped-code  []  ;
        ns9:op-mapped-code  []  ;
        ns9:op-mapped-code  []  ;
        ns9:op-mapped-code  []  ;
        ns9:op-mapped-code  []  ;
        ns9:start.use       "1995-12-04" ;
        ns5:isTextual       true ;
        ns5:order           6 ;
        ns5:startDate       "1995-12-04"^^<http://www.w3.org/2001/XMLSchema#date> ;
        ns5:status          <http://publications.europa.eu/resource/authority/concept-status/CURRENT> ;
        ns5:xlDefinition    []  ;
        ns5:xlNotation      []  ;
        ns5:xlNotation      []  ;
        ns5:xlNotation      []  ;
        ns5:xlNotation      []  ;
        ns5:xlNotation      []  ;
        ns10:op-code        "JS" ;
        dc:identifier       "JS" ;
        ns4:created         "2018-11-06"^^<http://www.w3.org/2001/XMLSchema#date> ;
        ns4:dateAccepted    "2018-11-28"^^<http://www.w3.org/2001/XMLSchema#date> ;
        ns4:dateSubmitted   "2018-11-14"^^<http://www.w3.org/2001/XMLSchema#date> ;
        owl:versionInfo     "20200624-0" ;
        skos:definition     "JavaScript is a high-level, interpreted programming language. It is a language which is also characterized as dynamic, weakly typed, prototype-based and multi-paradigm."@en ;
        skos:inScheme       ns10:file-type ;
        skos:prefLabel      "JavaScript"@en ;
        skos:topConceptOf   ns10:file-type ;
        ns7:altLabel        []  ;
        ns7:prefLabel       []  .

<http://publications.europa.eu/resource/authority/file-type/FMX4>
        a                   skos:Concept , ns5:FileType ;
        ns6:context         <http://publications.europa.eu/resource/authority/use-context/IMMC> , <http://publications.europa.eu/resource/authority/use-context/CELLAR> , <http://publications.europa.eu/resource/authority/use-context/EUDOR> , <http://publications.europa.eu/resource/authority/use-context/ODP> ;
        ns9:authority-code  "FMX4" ;
        ns9:deprecated      "false" ;
        ns9:op-code         "FMX4" ;
        ns9:op-mapped-code  []  ;
        ns9:op-mapped-code  []  ;
        ns9:op-mapped-code  []  ;
        ns9:op-mapped-code  []  ;
        ns9:op-mapped-code  []  ;
        ns9:op-mapped-code  []  ;
        ns9:start.use       "2004-05-01" ;
        ns5:isTextual       true ;
        ns5:order           180 ;
        ns5:startDate       "2004-05-01"^^<http://www.w3.org/2001/XMLSchema#date> ;
        ns5:status          <http://publications.europa.eu/resource/authority/concept-status/CURRENT> ;
        ns5:xlDefinition    []  ;
        ns5:xlNotation      []  ;
        ns5:xlNotation      []  ;
        ns5:xlNotation      []  ;
        ns5:xlNotation      []  ;
        ns5:xlNotation      []  ;
        ns10:op-code        "FMX4" ;
        dc:identifier       "FMX4" ;
        ns4:created         "2012-03-19"^^<http://www.w3.org/2001/XMLSchema#date> ;
        ns4:dateAccepted    "2012-11-27"^^<http://www.w3.org/2001/XMLSchema#date> ;
        ns4:dateSubmitted   "2012-09-27"^^<http://www.w3.org/2001/XMLSchema#date> ;
        owl:versionInfo     "20200624-0" ;
        skos:definition     "Formex describes the format for the exchange of data between the Publication Office and its contractors. In particular, it defines the logical markup for documents which are published in the different series of the Offical Journal of the European Union. Formex V4 is based on the international standard XML."@en ;
        skos:inScheme       ns10:file-type ;
        skos:prefLabel      "Formex 4"@en ;
        skos:topConceptOf   ns10:file-type ;
        ns7:altLabel        []  ;
        ns7:prefLabel       []  .

<http://publications.europa.eu/resource/authority/file-type/CSV>
        a                    ns5:FileType , skos:Concept ;
        ns6:context          <http://publications.europa.eu/resource/authority/use-context/ODP> , <http://publications.europa.eu/resource/authority/use-context/IMMC> , <http://publications.europa.eu/resource/authority/use-context/DCAT_AP> , <http://publications.europa.eu/resource/authority/use-context/CELLAR> ;
        ns9:authority-code   "CSV" ;
        ns9:deprecated       "false" ;
        ns9:op-code          "CSV" ;
        ns9:op-mapped-code   []  ;
        ns9:op-mapped-code   []  ;
        ns9:op-mapped-code   []  ;
        ns9:op-mapped-code   []  ;
        ns9:start.use        "2013-05-21" ;
        ns5:machineReadable  true ;
        ns5:nonPropExt       true ;
        ns5:startDate        "2013-05-21"^^<http://www.w3.org/2001/XMLSchema#date> ;
        ns5:status           <http://publications.europa.eu/resource/authority/concept-status/CURRENT> ;
        ns5:xlDefinition     []  ;
        ns5:xlNotation       []  ;
        ns5:xlNotation       []  ;
        ns5:xlNotation       []  ;
        ns10:op-code         "CSV" ;
        dc:identifier        "CSV" ;
        ns4:created          "2013-05-21"^^<http://www.w3.org/2001/XMLSchema#date> ;
        ns4:dateAccepted     "2013-09-26"^^<http://www.w3.org/2001/XMLSchema#date> ;
        ns4:dateSubmitted    "2013-09-26"^^<http://www.w3.org/2001/XMLSchema#date> ;
        owl:versionInfo      "20200624-0" ;
        skos:definition      "CSV – comma-separated values – files store tabular data (numbers and text) in plain text. Each line of the file is a data record. Each record consists of one or more fields, separated by commas."@en ;
        skos:inScheme        ns10:file-type ;
        skos:prefLabel       "CSV"@en ;
        skos:topConceptOf    ns10:file-type ;
        ns7:altLabel         []  ;
        ns7:prefLabel        []  .

<http://publications.europa.eu/resource/authority/file-type/ODS>
        a                    ns5:FileType , skos:Concept ;
        ns6:context          <http://publications.europa.eu/resource/authority/use-context/ODP> , <http://publications.europa.eu/resource/authority/use-context/DCAT_AP> , <http://publications.europa.eu/resource/authority/use-context/CELLAR> , <http://publications.europa.eu/resource/authority/use-context/IMMC> ;
        ns9:authority-code   "ODS" ;
        ns9:deprecated       "false" ;
        ns9:op-code          "ODS" ;
        ns9:op-mapped-code   []  ;
        ns9:op-mapped-code   []  ;
        ns9:op-mapped-code   []  ;
        ns9:start.use        "2013-11-27" ;
        ns5:machineReadable  true ;
        ns5:nonPropExt       true ;
        ns5:startDate        "2013-11-27"^^<http://www.w3.org/2001/XMLSchema#date> ;
        ns5:status           <http://publications.europa.eu/resource/authority/concept-status/CURRENT> ;
        ns5:xlDefinition     []  ;
        ns5:xlNotation       []  ;
        ns5:xlNotation       []  ;
        ns10:op-code         "ODS" ;
        dc:identifier        "ODS" ;
        ns4:created          "2012-09-01"^^<http://www.w3.org/2001/XMLSchema#date> ;
        ns4:dateAccepted     "2014-03-12"^^<http://www.w3.org/2001/XMLSchema#date> ;
        ns4:dateSubmitted    "2014-02-19"^^<http://www.w3.org/2001/XMLSchema#date> ;
        owl:versionInfo      "20200624-0" ;
        skos:definition      "ODS is an OpenDocument file format for spreadsheets. OpenDocument was developed with the aim of providing an open, XML-based file format specification for office applications."@en ;
        skos:inScheme        ns10:file-type ;
        skos:prefLabel       "ODS"@en ;
        skos:topConceptOf    ns10:file-type ;
        ns7:altLabel         []  ;
        ns7:prefLabel        []  .

<http://publications.europa.eu/resource/authority/file-type/RTF>
        a                   skos:Concept , ns5:FileType ;
        ns6:context         <http://publications.europa.eu/resource/authority/use-context/CELLAR> , <http://publications.europa.eu/resource/authority/use-context/IMMC> , <http://publications.europa.eu/resource/authority/use-context/OJEEP> ;
        ns9:authority-code  "RTF" ;
        ns9:deprecated      "false" ;
        ns9:op-code         "RTF" ;
        ns9:op-mapped-code  []  ;
        ns9:op-mapped-code  []  ;
        ns9:op-mapped-code  []  ;
        ns9:op-mapped-code  []  ;
        ns9:op-mapped-code  []  ;
        ns9:op-mapped-code  []  ;
        ns9:op-mapped-code  []  ;
        ns9:start.use       "2012-09-01" ;
        ns5:isTextual       true ;
        ns5:nonPropExt      true ;
        ns5:order           110 ;
        ns5:startDate       "2012-09-01"^^<http://www.w3.org/2001/XMLSchema#date> ;
        ns5:status          <http://publications.europa.eu/resource/authority/concept-status/CURRENT> ;
        ns5:xlDefinition    []  ;
        ns5:xlNotation      []  ;
        ns5:xlNotation      []  ;
        ns5:xlNotation      []  ;
        ns5:xlNotation      []  ;
        ns5:xlNotation      []  ;
        ns10:op-code        "RTF" ;
        dc:identifier       "RTF" ;
        ns4:created         "2012-03-19"^^<http://www.w3.org/2001/XMLSchema#date> ;
        ns4:dateAccepted    "2012-11-27"^^<http://www.w3.org/2001/XMLSchema#date> ;
        ns4:dateSubmitted   "2012-09-27"^^<http://www.w3.org/2001/XMLSchema#date> ;
        owl:versionInfo     "20200624-0" ;
        skos:definition     "RTF – Rich Text Format – is a proprietary document file format developed for cross-platform document interchange with Microsoft products."@en ;
        skos:inScheme       ns10:file-type ;
        skos:prefLabel      "RTF"@en ;
        skos:topConceptOf   ns10:file-type ;
        ns7:altLabel        []  ;
        ns7:prefLabel       []  .

<http://publications.europa.eu/resource/authority/file-type/MHTML>
        a                   skos:Concept , ns5:FileType ;
        ns6:context         <http://publications.europa.eu/resource/authority/use-context/IMMC> ;
        ns9:authority-code  "MHTML" ;
        ns9:deprecated      "false" ;
        ns9:op-code         "MHTML" ;
        ns9:op-mapped-code  []  ;
        ns9:op-mapped-code  []  ;
        ns9:start.use       "1999-03-01" ;
        ns5:startDate       "1999-03-01"^^<http://www.w3.org/2001/XMLSchema#date> ;
        ns5:status          <http://publications.europa.eu/resource/authority/concept-status/CURRENT> ;
        ns5:xlDefinition    []  ;
        ns5:xlNotation      []  ;
        ns5:xlNotation      []  ;
        ns5:xlNotation      []  ;
        ns10:op-code        "MHTML" ;
        dc:identifier       "MHTML" ;
        ns4:created         "2016-08-18"^^<http://www.w3.org/2001/XMLSchema#date> ;
        ns4:dateAccepted    "2016-09-09"^^<http://www.w3.org/2001/XMLSchema#date> ;
        ns4:dateSubmitted   "2016-08-22"^^<http://www.w3.org/2001/XMLSchema#date> ;
        owl:versionInfo     "20200624-0" ;
        skos:definition     "MHTML – MIME Encapsulation of Aggregate HTML Documents – is a web page archive format used to combine in a single document the HTML code and its companion resources that are otherwise represented by external links (such as images, Flash animations, Java applets and audio files). The content of an MHTML file is encoded as if it were an HTML e-mail message."@en ;
        skos:inScheme       ns10:file-type ;
        skos:prefLabel      "MHTML"@en ;
        skos:topConceptOf   ns10:file-type ;
        ns7:altLabel        []  ;
        ns7:prefLabel       []  .

<http://publications.europa.eu/resource/authority/file-type/N3>
        a                   skos:Concept , ns5:FileType ;
        ns6:context         <http://publications.europa.eu/resource/authority/use-context/DCAT_AP> , <http://publications.europa.eu/resource/authority/use-context/IMMC> , <http://publications.europa.eu/resource/authority/use-context/ODP> ;
        ns9:authority-code  "N3" ;
        ns9:deprecated      "false" ;
        ns9:op-code         "N3" ;
        ns9:op-mapped-code  []  ;
        ns9:start.use       "2008-01-01" ;
        ns5:startDate       "2008-01-01"^^<http://www.w3.org/2001/XMLSchema#date> ;
        ns5:status          <http://publications.europa.eu/resource/authority/concept-status/CURRENT> ;
        ns5:xlDefinition    []  ;
        ns5:xlNotation      []  ;
        ns5:xlNotation      []  ;
        ns10:op-code        "N3" ;
        dc:identifier       "N3" ;
        ns4:created         "2018-11-06"^^<http://www.w3.org/2001/XMLSchema#date> ;
        ns4:dateAccepted    "2018-11-28"^^<http://www.w3.org/2001/XMLSchema#date> ;
        ns4:dateSubmitted   "2018-11-14"^^<http://www.w3.org/2001/XMLSchema#date> ;
        owl:versionInfo     "20200624-0" ;
        skos:definition     "Non-XML serialization of Resource Description Framework models."@en ;
        skos:inScheme       ns10:file-type ;
        skos:prefLabel      "N3"@en ;
        skos:topConceptOf   ns10:file-type ;
        ns7:altLabel        []  ;
        ns7:prefLabel       []  .

<http://publications.europa.eu/resource/authority/file-type/RDF_TRIX>
        a                   ns5:FileType , skos:Concept ;
        ns6:context         <http://publications.europa.eu/resource/authority/use-context/IMMC> ;
        ns9:authority-code  "RDF_TRIX" ;
        ns9:deprecated      "false" ;
        ns9:op-code         "RDF_TRIX" ;
        ns9:op-mapped-code  []  ;
        ns9:op-mapped-code  []  ;
        ns9:start.use       "2004-05-13" ;
        ns5:startDate       "2004-05-13"^^<http://www.w3.org/2001/XMLSchema#date> ;
        ns5:status          <http://publications.europa.eu/resource/authority/concept-status/CURRENT> ;
        ns5:xlDefinition    []  ;
        ns5:xlNotation      []  ;
        ns5:xlNotation      []  ;
        ns5:xlNotation      []  ;
        ns10:op-code        "RDF_TRIX" ;
        dc:identifier       "RDF_TRIX" ;
        ns4:created         "2020-05-12"^^<http://www.w3.org/2001/XMLSchema#date> ;
        ns4:dateAccepted    "2020-06-04"^^<http://www.w3.org/2001/XMLSchema#date> ;
        ns4:dateSubmitted   "2020-05-19"^^<http://www.w3.org/2001/XMLSchema#date> ;
        owl:versionInfo     "20200624-0" ;
        skos:definition     "TriX (Triples in XML) is a serialization format for RDF (Resource Description Framework) graphs. It is an XML format for serializing Named Graphs and RDF Datasets which offers a compact and readable alternative to the XML-based RDF/XML syntax."@en ;
        skos:inScheme       ns10:file-type ;
        skos:prefLabel      "RDF TriX"@en ;
        skos:topConceptOf   ns10:file-type ;
        ns7:altLabel        []  ;
        ns7:prefLabel       []  .

<http://publications.europa.eu/resource/authority/file-type/SVG>
        a                   ns5:FileType , skos:Concept ;
        ns6:context         <http://publications.europa.eu/resource/authority/use-context/IMMC> , <http://publications.europa.eu/resource/authority/use-context/ODP> , <http://publications.europa.eu/resource/authority/use-context/DCAT_AP> ;
        ns9:authority-code  "SVG" ;
        ns9:deprecated      "false" ;
        ns9:op-code         "SVG" ;
        ns9:op-mapped-code  []  ;
        ns9:op-mapped-code  []  ;
        ns9:start.use       "2001-09-04" ;
        ns5:startDate       "2001-09-04"^^<http://www.w3.org/2001/XMLSchema#date> ;
        ns5:status          <http://publications.europa.eu/resource/authority/concept-status/CURRENT> ;
        ns5:xlDefinition    []  ;
        ns5:xlNotation      []  ;
        ns5:xlNotation      []  ;
        ns5:xlNotation      []  ;
        ns10:op-code        "SVG" ;
        dc:identifier       "SVG" ;
        ns4:created         "2018-11-06"^^<http://www.w3.org/2001/XMLSchema#date> ;
        ns4:dateAccepted    "2018-11-28"^^<http://www.w3.org/2001/XMLSchema#date> ;
        ns4:dateSubmitted   "2018-11-14"^^<http://www.w3.org/2001/XMLSchema#date> ;
        owl:versionInfo     "20200624-0" ;
        skos:definition     "Open standard for two-dimensional vector graphics."@en ;
        skos:inScheme       ns10:file-type ;
        skos:prefLabel      "SVG"@en ;
        skos:topConceptOf   ns10:file-type ;
        ns7:altLabel        []  ;
        ns7:prefLabel       []  .

<http://publications.europa.eu/resource/authority/file-type/APPX>
        a                   ns5:FileType , skos:Concept ;
        ns6:context         <http://publications.europa.eu/resource/authority/use-context/IMMC> , <http://publications.europa.eu/resource/authority/use-context/DCAT_AP> ;
        ns9:authority-code  "APPX" ;
        ns9:deprecated      "false" ;
        ns9:op-code         "APPX" ;
        ns9:op-mapped-code  []  ;
        ns9:op-mapped-code  []  ;
        ns9:start.use       "2012-10-26" ;
        ns5:startDate       "2012-10-26"^^<http://www.w3.org/2001/XMLSchema#date> ;
        ns5:status          <http://publications.europa.eu/resource/authority/concept-status/CURRENT> ;
        ns5:xlDefinition    []  ;
        ns5:xlNotation      []  ;
        ns5:xlNotation      []  ;
        ns5:xlNotation      []  ;
        ns10:op-code        "APPX" ;
        dc:identifier       "APPX" ;
        ns4:created         "2020-05-15"^^<http://www.w3.org/2001/XMLSchema#date> ;
        ns4:dateAccepted    "2020-06-04"^^<http://www.w3.org/2001/XMLSchema#date> ;
        ns4:dateSubmitted   "2020-05-19"^^<http://www.w3.org/2001/XMLSchema#date> ;
        owl:versionInfo     "20200624-0" ;
        skos:definition     "AppX is a file format used to distribute and install apps on Windows 8.x and 10, Windows Phone 8.1, Windows 10 Mobile, Xbox One, Hololens and Windows 10 IoT Core."@en ;
        skos:inScheme       ns10:file-type ;
        skos:prefLabel      "AppX"@en ;
        skos:topConceptOf   ns10:file-type ;
        ns7:altLabel        []  ;
        ns7:prefLabel       []  .

<http://publications.europa.eu/resource/authority/file-type/ODF>
        a                   skos:Concept , ns5:FileType ;
        ns6:context         <http://publications.europa.eu/resource/authority/use-context/OJEEP> , <http://publications.europa.eu/resource/authority/use-context/CELLAR> , <http://publications.europa.eu/resource/authority/use-context/ODP> , <http://publications.europa.eu/resource/authority/use-context/IMMC> ;
        ns9:authority-code  "ODF" ;
        ns9:deprecated      "false" ;
        ns9:op-code         "ODF" ;
        ns9:op-mapped-code  []  ;
        ns9:start.use       "2012-09-01" ;
        ns5:startDate       "2012-09-01"^^<http://www.w3.org/2001/XMLSchema#date> ;
        ns5:status          <http://publications.europa.eu/resource/authority/concept-status/CURRENT> ;
        ns5:xlDefinition    []  ;
        ns5:xlNotation      []  ;
        ns5:xlNotation      []  ;
        ns5:xlNotation      []  ;
        ns10:op-code        "ODF" ;
        dc:identifier       "ODF" ;
        ns4:created         "2014-03-04"^^<http://www.w3.org/2001/XMLSchema#date> ;
        owl:versionInfo     "20200624-0" ;
        skos:definition     "ODF – Open Document Format for Office Applications, also known as OpenDocument – is an XML-based file format for spreadsheets, charts, presentations and word processing documents. It was developed with the aim of providing an open, XML-based file format specification for office applications."@en ;
        skos:inScheme       ns10:file-type ;
        skos:prefLabel      "ODF"@en ;
        skos:topConceptOf   ns10:file-type ;
        ns7:altLabel        []  ;
        ns7:prefLabel       []  .

<http://publications.europa.eu/resource/authority/file-type/HTML_SIMPL>
        a                   skos:Concept , ns5:FileType ;
        ns6:context         <http://publications.europa.eu/resource/authority/use-context/CELLAR> , <http://publications.europa.eu/resource/authority/use-context/IMMC> ;
        ns9:authority-code  "HTML_SIMPL" ;
        ns9:deprecated      "false" ;
        ns9:op-code         "HTML_SIMPL" ;
        ns9:op-mapped-code  []  ;
        ns9:op-mapped-code  []  ;
        ns9:op-mapped-code  []  ;
        ns9:op-mapped-code  []  ;
        ns9:op-mapped-code  []  ;
        ns9:op-mapped-code  []  ;
        ns9:op-mapped-code  []  ;
        ns9:start.use       "2012-09-01" ;
        ns5:isTextual       true ;
        ns5:order           310 ;
        ns5:startDate       "2012-09-01"^^<http://www.w3.org/2001/XMLSchema#date> ;
        ns5:status          <http://publications.europa.eu/resource/authority/concept-status/CURRENT> ;
        ns5:xlDefinition    []  ;
        ns5:xlNotation      []  ;
        ns5:xlNotation      []  ;
        ns5:xlNotation      []  ;
        ns5:xlNotation      []  ;
        ns5:xlNotation      []  ;
        ns5:xlNotation      []  ;
        ns10:op-code        "HTML_SIMPL" ;
        dc:identifier       "HTML_SIMPL" ;
        ns4:created         "2016-05-12"^^<http://www.w3.org/2001/XMLSchema#date> ;
        ns4:dateAccepted    "2016-06-01"^^<http://www.w3.org/2001/XMLSchema#date> ;
        ns4:dateSubmitted   "2016-05-18"^^<http://www.w3.org/2001/XMLSchema#date> ;
        owl:versionInfo     "20200624-0" ;
        skos:definition     "HTML is a markup language for describing web documents. Its simplified version is used for storage in the Publications Office."@en ;
        skos:inScheme       ns10:file-type ;
        skos:prefLabel      "HTML simplified"@en ;
        skos:topConceptOf   ns10:file-type ;
        ns7:altLabel        []  ;
        ns7:prefLabel       []  .

<http://publications.europa.eu/resource/authority/file-type/ICS>
        a                    ns5:FileType , skos:Concept ;
        ns6:context          <http://publications.europa.eu/resource/authority/use-context/DCAT_AP> , <http://publications.europa.eu/resource/authority/use-context/ODP> , <http://publications.europa.eu/resource/authority/use-context/IMMC> ;
        ns9:authority-code   "ICS" ;
        ns9:deprecated       "false" ;
        ns9:op-code          "ICS" ;
        ns9:op-mapped-code   []  ;
        ns9:op-mapped-code   []  ;
        ns9:op-mapped-code   []  ;
        ns9:op-mapped-code   []  ;
        ns9:op-mapped-code   []  ;
        ns9:op-mapped-code   []  ;
        ns9:start.use        "1998-01-01" ;
        ns5:machineReadable  true ;
        ns5:nonPropExt       true ;
        ns5:startDate        "1998-01-01"^^<http://www.w3.org/2001/XMLSchema#date> ;
        ns5:status           <http://publications.europa.eu/resource/authority/concept-status/CURRENT> ;
        ns5:xlDefinition     []  ;
        ns5:xlNotation       []  ;
        ns5:xlNotation       []  ;
        ns5:xlNotation       []  ;
        ns5:xlNotation       []  ;
        ns5:xlNotation       []  ;
        ns10:op-code         "ICS" ;
        dc:identifier        "ICS" ;
        ns4:created          "2018-11-06"^^<http://www.w3.org/2001/XMLSchema#date> ;
        ns4:dateAccepted     "2018-11-28"^^<http://www.w3.org/2001/XMLSchema#date> ;
        ns4:dateSubmitted    "2018-11-14"^^<http://www.w3.org/2001/XMLSchema#date> ;
        owl:versionInfo      "20200624-0" ;
        skos:definition      "iCalendar is a computer file format which allows Internet users to send meeting requests and tasks to other Internet users by sharing or sending files in this format through various methods."@en ;
        skos:inScheme        ns10:file-type ;
        skos:prefLabel       "ICalendar"@en ;
        skos:topConceptOf    ns10:file-type ;
        ns7:altLabel         []  ;
        ns7:prefLabel        []  .

<http://publications.europa.eu/resource/authority/file-type/PDF>
        a                   ns5:FileType , skos:Concept ;
        ns6:context         <http://publications.europa.eu/resource/authority/use-context/EUDOR> , <http://publications.europa.eu/resource/authority/use-context/ODP> , <http://publications.europa.eu/resource/authority/use-context/PUB> , <http://publications.europa.eu/resource/authority/use-context/DCAT_AP> , <http://publications.europa.eu/resource/authority/use-context/CELLAR> , <http://publications.europa.eu/resource/authority/use-context/OJEEP> , <http://publications.europa.eu/resource/authority/use-context/IMMC> ;
        ns9:authority-code  "PDF" ;
        ns9:deprecated      "false" ;
        ns9:op-code         "PDF" ;
        ns9:op-mapped-code  []  ;
        ns9:op-mapped-code  []  ;
        ns9:op-mapped-code  []  ;
        ns9:op-mapped-code  []  ;
        ns9:op-mapped-code  []  ;
        ns9:op-mapped-code  []  ;
        ns9:start.use       "2012-09-01" ;
        ns5:isTextual       false ;
        ns5:order           230 ;
        ns5:startDate       "2012-09-01"^^<http://www.w3.org/2001/XMLSchema#date> ;
        ns5:status          <http://publications.europa.eu/resource/authority/concept-status/CURRENT> ;
        ns5:xlDefinition    []  ;
        ns5:xlNotation      []  ;
        ns5:xlNotation      []  ;
        ns5:xlNotation      []  ;
        ns5:xlNotation      []  ;
        ns5:xlNotation      []  ;
        ns10:op-code        "PDF" ;
        dc:identifier       "PDF" ;
        ns4:created         "2012-03-19"^^<http://www.w3.org/2001/XMLSchema#date> ;
        ns4:dateAccepted    "2012-11-27"^^<http://www.w3.org/2001/XMLSchema#date> ;
        ns4:dateSubmitted   "2012-09-27"^^<http://www.w3.org/2001/XMLSchema#date> ;
        owl:versionInfo     "20200624-0" ;
        skos:definition     "PDF – Portable Document Format – is a file format developed to present documents, including text formatting and images, in a manner independent of application software, hardware and operating systems. Based on the PostScript language, each PDF file encapsulates a complete description of a fixed-layout flat document, including the text, fonts, vector graphics, raster images and other information needed to display it. PDF was standardized as an open format and does not require any royalties for its implementation."@en ;
        skos:inScheme       ns10:file-type ;
        skos:prefLabel      "PDF"@en ;
        skos:topConceptOf   ns10:file-type ;
        ns7:altLabel        []  ;
        ns7:prefLabel       []  .

<http://publications.europa.eu/resource/authority/file-type/SGML>
        a                   ns5:FileType , skos:Concept ;
        ns6:context         <http://publications.europa.eu/resource/authority/use-context/DCAT_AP> , <http://publications.europa.eu/resource/authority/use-context/IMMC> , <http://publications.europa.eu/resource/authority/use-context/EUDOR> , <http://publications.europa.eu/resource/authority/use-context/ODP> , <http://publications.europa.eu/resource/authority/use-context/CELLAR> ;
        ns9:authority-code  "SGML" ;
        ns9:deprecated      "false" ;
        ns9:op-code         "SGML" ;
        ns9:op-mapped-code  []  ;
        ns9:op-mapped-code  []  ;
        ns9:op-mapped-code  []  ;
        ns9:op-mapped-code  []  ;
        ns9:op-mapped-code  []  ;
        ns9:op-mapped-code  []  ;
        ns9:op-mapped-code  []  ;
        ns9:start.use       "2012-09-01" ;
        ns5:isTextual       true ;
        ns5:order           100 ;
        ns5:startDate       "2012-09-01"^^<http://www.w3.org/2001/XMLSchema#date> ;
        ns5:status          <http://publications.europa.eu/resource/authority/concept-status/CURRENT> ;
        ns5:xlDefinition    []  ;
        ns5:xlNotation      []  ;
        ns5:xlNotation      []  ;
        ns5:xlNotation      []  ;
        ns5:xlNotation      []  ;
        ns5:xlNotation      []  ;
        ns5:xlNotation      []  ;
        ns10:op-code        "SGML" ;
        dc:identifier       "SGML" ;
        ns4:created         "2012-03-19"^^<http://www.w3.org/2001/XMLSchema#date> ;
        ns4:dateAccepted    "2012-11-27"^^<http://www.w3.org/2001/XMLSchema#date> ;
        ns4:dateSubmitted   "2012-09-27"^^<http://www.w3.org/2001/XMLSchema#date> ;
        owl:versionInfo     "20200624-0" ;
        skos:definition     "SGML – Standard Generalized Markup Language – is a standard for defining generalized markup languages for documents. Generalized markup is based on two postulates: markup should be declarative and rigorous."@en ;
        skos:inScheme       ns10:file-type ;
        skos:prefLabel      "SGML"@en ;
        skos:topConceptOf   ns10:file-type ;
        ns7:altLabel        []  ;
        ns7:prefLabel       []  .

<http://publications.europa.eu/resource/authority/file-type/PDF1X>
        a                   skos:Concept , ns5:FileType ;
        ns6:context         <http://publications.europa.eu/resource/authority/use-context/IMMC> , <http://publications.europa.eu/resource/authority/use-context/CELLAR> ;
        ns9:authority-code  "PDF1X" ;
        ns9:deprecated      "false" ;
        ns9:op-code         "PDF1X" ;
        ns9:op-mapped-code  []  ;
        ns9:op-mapped-code  []  ;
        ns9:op-mapped-code  []  ;
        ns9:op-mapped-code  []  ;
        ns9:op-mapped-code  []  ;
        ns9:op-mapped-code  []  ;
        ns9:op-mapped-code  []  ;
        ns9:start.use       "2012-09-01" ;
        ns5:isTextual       false ;
        ns5:order           280 ;
        ns5:startDate       "2012-09-01"^^<http://www.w3.org/2001/XMLSchema#date> ;
        ns5:status          <http://publications.europa.eu/resource/authority/concept-status/CURRENT> ;
        ns5:xlDefinition    []  ;
        ns5:xlNotation      []  ;
        ns5:xlNotation      []  ;
        ns5:xlNotation      []  ;
        ns5:xlNotation      []  ;
        ns5:xlNotation      []  ;
        ns5:xlNotation      []  ;
        ns10:op-code        "PDF1X" ;
        dc:identifier       "PDF1X" ;
        ns4:created         "2015-12-03"^^<http://www.w3.org/2001/XMLSchema#date> ;
        ns4:dateAccepted    "2016-01-20"^^<http://www.w3.org/2001/XMLSchema#date> ;
        ns4:dateSubmitted   "2016-01-06"^^<http://www.w3.org/2001/XMLSchema#date> ;
        owl:versionInfo     "20200624-0" ;
        skos:definition     "PDF1X is a PDF specification used mainly for high quality color printing."@en ;
        skos:inScheme       ns10:file-type ;
        skos:prefLabel      "PDF1X"@en ;
        skos:topConceptOf   ns10:file-type ;
        ns7:altLabel        []  ;
        ns7:prefLabel       []  .

<http://publications.europa.eu/resource/authority/file-type/PPT>
        a                   skos:Concept , ns5:FileType ;
        ns6:context         <http://publications.europa.eu/resource/authority/use-context/ODP> , <http://publications.europa.eu/resource/authority/use-context/DCAT_AP> , <http://publications.europa.eu/resource/authority/use-context/IMMC> , <http://publications.europa.eu/resource/authority/use-context/OJEEP> , <http://publications.europa.eu/resource/authority/use-context/CELLAR> ;
        ns9:authority-code  "PPT" ;
        ns9:deprecated      "false" ;
        ns9:op-code         "PPT" ;
        ns9:op-mapped-code  []  ;
        ns9:op-mapped-code  []  ;
        ns9:op-mapped-code  []  ;
        ns9:op-mapped-code  []  ;
        ns9:op-mapped-code  []  ;
        ns9:op-mapped-code  []  ;
        ns9:start.use       "2012-09-01" ;
        ns5:isTextual       false ;
        ns5:order           140 ;
        ns5:startDate       "2012-09-01"^^<http://www.w3.org/2001/XMLSchema#date> ;
        ns5:status          <http://publications.europa.eu/resource/authority/concept-status/CURRENT> ;
        ns5:xlDefinition    []  ;
        ns5:xlNotation      []  ;
        ns5:xlNotation      []  ;
        ns5:xlNotation      []  ;
        ns5:xlNotation      []  ;
        ns5:xlNotation      []  ;
        ns10:op-code        "PPT" ;
        dc:identifier       "PPT" ;
        ns4:created         "2012-03-19"^^<http://www.w3.org/2001/XMLSchema#date> ;
        ns4:dateAccepted    "2012-11-27"^^<http://www.w3.org/2001/XMLSchema#date> ;
        ns4:dateSubmitted   "2012-09-27"^^<http://www.w3.org/2001/XMLSchema#date> ;
        owl:versionInfo     "20200624-0" ;
        skos:definition     "PPT is a binary media type of Microsoft PowerPoint presentation program. PowerPoint was originally designed to provide visuals for group presentations within business organizations, but has come to be very widely used in many other communication situations, both in business and beyond."@en ;
        skos:inScheme       ns10:file-type ;
        skos:prefLabel      "PowerPoint PPT"@en ;
        skos:topConceptOf   ns10:file-type ;
        ns7:altLabel        []  ;
        ns7:prefLabel       []  .

<http://publications.europa.eu/resource/authority/file-type/JAR>
        a                   ns5:FileType , skos:Concept ;
        ns6:context         <http://publications.europa.eu/resource/authority/use-context/IMMC> , <http://publications.europa.eu/resource/authority/use-context/DCAT_AP> ;
        ns9:authority-code  "JAR" ;
        ns9:deprecated      "false" ;
        ns9:op-code         "JAR" ;
        ns9:op-mapped-code  []  ;
        ns9:start.use       "1997-01-01" ;
        ns5:startDate       "1997-01-01"^^<http://www.w3.org/2001/XMLSchema#date> ;
        ns5:status          <http://publications.europa.eu/resource/authority/concept-status/CURRENT> ;
        ns5:xlDefinition    []  ;
        ns5:xlNotation      []  ;
        ns5:xlNotation      []  ;
        ns10:op-code        "JAR" ;
        dc:identifier       "JAR" ;
        ns4:created         "2020-05-15"^^<http://www.w3.org/2001/XMLSchema#date> ;
        ns4:dateAccepted    "2020-06-04"^^<http://www.w3.org/2001/XMLSchema#date> ;
        ns4:dateSubmitted   "2020-05-19"^^<http://www.w3.org/2001/XMLSchema#date> ;
        owl:versionInfo     "20200624-0" ;
        skos:definition     "JAR (Java Archive) is an archive file that includes a Java-specific manifest file. It is built on the ZIP format."@en ;
        skos:inScheme       ns10:file-type ;
        skos:prefLabel      "JAR"@en ;
        skos:topConceptOf   ns10:file-type ;
        ns7:altLabel        []  ;
        ns7:prefLabel       []  .

<http://publications.europa.eu/resource/authority/file-type/DEB>
        a                   skos:Concept , ns5:FileType ;
        ns6:context         <http://publications.europa.eu/resource/authority/use-context/IMMC> , <http://publications.europa.eu/resource/authority/use-context/DCAT_AP> ;
        ns9:authority-code  "DEB" ;
        ns9:deprecated      "false" ;
        ns9:op-code         "DEB" ;
        ns9:op-mapped-code  []  ;
        ns9:start.use       "1994-04-01" ;
        ns5:startDate       "1994-04-01"^^<http://www.w3.org/2001/XMLSchema#date> ;
        ns5:status          <http://publications.europa.eu/resource/authority/concept-status/CURRENT> ;
        ns5:xlDefinition    []  ;
        ns5:xlNotation      []  ;
        ns5:xlNotation      []  ;
        ns10:op-code        "DEB" ;
        dc:identifier       "DEB" ;
        ns4:created         "2020-05-15"^^<http://www.w3.org/2001/XMLSchema#date> ;
        ns4:dateAccepted    "2020-06-04"^^<http://www.w3.org/2001/XMLSchema#date> ;
        ns4:dateSubmitted   "2020-05-19"^^<http://www.w3.org/2001/XMLSchema#date> ;
        owl:versionInfo     "20200624-0" ;
        skos:definition     "Debian package is a standard Unix ar archive that includes two tar archives. One archive holds the control information and another contains the installable data."@en ;
        skos:inScheme       ns10:file-type ;
        skos:prefLabel      "deb"@en ;
        skos:topConceptOf   ns10:file-type ;
        ns7:altLabel        []  ;
        ns7:prefLabel       []  .

<http://publications.europa.eu/resource/authority/file-type/BWF>
        a                   skos:Concept , ns5:FileType ;
        ns6:context         <http://publications.europa.eu/resource/authority/use-context/IMMC> ;
        ns9:authority-code  "BWF" ;
        ns9:deprecated      "false" ;
        ns9:op-code         "BWF" ;
        ns9:op-mapped-code  []  ;
        ns9:op-mapped-code  []  ;
        ns9:start.use       "2001-07-01" ;
        ns5:startDate       "2001-07-01"^^<http://www.w3.org/2001/XMLSchema#date> ;
        ns5:status          <http://publications.europa.eu/resource/authority/concept-status/CURRENT> ;
        ns5:xlDefinition    []  ;
        ns5:xlNotation      []  ;
        ns5:xlNotation      []  ;
        ns5:xlNotation      []  ;
        ns10:op-code        "BWF" ;
        dc:identifier       "BWF" ;
        ns4:created         "2016-08-18"^^<http://www.w3.org/2001/XMLSchema#date> ;
        ns4:dateAccepted    "2016-09-09"^^<http://www.w3.org/2001/XMLSchema#date> ;
        ns4:dateSubmitted   "2016-08-22"^^<http://www.w3.org/2001/XMLSchema#date> ;
        owl:versionInfo     "20200624-0" ;
        skos:definition     "BWF – Broadcast Wave Format – is an extension of the Microsoft WAV audio format and is the recording format of most file-based non-linear digital recorders used for motion picture, radio and television production. The purpose of this file format is the addition of metadata to facilitate the seamless exchange of sound data between different computer platforms and applications."@en ;
        skos:inScheme       ns10:file-type ;
        skos:prefLabel      "BWF"@en ;
        skos:topConceptOf   ns10:file-type ;
        ns7:altLabel        []  ;
        ns7:prefLabel       []  .

<http://publications.europa.eu/resource/authority/file-type/RDF>
        a                   skos:Concept , ns5:FileType ;
        ns6:context         <http://publications.europa.eu/resource/authority/use-context/IMMC> , <http://publications.europa.eu/resource/authority/use-context/CELLAR> , <http://publications.europa.eu/resource/authority/use-context/ODP> ;
        ns9:authority-code  "RDF" ;
        ns9:deprecated      "false" ;
        ns9:op-code         "RDF" ;
        ns9:op-mapped-code  []  ;
        ns9:start.use       "2012-09-01" ;
        ns5:startDate       "2012-09-01"^^<http://www.w3.org/2001/XMLSchema#date> ;
        ns5:status          <http://publications.europa.eu/resource/authority/concept-status/CURRENT> ;
        ns5:xlDefinition    []  ;
        ns5:xlNotation      []  ;
        ns5:xlNotation      []  ;
        ns10:op-code        "RDF" ;
        dc:identifier       "RDF" ;
        ns4:created         "2014-03-04"^^<http://www.w3.org/2001/XMLSchema#date> ;
        ns4:dateAccepted    "2014-03-12"^^<http://www.w3.org/2001/XMLSchema#date> ;
        ns4:dateSubmitted   "2014-02-19"^^<http://www.w3.org/2001/XMLSchema#date> ;
        owl:versionInfo     "20200624-0" ;
        skos:definition     "RDF – Resource Description Framework – is a standard model for data interchange on the Web. RDF has features that facilitate data merging. RDF extends the linking structure of the Web to use URIs to name the relationship between things as well as the two ends of the link (this is usually referred to as a ‘triple’). Using this simple model, it allows structured and semi-structured data to be mixed, exposed and shared across different applications. This linking structure forms a directed, labeled graph, where the edges represent the named link between two resources, represented by the graph nodes."@en ;
        skos:inScheme       ns10:file-type ;
        skos:prefLabel      "RDF"@en ;
        skos:topConceptOf   ns10:file-type ;
        ns7:altLabel        []  ;
        ns7:prefLabel       []  .

<http://publications.europa.eu/resource/authority/file-type/JSON_LD>
        a                    ns5:FileType , skos:Concept ;
        ns6:context          <http://publications.europa.eu/resource/authority/use-context/IMMC> , <http://publications.europa.eu/resource/authority/use-context/ODP> , <http://publications.europa.eu/resource/authority/use-context/CELLAR> ;
        ns9:authority-code   "JSON_LD" ;
        ns9:deprecated       "false" ;
        ns9:op-code          "JSON_LD" ;
        ns9:op-mapped-code   []  ;
        ns9:op-mapped-code   []  ;
        ns9:op-mapped-code   []  ;
        ns9:start.use        "2011-12-27" ;
        ns5:machineReadable  true ;
        ns5:nonPropExt       true ;
        ns5:startDate        "2011-12-27"^^<http://www.w3.org/2001/XMLSchema#date> ;
        ns5:status           <http://publications.europa.eu/resource/authority/concept-status/CURRENT> ;
        ns5:xlDefinition     []  ;
        ns5:xlNotation       []  ;
        ns5:xlNotation       []  ;
        ns10:op-code         "JSON_LD" ;
        dc:identifier        "JSON_LD" ;
        ns4:created          "2015-04-07"^^<http://www.w3.org/2001/XMLSchema#date> ;
        ns4:dateSubmitted    "2015-04-22"^^<http://www.w3.org/2001/XMLSchema#date> ;
        owl:versionInfo      "20200624-0" ;
        skos:definition      "JSON-LD is a JSON-based format to serialize Linked Data. It is primarily intended to be a way to use Linked Data in Web-based programming environments, to build interoperable Web services, and to store Linked Data in JSON-based storage engines."@en ;
        skos:inScheme        ns10:file-type ;
        skos:prefLabel       "JSON-LD"@en ;
        skos:topConceptOf    ns10:file-type ;
        ns7:altLabel         []  ;
        ns7:prefLabel        []  .

<http://publications.europa.eu/resource/authority/file-type/ZIP>
        a                   skos:Concept , ns5:FileType ;
        ns6:context         <http://publications.europa.eu/resource/authority/use-context/DCAT_AP> , <http://publications.europa.eu/resource/authority/use-context/OJEEP> , <http://publications.europa.eu/resource/authority/use-context/IMMC> , <http://publications.europa.eu/resource/authority/use-context/ODP> , <http://publications.europa.eu/resource/authority/use-context/EUDOR> , <http://publications.europa.eu/resource/authority/use-context/CELLAR> , <http://publications.europa.eu/resource/authority/use-context/PUB> ;
        ns9:authority-code  "ZIP" ;
        ns9:deprecated      "false" ;
        ns9:op-code         "ZIP" ;
        ns9:op-mapped-code  []  ;
        ns9:op-mapped-code  []  ;
        ns9:op-mapped-code  []  ;
        ns9:op-mapped-code  []  ;
        ns9:op-mapped-code  []  ;
        ns9:op-mapped-code  []  ;
        ns9:op-mapped-code  []  ;
        ns9:start.use       "2012-09-01" ;
        ns5:isTextual       false ;
        ns5:nonPropExt      true ;
        ns5:order           30 ;
        ns5:startDate       "2012-09-01"^^<http://www.w3.org/2001/XMLSchema#date> ;
        ns5:status          <http://publications.europa.eu/resource/authority/concept-status/CURRENT> ;
        ns5:xlDefinition    []  ;
        ns5:xlNotation      []  ;
        ns5:xlNotation      []  ;
        ns5:xlNotation      []  ;
        ns5:xlNotation      []  ;
        ns5:xlNotation      []  ;
        ns10:op-code        "ZIP" ;
        dc:identifier       "ZIP" ;
        ns4:created         "2012-03-19"^^<http://www.w3.org/2001/XMLSchema#date> ;
        ns4:dateAccepted    "2012-11-27"^^<http://www.w3.org/2001/XMLSchema#date> ;
        ns4:dateSubmitted   "2012-09-27"^^<http://www.w3.org/2001/XMLSchema#date> ;
        owl:versionInfo     "20200624-0" ;
        skos:definition     "ZIP is an archive file format that supports lossless data compression. A ZIP file may contain one or more files or directories that may have been compressed."@en ;
        skos:inScheme       ns10:file-type ;
        skos:prefLabel      "ZIP"@en ;
        skos:topConceptOf   ns10:file-type ;
        ns7:altLabel        []  ;
        ns7:prefLabel       []  .

<http://publications.europa.eu/resource/authority/file-type/Z>
        a                   ns5:FileType , skos:Concept ;
        ns6:context         <http://publications.europa.eu/resource/authority/use-context/IMMC> , <http://publications.europa.eu/resource/authority/use-context/DCAT_AP> ;
        ns9:authority-code  "Z" ;
        ns9:deprecated      "false" ;
        ns9:op-code         "Z" ;
        ns9:op-mapped-code  []  ;
        ns9:start.use       "1985-02-01" ;
        ns5:startDate       "1985-02-01"^^<http://www.w3.org/2001/XMLSchema#date> ;
        ns5:status          <http://publications.europa.eu/resource/authority/concept-status/CURRENT> ;
        ns5:xlDefinition    []  ;
        ns5:xlNotation      []  ;
        ns5:xlNotation      []  ;
        ns10:op-code        "Z" ;
        dc:identifier       "Z" ;
        ns4:created         "2020-05-15"^^<http://www.w3.org/2001/XMLSchema#date> ;
        ns4:dateAccepted    "2020-06-04"^^<http://www.w3.org/2001/XMLSchema#date> ;
        ns4:dateSubmitted   "2020-05-19"^^<http://www.w3.org/2001/XMLSchema#date> ;
        owl:versionInfo     "20200624-0" ;
        skos:definition     "Compressed file produced by Unix shell compression program based on the LZW (Lempel-Ziv-Welch) compression algorithm."@en ;
        skos:inScheme       ns10:file-type ;
        skos:prefLabel      "Z"@en ;
        skos:topConceptOf   ns10:file-type ;
        ns7:altLabel        []  ;
        ns7:prefLabel       []  .

<http://publications.europa.eu/resource/authority/file-type/SWM>
        a                   ns5:FileType , skos:Concept ;
        ns6:context         <http://publications.europa.eu/resource/authority/use-context/DCAT_AP> , <http://publications.europa.eu/resource/authority/use-context/IMMC> ;
        ns9:authority-code  "SWM" ;
        ns9:deprecated      "false" ;
        ns9:op-code         "SWM" ;
        ns9:op-mapped-code  []  ;
        ns9:start.use       "2007-01-30" ;
        ns5:startDate       "2007-01-30"^^<http://www.w3.org/2001/XMLSchema#date> ;
        ns5:status          <http://publications.europa.eu/resource/authority/concept-status/CURRENT> ;
        ns5:xlDefinition    []  ;
        ns5:xlNotation      []  ;
        ns5:xlNotation      []  ;
        ns10:op-code        "SWM" ;
        dc:identifier       "SWM" ;
        ns4:created         "2020-05-15"^^<http://www.w3.org/2001/XMLSchema#date> ;
        ns4:dateAccepted    "2020-06-04"^^<http://www.w3.org/2001/XMLSchema#date> ;
        ns4:dateSubmitted   "2020-05-19"^^<http://www.w3.org/2001/XMLSchema#date> ;
        owl:versionInfo     "20200624-0" ;
        skos:definition     "Split WIM file is a Windows Imaging Format file that has been split into multiple parts."@en ;
        skos:inScheme       ns10:file-type ;
        skos:prefLabel      "SWM"@en ;
        skos:topConceptOf   ns10:file-type ;
        ns7:altLabel        []  ;
        ns7:prefLabel       []  .

<http://publications.europa.eu/resource/authority/file-type/ATOM>
        a                   ns5:FileType , skos:Concept ;
        ns6:context         <http://publications.europa.eu/resource/authority/use-context/CELLAR> , <http://publications.europa.eu/resource/authority/use-context/ODP> , <http://publications.europa.eu/resource/authority/use-context/IMMC> ;
        ns9:authority-code  "ATOM" ;
        ns9:deprecated      "false" ;
        ns9:op-code         "ATOM" ;
        ns9:op-mapped-code  []  ;
        ns9:op-mapped-code  []  ;
        ns9:start.use       "2005-12-01" ;
        ns5:startDate       "2005-12-01"^^<http://www.w3.org/2001/XMLSchema#date> ;
        ns5:status          <http://publications.europa.eu/resource/authority/concept-status/CURRENT> ;
        ns5:xlDefinition    []  ;
        ns5:xlNotation      []  ;
        ns5:xlNotation      []  ;
        ns5:xlNotation      []  ;
        ns10:op-code        "ATOM" ;
        dc:identifier       "ATOM" ;
        ns4:created         "2015-04-21"^^<http://www.w3.org/2001/XMLSchema#date> ;
        ns4:dateSubmitted   "2015-04-22"^^<http://www.w3.org/2001/XMLSchema#date> ;
        owl:versionInfo     "20200624-0" ;
        skos:definition     "The Atom Feed or Atom Syndication Format is an XML language used for web feeds. Web feeds allow software programs to check for updates published on a website."@en ;
        skos:inScheme       ns10:file-type ;
        skos:prefLabel      "Atom Feed"@en ;
        skos:topConceptOf   ns10:file-type ;
        ns7:altLabel        []  ;
        ns7:prefLabel       []  .

<http://publications.europa.eu/resource/authority/file-type/WMS_SRVC>
        a                   skos:Concept , ns5:FileType ;
        ns6:context         <http://publications.europa.eu/resource/authority/use-context/IMMC> , <http://publications.europa.eu/resource/authority/use-context/ODP> , <http://publications.europa.eu/resource/authority/use-context/DCAT_AP> ;
        ns9:authority-code  "WMS_SRVC" ;
        ns9:deprecated      "false" ;
        ns9:op-code         "WMS_SRVC" ;
        ns9:op-mapped-code  []  ;
        ns9:start.use       "1999-01-01" ;
        ns5:nonPropExt      true ;
        ns5:startDate       "1999-01-01"^^<http://www.w3.org/2001/XMLSchema#date> ;
        ns5:status          <http://publications.europa.eu/resource/authority/concept-status/CURRENT> ;
        ns5:xlDefinition    []  ;
        ns5:xlNotation      []  ;
        ns5:xlNotation      []  ;
        ns10:op-code        "WMS_SRVC" ;
        dc:identifier       "WMS_SRVC" ;
        ns4:created         "2018-11-12"^^<http://www.w3.org/2001/XMLSchema#date> ;
        ns4:dateAccepted    "2018-11-28"^^<http://www.w3.org/2001/XMLSchema#date> ;
        ns4:dateSubmitted   "2018-11-14"^^<http://www.w3.org/2001/XMLSchema#date> ;
        owl:versionInfo     "20200624-0" ;
        skos:definition     "A Web Map Service (WMS) is a standard protocol developed by the Open Geospatial Consortium (OGC) for serving georeferenced map images over the Internet. These images are typically produced by a map server from data provided by a geographic information system (GIS) database."@en ;
        skos:inScheme       ns10:file-type ;
        skos:prefLabel      "WMS"@en ;
        skos:topConceptOf   ns10:file-type ;
        ns7:altLabel        []  ;
        ns7:prefLabel       []  .

<http://publications.europa.eu/resource/authority/file-type/MSG_HTTP>
        a                   ns5:FileType , skos:Concept ;
        ns6:context         <http://publications.europa.eu/resource/authority/use-context/IMMC> , <http://publications.europa.eu/resource/authority/use-context/CELLAR> ;
        ns9:authority-code  "MSG_HTTP" ;
        ns9:deprecated      "false" ;
        ns9:op-code         "MSG_HTTP" ;
        ns9:start.use       "2014-06-01" ;
        ns5:startDate       "2014-06-01"^^<http://www.w3.org/2001/XMLSchema#date> ;
        ns5:status          <http://publications.europa.eu/resource/authority/concept-status/CURRENT> ;
        ns5:xlDefinition    []  ;
        ns5:xlNotation      []  ;
        ns10:op-code        "MSG_HTTP" ;
        dc:identifier       "MSG_HTTP" ;
        ns4:created         "2015-05-12"^^<http://www.w3.org/2001/XMLSchema#date> ;
        ns4:dateSubmitted   "2015-05-12"^^<http://www.w3.org/2001/XMLSchema#date> ;
        owl:versionInfo     "20200624-0" ;
        skos:definition     "HTTP – Hypertext Transfer Protocol – is a stateless application-level request/response protocol that uses extensible semantics and self-descriptive message payloads for flexible interaction with network-based hypertext information systems. Message Syntax and Routing is part of the HTTP/1.1 specification."@en ;
        skos:inScheme       ns10:file-type ;
        skos:prefLabel      "HTTP Message"@en ;
        skos:topConceptOf   ns10:file-type ;
        ns7:altLabel        []  ;
        ns7:prefLabel       []  .

<http://publications.europa.eu/resource/authority/file-type/SCHEMA_XML>
        a                   ns5:FileType , skos:Concept ;
        ns6:context         <http://publications.europa.eu/resource/authority/use-context/CELLAR> , <http://publications.europa.eu/resource/authority/use-context/ODP> , <http://publications.europa.eu/resource/authority/use-context/IMMC> ;
        ns9:authority-code  "SCHEMA_XML" ;
        ns9:deprecated      "false" ;
        ns9:op-code         "SCHEMA_XML" ;
        ns9:op-mapped-code  []  ;
        ns9:start.use       "2012-09-01" ;
        ns5:startDate       "2012-09-01"^^<http://www.w3.org/2001/XMLSchema#date> ;
        ns5:status          <http://publications.europa.eu/resource/authority/concept-status/CURRENT> ;
        ns5:xlDefinition    []  ;
        ns5:xlNotation      []  ;
        ns5:xlNotation      []  ;
        ns10:op-code        "SCHEMA_XML" ;
        dc:identifier       "SCHEMA_XML" ;
        ns4:created         "2012-09-01"^^<http://www.w3.org/2001/XMLSchema#date> ;
        ns4:dateAccepted    "2014-03-12"^^<http://www.w3.org/2001/XMLSchema#date> ;
        ns4:dateSubmitted   "2014-02-19"^^<http://www.w3.org/2001/XMLSchema#date> ;
        owl:versionInfo     "20200624-0" ;
        skos:definition     "An XML schema is a description of a type of XML document, typically expressed in terms of constraints on the structure and content of documents of that type, above and beyond the basic syntactical constraints imposed by XML itself."@en ;
        skos:inScheme       ns10:file-type ;
        skos:prefLabel      "XML schema"@en ;
        skos:topConceptOf   ns10:file-type ;
        ns7:altLabel        []  ;
        ns7:prefLabel       []  .

<http://publications.europa.eu/resource/authority/file-type/LZO>
        a                   ns5:FileType , skos:Concept ;
        ns6:context         <http://publications.europa.eu/resource/authority/use-context/DCAT_AP> , <http://publications.europa.eu/resource/authority/use-context/IMMC> ;
        ns9:authority-code  "LZO" ;
        ns9:deprecated      "false" ;
        ns9:op-code         "LZO" ;
        ns9:op-mapped-code  []  ;
        ns9:start.use       "1996-01-01" ;
        ns5:startDate       "1996-01-01"^^<http://www.w3.org/2001/XMLSchema#date> ;
        ns5:status          <http://publications.europa.eu/resource/authority/concept-status/CURRENT> ;
        ns5:xlDefinition    []  ;
        ns5:xlNotation      []  ;
        ns5:xlNotation      []  ;
        ns10:op-code        "LZO" ;
        dc:identifier       "LZO" ;
        ns4:created         "2020-05-15"^^<http://www.w3.org/2001/XMLSchema#date> ;
        ns4:dateAccepted    "2020-06-04"^^<http://www.w3.org/2001/XMLSchema#date> ;
        ns4:dateSubmitted   "2020-05-19"^^<http://www.w3.org/2001/XMLSchema#date> ;
        owl:versionInfo     "20200624-0" ;
        skos:definition     "Compressed file produced using LZO (Lempel-Ziv-Oberhumer), a lossless data compression algorithm that is focused on decompression speed."@en ;
        skos:inScheme       ns10:file-type ;
        skos:prefLabel      "lzo"@en ;
        skos:topConceptOf   ns10:file-type ;
        ns7:altLabel        []  ;
        ns7:prefLabel       []  .

<http://publications.europa.eu/resource/authority/file-type/WARC>
        a                   skos:Concept , ns5:FileType ;
        ns6:context         <http://publications.europa.eu/resource/authority/use-context/IMMC> , <http://publications.europa.eu/resource/authority/use-context/CELLAR> ;
        ns9:authority-code  "WARC" ;
        ns9:deprecated      "false" ;
        ns9:op-code         "WARC" ;
        ns9:op-mapped-code  []  ;
        ns9:op-mapped-code  []  ;
        ns9:op-mapped-code  []  ;
        ns9:op-mapped-code  []  ;
        ns9:op-mapped-code  []  ;
        ns9:op-mapped-code  []  ;
        ns9:start.use       "2009-05-15" ;
        ns5:isTextual       false ;
        ns5:order           25 ;
        ns5:startDate       "2009-05-15"^^<http://www.w3.org/2001/XMLSchema#date> ;
        ns5:status          <http://publications.europa.eu/resource/authority/concept-status/CURRENT> ;
        ns5:xlDefinition    []  ;
        ns5:xlNotation      []  ;
        ns5:xlNotation      []  ;
        ns5:xlNotation      []  ;
        ns5:xlNotation      []  ;
        ns5:xlNotation      []  ;
        ns10:op-code        "WARC" ;
        dc:identifier       "WARC" ;
        ns4:created         "2017-05-19"^^<http://www.w3.org/2001/XMLSchema#date> ;
        ns4:dateAccepted    "2017-06-08"^^<http://www.w3.org/2001/XMLSchema#date> ;
        ns4:dateSubmitted   "2017-05-22"^^<http://www.w3.org/2001/XMLSchema#date> ;
        owl:versionInfo     "20200624-0" ;
        skos:definition     "WARC is a web archive format which specifies a method for combining multiple digital resources into an aggregate archive file together with related information."@en ;
        skos:inScheme       ns10:file-type ;
        skos:prefLabel      "WARC"@en ;
        skos:topConceptOf   ns10:file-type ;
        ns7:altLabel        []  ;
        ns7:prefLabel       []  .

<http://publications.europa.eu/resource/authority/file-type/MPEG4_AVC>
        a                   ns5:FileType , skos:Concept ;
        ns6:context         <http://publications.europa.eu/resource/authority/use-context/IMMC> ;
        ns9:authority-code  "MPEG4_AVC" ;
        ns9:deprecated      "false" ;
        ns9:op-code         "MPEG4_AVC" ;
        ns9:op-mapped-code  []  ;
        ns9:op-mapped-code  []  ;
        ns9:op-mapped-code  []  ;
        ns9:start.use       "2003-05-30" ;
        ns5:startDate       "2003-05-30"^^<http://www.w3.org/2001/XMLSchema#date> ;
        ns5:status          <http://publications.europa.eu/resource/authority/concept-status/CURRENT> ;
        ns5:xlDefinition    []  ;
        ns5:xlNotation      []  ;
        ns5:xlNotation      []  ;
        ns5:xlNotation      []  ;
        ns5:xlNotation      []  ;
        ns5:xlNotation      []  ;
        ns5:xlNotation      []  ;
        ns10:op-code        "MPEG4_AVC" ;
        dc:identifier       "MPEG4_AVC" ;
        ns4:created         "2016-08-18"^^<http://www.w3.org/2001/XMLSchema#date> ;
        ns4:dateAccepted    "2016-09-09"^^<http://www.w3.org/2001/XMLSchema#date> ;
        ns4:dateSubmitted   "2016-08-22"^^<http://www.w3.org/2001/XMLSchema#date> ;
        owl:versionInfo     "20200624-0" ;
        skos:definition     "MPEG-4 – Moving Picture Experts Group – Part 10, Advanced Video Coding is a block-oriented motion-compensation-based video compression standard. It is one of the most commonly used formats for the recording, compression and distribution of video content."@en ;
        skos:inScheme       ns10:file-type ;
        skos:prefLabel      "MPEG-4 AVC"@en ;
        skos:topConceptOf   ns10:file-type ;
        ns7:altLabel        []  ;
        ns7:prefLabel       []  .

<http://publications.europa.eu/resource/authority/file-type/SHP>
        a                    ns5:FileType , skos:Concept ;
        ns6:context          <http://publications.europa.eu/resource/authority/use-context/IMMC> , <http://publications.europa.eu/resource/authority/use-context/CELLAR> ;
        ns9:authority-code   "SHP" ;
        ns9:deprecated       "false" ;
        ns9:op-code          "SHP" ;
        ns9:op-mapped-code   []  ;
        ns9:op-mapped-code   []  ;
        ns9:op-mapped-code   []  ;
        ns9:op-mapped-code   []  ;
        ns9:start.use        "1998-07-01" ;
        ns5:machineReadable  true ;
        ns5:startDate        "1998-07-01"^^<http://www.w3.org/2001/XMLSchema#date> ;
        ns5:status           <http://publications.europa.eu/resource/authority/concept-status/CURRENT> ;
        ns5:xlDefinition     []  ;
        ns5:xlNotation       []  ;
        ns5:xlNotation       []  ;
        ns5:xlNotation       []  ;
        ns5:xlNotation       []  ;
        ns10:op-code         "SHP" ;
        dc:identifier        "SHP" ;
        ns4:created          "2015-04-20"^^<http://www.w3.org/2001/XMLSchema#date> ;
        ns4:dateSubmitted    "2015-04-22"^^<http://www.w3.org/2001/XMLSchema#date> ;
        owl:versionInfo      "20200624-0" ;
        skos:definition      "SHP – shapefile format – is a popular geospatial vector data format for geographic information system (GIS) software. Esri shapefile is a zip archive that contains at least the shp, shx and dbf files."@en ;
        skos:inScheme        ns10:file-type ;
        skos:prefLabel       "Esri Shape"@en ;
        skos:topConceptOf    ns10:file-type ;
        ns7:altLabel         []  ;
        ns7:prefLabel        []  .

<http://publications.europa.eu/resource/authority/file-type/PL>
        a                   ns5:FileType , skos:Concept ;
        ns6:context         <http://publications.europa.eu/resource/authority/use-context/ODP> , <http://publications.europa.eu/resource/authority/use-context/IMMC> , <http://publications.europa.eu/resource/authority/use-context/DCAT_AP> ;
        ns9:authority-code  "PL" ;
        ns9:deprecated      "false" ;
        ns9:op-code         "PL" ;
        ns9:op-mapped-code  []  ;
        ns9:op-mapped-code  []  ;
        ns9:op-mapped-code  []  ;
        ns9:op-mapped-code  []  ;
        ns9:start.use       "1987-12-18" ;
        ns5:startDate       "1987-12-18"^^<http://www.w3.org/2001/XMLSchema#date> ;
        ns5:status          <http://publications.europa.eu/resource/authority/concept-status/CURRENT> ;
        ns5:xlDefinition    []  ;
        ns5:xlNotation      []  ;
        ns5:xlNotation      []  ;
        ns5:xlNotation      []  ;
        ns5:xlNotation      []  ;
        ns5:xlNotation      []  ;
        ns10:op-code        "PL" ;
        dc:identifier       "PL" ;
        ns4:created         "2018-11-06"^^<http://www.w3.org/2001/XMLSchema#date> ;
        ns4:dateAccepted    "2018-11-28"^^<http://www.w3.org/2001/XMLSchema#date> ;
        ns4:dateSubmitted   "2018-11-14"^^<http://www.w3.org/2001/XMLSchema#date> ;
        owl:versionInfo     "20200624-0" ;
        skos:definition     "Source code written in the Perl programming language."@en ;
        skos:inScheme       ns10:file-type ;
        skos:prefLabel      "Perl script"@en ;
        skos:topConceptOf   ns10:file-type ;
        ns7:altLabel        []  ;
        ns7:prefLabel       []  .

<http://publications.europa.eu/resource/authority/file-type/RSS>
        a                    skos:Concept , ns5:FileType ;
        ns6:context          <http://publications.europa.eu/resource/authority/use-context/DCAT_AP> , <http://publications.europa.eu/resource/authority/use-context/ODP> , <http://publications.europa.eu/resource/authority/use-context/IMMC> , <http://publications.europa.eu/resource/authority/use-context/CELLAR> ;
        ns9:authority-code   "RSS" ;
        ns9:deprecated       "false" ;
        ns9:op-code          "RSS" ;
        ns9:op-mapped-code   []  ;
        ns9:op-mapped-code   []  ;
        ns9:op-mapped-code   []  ;
        ns9:op-mapped-code   []  ;
        ns9:start.use        "2013-11-27" ;
        ns5:machineReadable  true ;
        ns5:nonPropExt       true ;
        ns5:startDate        "2013-11-27"^^<http://www.w3.org/2001/XMLSchema#date> ;
        ns5:status           <http://publications.europa.eu/resource/authority/concept-status/CURRENT> ;
        ns5:xlDefinition     []  ;
        ns5:xlNotation       []  ;
        ns5:xlNotation       []  ;
        ns5:xlNotation       []  ;
        ns10:op-code         "RSS" ;
        dc:identifier        "RSS" ;
        ns4:created          "2012-09-01"^^<http://www.w3.org/2001/XMLSchema#date> ;
        ns4:dateAccepted     "2014-03-12"^^<http://www.w3.org/2001/XMLSchema#date> ;
        ns4:dateSubmitted    "2014-02-19"^^<http://www.w3.org/2001/XMLSchema#date> ;
        owl:versionInfo      "20200624-0" ;
        skos:definition      "RSS – Rich Site Summary; originally RDF Site Summary; often called Really Simple Syndication – is a type of web feed which allows users to access updates to online content in a standardized, computer-readable format. These feeds can, for example, allow a user to keep track of many different websites in a single news aggregator. Websites usually use RSS feeds to publish frequently updated information, such as blog entries, news headlines, audio, video. An RSS document (called ‘feed’, ‘web feed’ or ‘channel’) includes full or summarized text and metadata."@en ;
        skos:inScheme        ns10:file-type ;
        skos:prefLabel       "RSS feed"@en ;
        skos:topConceptOf    ns10:file-type ;
        ns7:altLabel         []  ;
        ns7:prefLabel        []  .

<http://publications.europa.eu/resource/authority/file-type/LEG>
        a                   skos:Concept , ns5:FileType ;
        ns6:context         <http://publications.europa.eu/resource/authority/use-context/IMMC> ;
        ns9:authority-code  "LEG" ;
        ns9:deprecated      "false" ;
        ns9:op-code         "LEG" ;
        ns9:op-mapped-code  []  ;
        ns9:start.use       "2016-06-01" ;
        ns5:startDate       "2016-06-01"^^<http://www.w3.org/2001/XMLSchema#date> ;
        ns5:status          <http://publications.europa.eu/resource/authority/concept-status/CURRENT> ;
        ns5:xlDefinition    []  ;
        ns5:xlNotation      []  ;
        ns5:xlNotation      []  ;
        ns10:op-code        "LEG" ;
        dc:identifier       "LEG" ;
        ns4:created         "2019-05-08"^^<http://www.w3.org/2001/XMLSchema#date> ;
        ns4:dateAccepted    "2019-06-04"^^<http://www.w3.org/2001/XMLSchema#date> ;
        ns4:dateSubmitted   "2019-05-20"^^<http://www.w3.org/2001/XMLSchema#date> ;
        owl:versionInfo     "20200624-0" ;
        skos:definition     "A ZIP archive file format for files containing an AKN4EU manifestation of a legislative document. It must contain at least an AKN4EU file called \"main.xml\", which always constitutes the entry point, and may contain other associated files and subfolders."@en ;
        skos:inScheme       ns10:file-type ;
        skos:prefLabel      "LEG"@en ;
        skos:topConceptOf   ns10:file-type ;
        ns7:altLabel        []  ;
        ns7:prefLabel       []  .

<http://publications.europa.eu/resource/authority/file-type/LAZ>
        a                   skos:Concept , ns5:FileType ;
        ns6:context         <http://publications.europa.eu/resource/authority/use-context/IMMC> , <http://publications.europa.eu/resource/authority/use-context/CELLAR> ;
        ns9:authority-code  "LAZ" ;
        ns9:deprecated      "false" ;
        ns9:op-code         "LAZ" ;
        ns9:op-mapped-code  []  ;
        ns9:start.use       "2003-05-09" ;
        ns5:startDate       "2003-05-09"^^<http://www.w3.org/2001/XMLSchema#date> ;
        ns5:status          <http://publications.europa.eu/resource/authority/concept-status/CURRENT> ;
        ns5:xlDefinition    []  ;
        ns5:xlNotation      []  ;
        ns5:xlNotation      []  ;
        ns10:op-code        "LAZ" ;
        dc:identifier       "LAZ" ;
        ns4:created         "2015-04-20"^^<http://www.w3.org/2001/XMLSchema#date> ;
        ns4:dateSubmitted   "2015-04-22"^^<http://www.w3.org/2001/XMLSchema#date> ;
        owl:versionInfo     "20200624-0" ;
        skos:definition     "LAZ is the media type which shall be used for compressed LAS files. This media type is incomplete as it lacks a reference to the specification of the format."@en ;
        skos:inScheme       ns10:file-type ;
        skos:prefLabel      "Compressed LAS file"@en ;
        skos:topConceptOf   ns10:file-type ;
        ns7:altLabel        []  ;
        ns7:prefLabel       []  .

<http://publications.europa.eu/resource/authority/file-type/AAC>
        a                   skos:Concept , ns5:FileType ;
        ns6:context         <http://publications.europa.eu/resource/authority/use-context/IMMC> , <http://publications.europa.eu/resource/authority/use-context/DCAT_AP> ;
        ns9:authority-code  "AAC" ;
        ns9:deprecated      "false" ;
        ns9:op-code         "AAC" ;
        ns9:op-mapped-code  []  ;
        ns9:op-mapped-code  []  ;
        ns9:op-mapped-code  []  ;
        ns9:op-mapped-code  []  ;
        ns9:start.use       "1997-01-01" ;
        ns5:startDate       "1997-01-01"^^<http://www.w3.org/2001/XMLSchema#date> ;
        ns5:status          <http://publications.europa.eu/resource/authority/concept-status/CURRENT> ;
        ns5:xlDefinition    []  ;
        ns5:xlNotation      []  ;
        ns5:xlNotation      []  ;
        ns5:xlNotation      []  ;
        ns5:xlNotation      []  ;
        ns5:xlNotation      []  ;
        ns10:op-code        "AAC" ;
        dc:identifier       "AAC" ;
        ns4:created         "2020-05-15"^^<http://www.w3.org/2001/XMLSchema#date> ;
        ns4:dateAccepted    "2020-06-04"^^<http://www.w3.org/2001/XMLSchema#date> ;
        ns4:dateSubmitted   "2020-05-19"^^<http://www.w3.org/2001/XMLSchema#date> ;
        owl:versionInfo     "20200624-0" ;
        skos:definition     "Advanced Audio Coding (AAC) is an audio coding standard for lossy digital audio compression. Designed to be the successor of the MP3 format, AAC generally achieves higher sound quality than MP3 at the same bit rate."@en ;
        skos:inScheme       ns10:file-type ;
        skos:prefLabel      "AAC"@en ;
        skos:topConceptOf   ns10:file-type ;
        ns7:altLabel        []  ;
        ns7:prefLabel       []  .

<http://publications.europa.eu/resource/authority/file-type/LZIP>
        a                   ns5:FileType , skos:Concept ;
        ns6:context         <http://publications.europa.eu/resource/authority/use-context/DCAT_AP> , <http://publications.europa.eu/resource/authority/use-context/IMMC> ;
        ns9:authority-code  "LZIP" ;
        ns9:deprecated      "false" ;
        ns9:op-code         "LZIP" ;
        ns9:op-mapped-code  []  ;
        ns9:start.use       "2008-01-01" ;
        ns5:startDate       "2008-01-01"^^<http://www.w3.org/2001/XMLSchema#date> ;
        ns5:status          <http://publications.europa.eu/resource/authority/concept-status/CURRENT> ;
        ns5:xlDefinition    []  ;
        ns5:xlNotation      []  ;
        ns5:xlNotation      []  ;
        ns10:op-code        "LZIP" ;
        dc:identifier       "LZIP" ;
        ns4:created         "2020-05-15"^^<http://www.w3.org/2001/XMLSchema#date> ;
        ns4:dateAccepted    "2020-06-04"^^<http://www.w3.org/2001/XMLSchema#date> ;
        ns4:dateSubmitted   "2020-05-19"^^<http://www.w3.org/2001/XMLSchema#date> ;
        owl:versionInfo     "20200624-0" ;
        skos:definition     "Compressed file produced by lzip, free, command-line tool for the compression of data that employs the Lempel-Ziv-Markov chain algorithm (LZMA)."@en ;
        skos:inScheme       ns10:file-type ;
        skos:prefLabel      "lzip"@en ;
        skos:topConceptOf   ns10:file-type ;
        ns7:altLabel        []  ;
        ns7:prefLabel       []  .

<http://publications.europa.eu/resource/authority/file-type/OCTET>
        a                   ns5:FileType , skos:Concept ;
        ns6:context         <http://publications.europa.eu/resource/authority/use-context/CELLAR> , <http://publications.europa.eu/resource/authority/use-context/IMMC> , <http://publications.europa.eu/resource/authority/use-context/ODP> ;
        ns9:authority-code  "OCTET" ;
        ns9:deprecated      "false" ;
        ns9:op-code         "OCTET" ;
        ns9:op-mapped-code  []  ;
        ns9:op-mapped-code  []  ;
        ns9:start.use       "1996-11-01" ;
        ns5:startDate       "1996-11-01"^^<http://www.w3.org/2001/XMLSchema#date> ;
        ns5:status          <http://publications.europa.eu/resource/authority/concept-status/CURRENT> ;
        ns5:xlDefinition    []  ;
        ns5:xlNotation      []  ;
        ns5:xlNotation      []  ;
        ns5:xlNotation      []  ;
        ns10:op-code        "OCTET" ;
        dc:identifier       "OCTET" ;
        ns4:created         "2015-04-21"^^<http://www.w3.org/2001/XMLSchema#date> ;
        ns4:dateSubmitted   "2015-04-22"^^<http://www.w3.org/2001/XMLSchema#date> ;
        owl:versionInfo     "20200624-0" ;
        skos:definition     "Octet is the Internet media type for an arbitrary byte stream. A byte streamor octet stream is a series of bytes."@en ;
        skos:inScheme       ns10:file-type ;
        skos:prefLabel      "Octet Stream"@en ;
        skos:topConceptOf   ns10:file-type ;
        ns7:altLabel        []  ;
        ns7:prefLabel       []  .

<http://publications.europa.eu/resource/authority/file-type/DBF>
        a                   skos:Concept , ns5:FileType ;
        ns6:context         <http://publications.europa.eu/resource/authority/use-context/DCAT_AP> , <http://publications.europa.eu/resource/authority/use-context/CELLAR> , <http://publications.europa.eu/resource/authority/use-context/IMMC> , <http://publications.europa.eu/resource/authority/use-context/ODP> ;
        ns9:authority-code  "DBF" ;
        ns9:deprecated      "false" ;
        ns9:op-code         "DBF" ;
        ns9:op-mapped-code  []  ;
        ns9:op-mapped-code  []  ;
        ns9:start.use       "2013-09-18" ;
        ns5:nonPropExt      true ;
        ns5:startDate       "2013-09-18"^^<http://www.w3.org/2001/XMLSchema#date> ;
        ns5:status          <http://publications.europa.eu/resource/authority/concept-status/CURRENT> ;
        ns5:xlDefinition    []  ;
        ns5:xlNotation      []  ;
        ns5:xlNotation      []  ;
        ns10:op-code        "DBF" ;
        dc:identifier       "DBF" ;
        ns4:created         "2013-09-18"^^<http://www.w3.org/2001/XMLSchema#date> ;
        ns4:dateAccepted    "2013-09-26"^^<http://www.w3.org/2001/XMLSchema#date> ;
        ns4:dateSubmitted   "2013-09-26"^^<http://www.w3.org/2001/XMLSchema#date> ;
        owl:versionInfo     "20200624-0" ;
        skos:definition     "DBF – dBase database file – is supported by a number of database products. dBase was one of the first database management systems for microcomputers."@en ;
        skos:inScheme       ns10:file-type ;
        skos:prefLabel      "DBF"@en ;
        skos:topConceptOf   ns10:file-type ;
        ns7:altLabel        []  ;
        ns7:prefLabel       []  .

<http://publications.europa.eu/resource/authority/file-type/TAB>
        a                   skos:Concept , ns5:FileType ;
        ns6:context         <http://publications.europa.eu/resource/authority/use-context/CELLAR> , <http://publications.europa.eu/resource/authority/use-context/IMMC> ;
        ns9:authority-code  "TAB" ;
        ns9:deprecated      "false" ;
        ns9:op-code         "TAB" ;
        ns9:op-mapped-code  []  ;
        ns9:start.use       "2000-03-26" ;
        ns5:startDate       "2000-03-26"^^<http://www.w3.org/2001/XMLSchema#date> ;
        ns5:status          <http://publications.europa.eu/resource/authority/concept-status/CURRENT> ;
        ns5:xlDefinition    []  ;
        ns5:xlNotation      []  ;
        ns5:xlNotation      []  ;
        ns10:op-code        "TAB" ;
        dc:identifier       "TAB" ;
        ns4:created         "2015-04-20"^^<http://www.w3.org/2001/XMLSchema#date> ;
        ns4:dateSubmitted   "2015-04-22"^^<http://www.w3.org/2001/XMLSchema#date> ;
        owl:versionInfo     "20200624-0" ;
        skos:definition     "MapInfo TAB is the media type which shall be used for the MapInfo TAB format. The file is a zip archive that contains at least the tab, dat, map and id files."@en ;
        skos:inScheme       ns10:file-type ;
        skos:prefLabel      "MapInfo TAB file"@en ;
        skos:topConceptOf   ns10:file-type ;
        ns7:altLabel        []  ;
        ns7:prefLabel       []  .

<http://publications.europa.eu/resource/authority/file-type/PWP>
        a                   ns5:FileType , skos:Concept ;
        ns6:context         <http://publications.europa.eu/resource/authority/use-context/IMMC> , <http://publications.europa.eu/resource/authority/use-context/CELLAR> ;
        ns9:authority-code  "PWP" ;
        ns9:deprecated      "false" ;
        ns9:op-code         "PWP" ;
        ns9:start.use       "2017-05-01" ;
        ns5:startDate       "2017-05-01"^^<http://www.w3.org/2001/XMLSchema#date> ;
        ns5:status          <http://publications.europa.eu/resource/authority/concept-status/CURRENT> ;
        ns5:xlDefinition    []  ;
        ns5:xlNotation      []  ;
        ns10:op-code        "PWP" ;
        dc:identifier       "PWP" ;
        ns4:created         "2018-01-05"^^<http://www.w3.org/2001/XMLSchema#date> ;
        ns4:dateAccepted    "2018-03-06"^^<http://www.w3.org/2001/XMLSchema#date> ;
        ns4:dateSubmitted   "2018-02-20"^^<http://www.w3.org/2001/XMLSchema#date> ;
        owl:versionInfo     "20200624-0" ;
        skos:definition     "Transmitting, storing, sharing or archiving a web publication is easier if it can be packaged as a single file. A Web Publication (WP) is a collection of one or more constituent resources, organized together in a uniquely identifiable grouping that may be presented using standard Open Web Platform technologies. A Packaged Web Publication (PWP) is a Web Publication whose constituent resources are combined into a single distributable file, using some standard packaging format."@en ;
        skos:inScheme       ns10:file-type ;
        skos:prefLabel      "PWP"@en ;
        skos:topConceptOf   ns10:file-type ;
        ns7:altLabel        []  ;
        ns7:prefLabel       []  .

<http://publications.europa.eu/resource/authority/file-type/GEOJSON>
        a                    ns5:FileType , skos:Concept ;
        ns6:context          <http://publications.europa.eu/resource/authority/use-context/EUDOR> , <http://publications.europa.eu/resource/authority/use-context/ODP> , <http://publications.europa.eu/resource/authority/use-context/CELLAR> , <http://publications.europa.eu/resource/authority/use-context/IMMC> ;
        ns9:authority-code   "GEOJSON" ;
        ns9:deprecated       "false" ;
        ns9:op-code          "GEOJSON" ;
        ns9:op-mapped-code   []  ;
        ns9:op-mapped-code   []  ;
        ns9:op-mapped-code   []  ;
        ns9:op-mapped-code   []  ;
        ns9:op-mapped-code   []  ;
        ns9:op-mapped-code   []  ;
        ns9:op-mapped-code   []  ;
        ns9:op-mapped-code   []  ;
        ns9:op-mapped-code   []  ;
        ns9:start.use        "2016-08-01" ;
        ns5:isTextual        true ;
        ns5:machineReadable  true ;
        ns5:nonPropExt       true ;
        ns5:order            15 ;
        ns5:startDate        "2016-08-01"^^<http://www.w3.org/2001/XMLSchema#date> ;
        ns5:status           <http://publications.europa.eu/resource/authority/concept-status/CURRENT> ;
        ns5:xlDefinition     []  ;
        ns5:xlNotation       []  ;
        ns5:xlNotation       []  ;
        ns5:xlNotation       []  ;
        ns5:xlNotation       []  ;
        ns5:xlNotation       []  ;
        ns5:xlNotation       []  ;
        ns10:op-code         "GEOJSON" ;
        dc:identifier        "GEOJSON" ;
        ns4:created          "2017-08-25"^^<http://www.w3.org/2001/XMLSchema#date> ;
        ns4:dateAccepted     "2017-09-05"^^<http://www.w3.org/2001/XMLSchema#date> ;
        ns4:dateSubmitted    "2017-08-22"^^<http://www.w3.org/2001/XMLSchema#date> ;
        owl:versionInfo      "20200624-0" ;
        skos:definition      "GeoJSON is an open standard format designed for representing simple geographical features, along with their non-spatial attributes, based on JSON."@en ;
        skos:inScheme        ns10:file-type ;
        skos:prefLabel       "GeoJSON"@en ;
        skos:topConceptOf    ns10:file-type ;
        ns7:altLabel         []  ;
        ns7:prefLabel        []  .

<http://publications.europa.eu/resource/authority/file-type/MBOX>
        a                   skos:Concept , ns5:FileType ;
        ns6:context         <http://publications.europa.eu/resource/authority/use-context/IMMC> ;
        ns9:authority-code  "MBOX" ;
        ns9:deprecated      "false" ;
        ns9:op-code         "MBOX" ;
        ns9:op-mapped-code  []  ;
        ns9:start.use       "2005-09-01" ;
        ns5:startDate       "2005-09-01"^^<http://www.w3.org/2001/XMLSchema#date> ;
        ns5:status          <http://publications.europa.eu/resource/authority/concept-status/CURRENT> ;
        ns5:xlDefinition    []  ;
        ns5:xlNotation      []  ;
        ns5:xlNotation      []  ;
        ns10:op-code        "MBOX" ;
        dc:identifier       "MBOX" ;
        ns4:created         "2016-08-18"^^<http://www.w3.org/2001/XMLSchema#date> ;
        ns4:dateAccepted    "2016-09-09"^^<http://www.w3.org/2001/XMLSchema#date> ;
        ns4:dateSubmitted   "2016-08-22"^^<http://www.w3.org/2001/XMLSchema#date> ;
        owl:versionInfo     "20200624-0" ;
        skos:definition     "MBOX is a generic term for a family of related file formats used for holding collections of email messages. All messages in an mbox mailbox are concatenated and stored as plain text in a single file."@en ;
        skos:inScheme       ns10:file-type ;
        skos:prefLabel      "MBOX"@en ;
        skos:topConceptOf   ns10:file-type ;
        ns7:altLabel        []  ;
        ns7:prefLabel       []  .

<http://publications.europa.eu/resource/authority/file-type/FMX2>
        a                   skos:Concept , ns5:FileType ;
        ns6:context         <http://publications.europa.eu/resource/authority/use-context/ODP> , <http://publications.europa.eu/resource/authority/use-context/EUDOR> , <http://publications.europa.eu/resource/authority/use-context/CELLAR> , <http://publications.europa.eu/resource/authority/use-context/IMMC> ;
        ns9:authority-code  "FMX2" ;
        ns9:deprecated      "true" ;
        ns9:end.use         "1999-03-31" ;
        ns9:op-code         "FMX2" ;
        ns9:op-mapped-code  []  ;
        ns9:op-mapped-code  []  ;
        ns9:op-mapped-code  []  ;
        ns9:op-mapped-code  []  ;
        ns9:op-mapped-code  []  ;
        ns9:op-mapped-code  []  ;
        ns9:op-mapped-code  []  ;
        ns9:start.use       "1989-01-01" ;
        ns5:endDate         "1999-03-31"^^<http://www.w3.org/2001/XMLSchema#date> ;
        ns5:isTextual       true ;
        ns5:order           174 ;
        ns5:startDate       "1989-01-01"^^<http://www.w3.org/2001/XMLSchema#date> ;
        ns5:status          <http://publications.europa.eu/resource/authority/concept-status/DEPRECATED> ;
        ns5:xlDefinition    []  ;
        ns5:xlNotation      []  ;
        ns5:xlNotation      []  ;
        ns5:xlNotation      []  ;
        ns5:xlNotation      []  ;
        ns5:xlNotation      []  ;
        ns5:xlNotation      []  ;
        ns10:op-code        "FMX2" ;
        dc:identifier       "FMX2" ;
        ns4:created         "2012-03-19"^^<http://www.w3.org/2001/XMLSchema#date> ;
        ns4:dateAccepted    "2012-11-27"^^<http://www.w3.org/2001/XMLSchema#date> ;
        ns4:dateSubmitted   "2012-09-27"^^<http://www.w3.org/2001/XMLSchema#date> ;
        owl:versionInfo     "20200624-0" ;
        skos:definition     "Formex describes the format for the exchange of data between the Publication Office and its contractors. In particular, it defines the logical markup for documents which are published in the different series of the Offical Journal of the European Union. Formex 2 was a previous version of Formex actually used."@en ;
        skos:inScheme       ns10:file-type ;
        skos:prefLabel      "Formex 2"@en ;
        skos:topConceptOf   ns10:file-type ;
        ns7:altLabel        []  ;
        ns7:prefLabel       []  .

<http://publications.europa.eu/resource/authority/file-type/HDT>
        a                   ns5:FileType , skos:Concept ;
        ns6:context         <http://publications.europa.eu/resource/authority/use-context/IMMC> ;
        ns9:authority-code  "HDT" ;
        ns9:deprecated      "false" ;
        ns9:op-code         "HDT" ;
        ns9:op-mapped-code  []  ;
        ns9:start.use       "2011-03-30" ;
        ns5:startDate       "2011-03-30"^^<http://www.w3.org/2001/XMLSchema#date> ;
        ns5:status          <http://publications.europa.eu/resource/authority/concept-status/CURRENT> ;
        ns5:xlDefinition    []  ;
        ns5:xlNotation      []  ;
        ns5:xlNotation      []  ;
        ns10:op-code        "HDT" ;
        dc:identifier       "HDT" ;
        ns4:created         "2019-05-08"^^<http://www.w3.org/2001/XMLSchema#date> ;
        ns4:dateAccepted    "2019-06-04"^^<http://www.w3.org/2001/XMLSchema#date> ;
        ns4:dateSubmitted   "2019-05-20"^^<http://www.w3.org/2001/XMLSchema#date> ;
        owl:versionInfo     "20200624-0" ;
        skos:definition     "HDT (Header, Dictionary, Triples) is a compact data structure and binary serialization format for Resource Description Framework (RDF) that keeps big datasets compressed to save space while maintaining search and browse operations without prior decompression."@en ;
        skos:inScheme       ns10:file-type ;
        skos:prefLabel      "HDT"@en ;
        skos:topConceptOf   ns10:file-type ;
        ns7:altLabel        []  ;
        ns7:prefLabel       []  .

<http://publications.europa.eu/resource/authority/file-type/METS_ZIP>
        a                   skos:Concept , ns5:FileType ;
        ns6:context         <http://publications.europa.eu/resource/authority/use-context/CELLAR> , <http://publications.europa.eu/resource/authority/use-context/IMMC> ;
        ns9:authority-code  "METS_ZIP" ;
        ns9:deprecated      "false" ;
        ns9:op-code         "METS_ZIP" ;
        ns9:op-mapped-code  []  ;
        ns9:op-mapped-code  []  ;
        ns9:start.use       "2003-10-27" ;
        ns5:startDate       "2003-10-27"^^<http://www.w3.org/2001/XMLSchema#date> ;
        ns5:status          <http://publications.europa.eu/resource/authority/concept-status/CURRENT> ;
        ns5:xlDefinition    []  ;
        ns5:xlNotation      []  ;
        ns5:xlNotation      []  ;
        ns5:xlNotation      []  ;
        ns10:op-code        "METS_ZIP" ;
        dc:identifier       "METS_ZIP" ;
        ns4:created         "2012-03-19"^^<http://www.w3.org/2001/XMLSchema#date> ;
        ns4:dateSubmitted   "2015-04-22"^^<http://www.w3.org/2001/XMLSchema#date> ;
        owl:versionInfo     "20200624-0" ;
        skos:definition     "METS package is a zip file containing METS XML files."@en ;
        skos:inScheme       ns10:file-type ;
        skos:prefLabel      "METS package"@en ;
        skos:topConceptOf   ns10:file-type ;
        ns7:altLabel        []  ;
        ns7:prefLabel       []  .

<http://publications.europa.eu/resource/authority/file-type/SPARQLQ>
        a                   ns5:FileType , skos:Concept ;
        ns6:context         <http://publications.europa.eu/resource/authority/use-context/CELLAR> , <http://publications.europa.eu/resource/authority/use-context/IMMC> , <http://publications.europa.eu/resource/authority/use-context/ODP> ;
        ns9:authority-code  "SPARQLQ" ;
        ns9:deprecated      "false" ;
        ns9:op-code         "SPARQLQ" ;
        ns9:op-mapped-code  []  ;
        ns9:op-mapped-code  []  ;
        ns9:op-mapped-code  []  ;
        ns9:op-mapped-code  []  ;
        ns9:op-mapped-code  []  ;
        ns9:op-mapped-code  []  ;
        ns9:op-mapped-code  []  ;
        ns9:start.use       "2012-09-01" ;
        ns5:isTextual       true ;
        ns5:order           90 ;
        ns5:startDate       "2012-09-01"^^<http://www.w3.org/2001/XMLSchema#date> ;
        ns5:status          <http://publications.europa.eu/resource/authority/concept-status/CURRENT> ;
        ns5:xlDefinition    []  ;
        ns5:xlNotation      []  ;
        ns5:xlNotation      []  ;
        ns5:xlNotation      []  ;
        ns5:xlNotation      []  ;
        ns5:xlNotation      []  ;
        ns5:xlNotation      []  ;
        ns10:op-code        "SPARQLQ" ;
        dc:identifier       "SPARQLQ" ;
        ns4:created         "2012-03-19"^^<http://www.w3.org/2001/XMLSchema#date> ;
        ns4:dateAccepted    "2012-11-27"^^<http://www.w3.org/2001/XMLSchema#date> ;
        ns4:dateSubmitted   "2012-09-27"^^<http://www.w3.org/2001/XMLSchema#date> ;
        owl:versionInfo     "20200624-0" ;
        skos:definition     "SPARQL – a recursive acronym for SPARQL Protocol and RDF Query Language – is an RDF query language, that is, a semantic query language for databases, able to retrieve and manipulate data stored in Resource Description Framework (RDF) format. It is recognised as one of the key technologies of the semantic web."@en ;
        skos:inScheme       ns10:file-type ;
        skos:prefLabel      "SPARQL"@en ;
        skos:topConceptOf   ns10:file-type ;
        ns7:altLabel        []  ;
        ns7:prefLabel       []  .

<http://publications.europa.eu/resource/authority/file-type/WARC_GZ>
        a                   ns5:FileType , skos:Concept ;
        ns6:context         <http://publications.europa.eu/resource/authority/use-context/CELLAR> , <http://publications.europa.eu/resource/authority/use-context/IMMC> ;
        ns9:authority-code  "WARC_GZ" ;
        ns9:deprecated      "false" ;
        ns9:op-code         "WARC_GZ" ;
        ns9:op-mapped-code  []  ;
        ns9:start.use       "2012-09-01" ;
        ns5:startDate       "2012-09-01"^^<http://www.w3.org/2001/XMLSchema#date> ;
        ns5:status          <http://publications.europa.eu/resource/authority/concept-status/CURRENT> ;
        ns5:xlDefinition    []  ;
        ns5:xlNotation      []  ;
        ns5:xlNotation      []  ;
        ns10:op-code        "WARC_GZ" ;
        dc:identifier       "WARC_GZ" ;
        ns4:created         "2015-12-21"^^<http://www.w3.org/2001/XMLSchema#date> ;
        ns4:dateAccepted    "2016-01-20"^^<http://www.w3.org/2001/XMLSchema#date> ;
        ns4:dateSubmitted   "2016-01-06"^^<http://www.w3.org/2001/XMLSchema#date> ;
        owl:versionInfo     "20200624-0" ;
        skos:definition     "WARC is a web archive format which specifies a method for combining multiple digital resources into an aggregate archive file together with related information. WARC GZ is WARC compressed by GZIP."@en ;
        skos:inScheme       ns10:file-type ;
        skos:prefLabel      "WARC GZ"@en ;
        skos:topConceptOf   ns10:file-type ;
        ns7:altLabel        []  ;
        ns7:prefLabel       []  .

<http://publications.europa.eu/resource/authority/file-type/TAR_GZ>
        a                   ns5:FileType , skos:Concept ;
        ns6:context         <http://publications.europa.eu/resource/authority/use-context/CELLAR> , <http://publications.europa.eu/resource/authority/use-context/IMMC> ;
        ns9:authority-code  "TAR_GZ" ;
        ns9:deprecated      "false" ;
        ns9:op-code         "TAR_GZ" ;
        ns9:op-mapped-code  []  ;
        ns9:start.use       "2012-09-01" ;
        ns5:startDate       "2012-09-01"^^<http://www.w3.org/2001/XMLSchema#date> ;
        ns5:status          <http://publications.europa.eu/resource/authority/concept-status/CURRENT> ;
        ns5:xlDefinition    []  ;
        ns5:xlNotation      []  ;
        ns5:xlNotation      []  ;
        ns10:op-code        "TAR_GZ" ;
        dc:identifier       "TAR_GZ" ;
        ns4:created         "2014-03-04"^^<http://www.w3.org/2001/XMLSchema#date> ;
        ns4:dateAccepted    "2014-03-12"^^<http://www.w3.org/2001/XMLSchema#date> ;
        ns4:dateSubmitted   "2014-02-19"^^<http://www.w3.org/2001/XMLSchema#date> ;
        owl:versionInfo     "20200624-0" ;
        skos:definition     "TAR – tape archive – is a computer software utility for collecting many files into one archive file, often referred to as a tarball, for distribution or backup purposes. GZ – gzip – is a file format and a software application used for file compression and decompression."@en ;
        skos:inScheme       ns10:file-type ;
        skos:prefLabel      "TAR GZ"@en ;
        skos:topConceptOf   ns10:file-type ;
        ns7:altLabel        []  ;
        ns7:prefLabel       []  .

<http://publications.europa.eu/resource/authority/file-type/MSI>
        a                   ns5:FileType , skos:Concept ;
        ns6:context         <http://publications.europa.eu/resource/authority/use-context/IMMC> , <http://publications.europa.eu/resource/authority/use-context/DCAT_AP> ;
        ns9:authority-code  "MSI" ;
        ns9:deprecated      "false" ;
        ns9:op-code         "MSI" ;
        ns9:op-mapped-code  []  ;
        ns9:op-mapped-code  []  ;
        ns9:start.use       "1999-08-31" ;
        ns5:startDate       "1999-08-31"^^<http://www.w3.org/2001/XMLSchema#date> ;
        ns5:status          <http://publications.europa.eu/resource/authority/concept-status/CURRENT> ;
        ns5:xlDefinition    []  ;
        ns5:xlNotation      []  ;
        ns5:xlNotation      []  ;
        ns5:xlNotation      []  ;
        ns10:op-code        "MSI" ;
        dc:identifier       "MSI" ;
        ns4:created         "2020-05-15"^^<http://www.w3.org/2001/XMLSchema#date> ;
        ns4:dateAccepted    "2020-06-04"^^<http://www.w3.org/2001/XMLSchema#date> ;
        ns4:dateSubmitted   "2020-05-19"^^<http://www.w3.org/2001/XMLSchema#date> ;
        owl:versionInfo     "20200624-0" ;
        skos:definition     "Archive file for Windows Installer containing the installation information and an optional .cab file payload."@en ;
        skos:inScheme       ns10:file-type ;
        skos:prefLabel      "MSI"@en ;
        skos:topConceptOf   ns10:file-type ;
        ns7:altLabel        []  ;
        ns7:prefLabel       []  .

<http://publications.europa.eu/resource/authority/file-type/RAR>
        a                   skos:Concept , ns5:FileType ;
        ns6:context         <http://publications.europa.eu/resource/authority/use-context/DCAT_AP> , <http://publications.europa.eu/resource/authority/use-context/IMMC> , <http://publications.europa.eu/resource/authority/use-context/ODP> ;
        ns9:authority-code  "RAR" ;
        ns9:deprecated      "false" ;
        ns9:op-code         "RAR" ;
        ns9:op-mapped-code  []  ;
        ns9:op-mapped-code  []  ;
        ns9:op-mapped-code  []  ;
        ns9:op-mapped-code  []  ;
        ns9:start.use       "1993-03-01" ;
        ns5:startDate       "1993-03-01"^^<http://www.w3.org/2001/XMLSchema#date> ;
        ns5:status          <http://publications.europa.eu/resource/authority/concept-status/CURRENT> ;
        ns5:xlDefinition    []  ;
        ns5:xlNotation      []  ;
        ns5:xlNotation      []  ;
        ns5:xlNotation      []  ;
        ns5:xlNotation      []  ;
        ns5:xlNotation      []  ;
        ns10:op-code        "RAR" ;
        dc:identifier       "RAR" ;
        ns4:created         "2018-11-06"^^<http://www.w3.org/2001/XMLSchema#date> ;
        ns4:dateAccepted    "2018-11-28"^^<http://www.w3.org/2001/XMLSchema#date> ;
        ns4:dateSubmitted   "2018-11-14"^^<http://www.w3.org/2001/XMLSchema#date> ;
        owl:versionInfo     "20200624-0" ;
        skos:definition     "RAR is a proprietary archive file format that supports data compression, error recovery and file spanning."@en ;
        skos:inScheme       ns10:file-type ;
        skos:prefLabel      "RAR"@en ;
        skos:topConceptOf   ns10:file-type ;
        ns7:altLabel        []  ;
        ns7:prefLabel       []  .

<http://publications.europa.eu/resource/authority/file-type/WORLD>
        a                   ns5:FileType , skos:Concept ;
        ns6:context         <http://publications.europa.eu/resource/authority/use-context/CELLAR> , <http://publications.europa.eu/resource/authority/use-context/IMMC> ;
        ns9:authority-code  "WORLD" ;
        ns9:deprecated      "false" ;
        ns9:op-code         "WORLD" ;
        ns9:op-mapped-code  []  ;
        ns9:op-mapped-code  []  ;
        ns9:start.use       "2001-03-26" ;
        ns5:startDate       "2001-03-26"^^<http://www.w3.org/2001/XMLSchema#date> ;
        ns5:status          <http://publications.europa.eu/resource/authority/concept-status/CURRENT> ;
        ns5:xlDefinition    []  ;
        ns5:xlNotation      []  ;
        ns5:xlNotation      []  ;
        ns5:xlNotation      []  ;
        ns10:op-code        "WORLD" ;
        dc:identifier       "WORLD" ;
        ns4:created         "2015-04-20"^^<http://www.w3.org/2001/XMLSchema#date> ;
        ns4:dateSubmitted   "2015-04-22"^^<http://www.w3.org/2001/XMLSchema#date> ;
        owl:versionInfo     "20200624-0" ;
        skos:definition     "A world file is a plain text computer data file used by geographic information systems (GIS) to georeference raster map images. The file extension usually depends on the format of the associated image, e.g. .jgw for JPEG (2000) or .tfw for TIFF."@en ;
        skos:inScheme       ns10:file-type ;
        skos:prefLabel      "World file"@en ;
        skos:topConceptOf   ns10:file-type ;
        ns7:altLabel        []  ;
        ns7:prefLabel       []  .

<http://publications.europa.eu/resource/authority/file-type/REST>
        a                   skos:Concept , ns5:FileType ;
        ns6:context         <http://publications.europa.eu/resource/authority/use-context/IMMC> , <http://publications.europa.eu/resource/authority/use-context/ODP> , <http://publications.europa.eu/resource/authority/use-context/CELLAR> ;
        ns9:authority-code  "REST" ;
        ns9:deprecated      "false" ;
        ns9:op-code         "REST" ;
        ns9:start.use       "2010-01-01" ;
        ns5:startDate       "2010-01-01"^^<http://www.w3.org/2001/XMLSchema#date> ;
        ns5:status          <http://publications.europa.eu/resource/authority/concept-status/CURRENT> ;
        ns5:xlDefinition    []  ;
        ns5:xlNotation      []  ;
        ns10:op-code        "REST" ;
        dc:identifier       "REST" ;
        ns4:created         "2015-04-21"^^<http://www.w3.org/2001/XMLSchema#date> ;
        ns4:dateSubmitted   "2015-04-22"^^<http://www.w3.org/2001/XMLSchema#date> ;
        owl:versionInfo     "20200624-0" ;
        skos:definition     "Esri REST is a standard way for web clients to communicate with geographic information system (GIS) servers through Representational State Transfer (REST) technology."@en ;
        skos:inScheme       ns10:file-type ;
        skos:prefLabel      "Esri REST"@en ;
        skos:topConceptOf   ns10:file-type ;
        ns7:altLabel        []  ;
        ns7:prefLabel       []  .

<http://publications.europa.eu/resource/authority/file-type/PDFA2A>
        a                   skos:Concept , ns5:FileType ;
        ns6:context         <http://publications.europa.eu/resource/authority/use-context/IMMC> ;
        ns9:authority-code  "PDFA2A" ;
        ns9:deprecated      "false" ;
        ns9:op-code         "PDFA2A" ;
        ns9:op-mapped-code  []  ;
        ns9:op-mapped-code  []  ;
        ns9:op-mapped-code  []  ;
        ns9:op-mapped-code  []  ;
        ns9:op-mapped-code  []  ;
        ns9:op-mapped-code  []  ;
        ns9:start.use       "2011-07-01" ;
        ns5:isTextual       false ;
        ns5:order           248 ;
        ns5:startDate       "2011-07-01"^^<http://www.w3.org/2001/XMLSchema#date> ;
        ns5:status          <http://publications.europa.eu/resource/authority/concept-status/CURRENT> ;
        ns5:xlDefinition    []  ;
        ns5:xlNotation      []  ;
        ns5:xlNotation      []  ;
        ns5:xlNotation      []  ;
        ns5:xlNotation      []  ;
        ns5:xlNotation      []  ;
        ns10:op-code        "PDFA2A" ;
        dc:identifier       "PDFA2A" ;
        ns4:created         "2016-08-18"^^<http://www.w3.org/2001/XMLSchema#date> ;
        ns4:dateAccepted    "2016-09-09"^^<http://www.w3.org/2001/XMLSchema#date> ;
        ns4:dateSubmitted   "2016-08-22"^^<http://www.w3.org/2001/XMLSchema#date> ;
        owl:versionInfo     "20200624-0" ;
        skos:definition     "PDF/A-2 is the Part 2 of the PDF standard and specifies three levels of conformance for PDF files. PDF/A-2a corresponds to conformance level a in PDF/A-1 (accessible)."@en ;
        skos:inScheme       ns10:file-type ;
        skos:prefLabel      "PDF/A-2a"@en ;
        skos:topConceptOf   ns10:file-type ;
        ns7:altLabel        []  ;
        ns7:prefLabel       []  .

<http://publications.europa.eu/resource/authority/file-type/TMX>
        a                   ns5:FileType , skos:Concept ;
        ns6:context         <http://publications.europa.eu/resource/authority/use-context/CELLAR> , <http://publications.europa.eu/resource/authority/use-context/IMMC> ;
        ns9:authority-code  "TMX" ;
        ns9:deprecated      "false" ;
        ns9:op-code         "TMX" ;
        ns9:op-mapped-code  []  ;
        ns9:op-mapped-code  []  ;
        ns9:start.use       "1997-11-25" ;
        ns5:startDate       "1997-11-25"^^<http://www.w3.org/2001/XMLSchema#date> ;
        ns5:status          <http://publications.europa.eu/resource/authority/concept-status/CURRENT> ;
        ns5:xlDefinition    []  ;
        ns5:xlNotation      []  ;
        ns5:xlNotation      []  ;
        ns5:xlNotation      []  ;
        ns10:op-code        "TMX" ;
        dc:identifier       "TMX" ;
        ns4:created         "2015-04-20"^^<http://www.w3.org/2001/XMLSchema#date> ;
        ns4:dateSubmitted   "2015-04-22"^^<http://www.w3.org/2001/XMLSchema#date> ;
        owl:versionInfo     "20200624-0" ;
        skos:definition     "TMX – Translation Memory eXchange – is an XML specification for the exchange of translation memory data between computer-aided translation and localization tools with little or no loss of critical data."@en ;
        skos:inScheme       ns10:file-type ;
        skos:prefLabel      "TMX"@en ;
        skos:topConceptOf   ns10:file-type ;
        ns7:altLabel        []  ;
        ns7:prefLabel       []  .

<http://publications.europa.eu/resource/authority/file-type/SB3>
        a                   skos:Concept , ns5:FileType ;
        ns6:context         <http://publications.europa.eu/resource/authority/use-context/IMMC> , <http://publications.europa.eu/resource/authority/use-context/DCAT_AP> ;
        ns9:authority-code  "SB3" ;
        ns9:deprecated      "false" ;
        ns9:op-code         "SB3" ;
        ns9:op-mapped-code  []  ;
        ns9:op-mapped-code  []  ;
        ns9:start.use       "2019-01-02" ;
        ns5:startDate       "2019-01-02"^^<http://www.w3.org/2001/XMLSchema#date> ;
        ns5:status          <http://publications.europa.eu/resource/authority/concept-status/CURRENT> ;
        ns5:xlDefinition    []  ;
        ns5:xlNotation      []  ;
        ns5:xlNotation      []  ;
        ns5:xlNotation      []  ;
        ns10:op-code        "SB3" ;
        dc:identifier       "SB3" ;
        ns4:created         "2020-05-15"^^<http://www.w3.org/2001/XMLSchema#date> ;
        ns4:dateAccepted    "2020-06-04"^^<http://www.w3.org/2001/XMLSchema#date> ;
        ns4:dateSubmitted   "2020-05-19"^^<http://www.w3.org/2001/XMLSchema#date> ;
        owl:versionInfo     "20200624-0" ;
        skos:definition     "Scratch 3.0 is a file format used to store exported Scratch 3.0 projects and sprites. These are ZIP archives which contain information encoded in a text-based JSON format and project media in separate files."@en ;
        skos:inScheme       ns10:file-type ;
        skos:prefLabel      "sb3"@en ;
        skos:topConceptOf   ns10:file-type ;
        ns7:altLabel        []  ;
        ns7:prefLabel       []  .

<http://publications.europa.eu/resource/authority/file-type/RDF_N_QUADS>
        a                    ns5:FileType , skos:Concept ;
        ns6:context          <http://publications.europa.eu/resource/authority/use-context/IMMC> , <http://publications.europa.eu/resource/authority/use-context/ODP> , <http://publications.europa.eu/resource/authority/use-context/CELLAR> ;
        ns9:authority-code   "RDF_N_QUADS" ;
        ns9:deprecated       "false" ;
        ns9:op-code          "RDF_N_QUADS" ;
        ns9:op-mapped-code   []  ;
        ns9:op-mapped-code   []  ;
        ns9:op-mapped-code   []  ;
        ns9:start.use        "2013-04-09" ;
        ns5:machineReadable  true ;
        ns5:nonPropExt       true ;
        ns5:startDate        "2013-04-09"^^<http://www.w3.org/2001/XMLSchema#date> ;
        ns5:status           <http://publications.europa.eu/resource/authority/concept-status/CURRENT> ;
        ns5:xlDefinition     []  ;
        ns5:xlNotation       []  ;
        ns5:xlNotation       []  ;
        ns10:op-code         "RDF_N_QUADS" ;
        dc:identifier        "RDF_N_QUADS" ;
        ns4:created          "2016-02-10"^^<http://www.w3.org/2001/XMLSchema#date> ;
        ns4:dateAccepted     "2016-03-02"^^<http://www.w3.org/2001/XMLSchema#date> ;
        ns4:dateSubmitted    "2016-02-16"^^<http://www.w3.org/2001/XMLSchema#date> ;
        owl:versionInfo      "20200624-0" ;
        skos:definition      "N-Quads is a line-based, plain text format for encoding an RDF dataset. N-quads statements are a sequence of RDF terms representing the subject, predicate, object and graph label of an RDF Triple and the graph it is part of in a dataset."@en ;
        skos:inScheme        ns10:file-type ;
        skos:prefLabel       "RDF N-Quads"@en ;
        skos:topConceptOf    ns10:file-type ;
        ns7:altLabel         []  ;
        ns7:prefLabel        []  .

<http://publications.europa.eu/resource/authority/file-type/XHTML>
        a                   ns5:FileType , skos:Concept ;
        ns6:context         <http://publications.europa.eu/resource/authority/use-context/OJEEP> , <http://publications.europa.eu/resource/authority/use-context/CELLAR> , <http://publications.europa.eu/resource/authority/use-context/IMMC> ;
        ns9:authority-code  "XHTML" ;
        ns9:deprecated      "false" ;
        ns9:op-code         "XHTML" ;
        ns9:op-mapped-code  []  ;
        ns9:op-mapped-code  []  ;
        ns9:op-mapped-code  []  ;
        ns9:op-mapped-code  []  ;
        ns9:op-mapped-code  []  ;
        ns9:op-mapped-code  []  ;
        ns9:op-mapped-code  []  ;
        ns9:op-mapped-code  []  ;
        ns9:op-mapped-code  []  ;
        ns9:start.use       "2012-09-01" ;
        ns5:isTextual       true ;
        ns5:order           360 ;
        ns5:startDate       "2012-09-01"^^<http://www.w3.org/2001/XMLSchema#date> ;
        ns5:status          <http://publications.europa.eu/resource/authority/concept-status/CURRENT> ;
        ns5:xlDefinition    []  ;
        ns5:xlNotation      []  ;
        ns5:xlNotation      []  ;
        ns5:xlNotation      []  ;
        ns5:xlNotation      []  ;
        ns5:xlNotation      []  ;
        ns5:xlNotation      []  ;
        ns5:xlNotation      []  ;
        ns5:xlNotation      []  ;
        ns10:op-code        "XHTML" ;
        dc:identifier       "XHTML" ;
        ns4:created         "2012-03-19"^^<http://www.w3.org/2001/XMLSchema#date> ;
        ns4:dateAccepted    "2012-11-27"^^<http://www.w3.org/2001/XMLSchema#date> ;
        ns4:dateSubmitted   "2012-09-27"^^<http://www.w3.org/2001/XMLSchema#date> ;
        owl:versionInfo     "20200624-0" ;
        skos:definition     "XHTML is a family of current and future document types and modules that reproduce, subset and extend HTML 4. XHTML family document types are XML based."@en ;
        skos:inScheme       ns10:file-type ;
        skos:prefLabel      "XHTML"@en ;
        skos:topConceptOf   ns10:file-type ;
        ns7:altLabel        []  ;
        ns7:prefLabel       []  .

<http://publications.europa.eu/resource/authority/file-type/MOBI>
        a                   skos:Concept , ns5:FileType ;
        ns6:context         <http://publications.europa.eu/resource/authority/use-context/IMMC> , <http://publications.europa.eu/resource/authority/use-context/CELLAR> , <http://publications.europa.eu/resource/authority/use-context/PUB> ;
        ns9:authority-code  "MOBI" ;
        ns9:deprecated      "false" ;
        ns9:op-code         "MOBI" ;
        ns9:op-mapped-code  []  ;
        ns9:op-mapped-code  []  ;
        ns9:op-mapped-code  []  ;
        ns9:op-mapped-code  []  ;
        ns9:op-mapped-code  []  ;
        ns9:op-mapped-code  []  ;
        ns9:op-mapped-code  []  ;
        ns9:start.use       "2012-09-01" ;
        ns5:isTextual       false ;
        ns5:order           160 ;
        ns5:startDate       "2012-09-01"^^<http://www.w3.org/2001/XMLSchema#date> ;
        ns5:status          <http://publications.europa.eu/resource/authority/concept-status/CURRENT> ;
        ns5:xlDefinition    []  ;
        ns5:xlNotation      []  ;
        ns5:xlNotation      []  ;
        ns5:xlNotation      []  ;
        ns5:xlNotation      []  ;
        ns5:xlNotation      []  ;
        ns5:xlNotation      []  ;
        ns10:op-code        "MOBI" ;
        dc:identifier       "MOBI" ;
        ns4:created         "2012-03-19"^^<http://www.w3.org/2001/XMLSchema#date> ;
        ns4:dateAccepted    "2012-11-27"^^<http://www.w3.org/2001/XMLSchema#date> ;
        ns4:dateSubmitted   "2012-09-27"^^<http://www.w3.org/2001/XMLSchema#date> ;
        owl:versionInfo     "20200624-0" ;
        skos:definition     "Mobipocket eBook is a proprietary e-book file format of Mobipocket SA company that can be used by mobile phones, personal digital assistants (PDA) and desktop operating systems."@en ;
        skos:inScheme       ns10:file-type ;
        skos:prefLabel      "Mobipocket eBook"@en ;
        skos:topConceptOf   ns10:file-type ;
        ns7:altLabel        []  ;
        ns7:prefLabel       []  .

<http://publications.europa.eu/resource/authority/file-type/TAR>
        a                   skos:Concept , ns5:FileType ;
        ns6:context         <http://publications.europa.eu/resource/authority/use-context/CELLAR> , <http://publications.europa.eu/resource/authority/use-context/ODP> , <http://publications.europa.eu/resource/authority/use-context/IMMC> ;
        ns9:authority-code  "TAR" ;
        ns9:deprecated      "false" ;
        ns9:op-code         "TAR" ;
        ns9:op-mapped-code  []  ;
        ns9:op-mapped-code  []  ;
        ns9:op-mapped-code  []  ;
        ns9:start.use       "2012-09-01" ;
        ns5:nonPropExt      true ;
        ns5:startDate       "2012-09-01"^^<http://www.w3.org/2001/XMLSchema#date> ;
        ns5:status          <http://publications.europa.eu/resource/authority/concept-status/CURRENT> ;
        ns5:xlDefinition    []  ;
        ns5:xlNotation      []  ;
        ns5:xlNotation      []  ;
        ns5:xlNotation      []  ;
        ns10:op-code        "TAR" ;
        dc:identifier       "TAR" ;
        ns4:created         "2012-09-01"^^<http://www.w3.org/2001/XMLSchema#date> ;
        ns4:dateAccepted    "2014-03-12"^^<http://www.w3.org/2001/XMLSchema#date> ;
        ns4:dateSubmitted   "2014-02-19"^^<http://www.w3.org/2001/XMLSchema#date> ;
        owl:versionInfo     "20200624-0" ;
        skos:definition     "TAR – tape archive – is a computer software utility for collecting many files into one archive file for distribution or backup purposes."@en ;
        skos:inScheme       ns10:file-type ;
        skos:prefLabel      "TAR"@en ;
        skos:topConceptOf   ns10:file-type ;
        ns7:altLabel        []  ;
        ns7:prefLabel       []  .

<http://publications.europa.eu/resource/authority/file-type/LHA>
        a                   ns5:FileType , skos:Concept ;
        ns6:context         <http://publications.europa.eu/resource/authority/use-context/DCAT_AP> , <http://publications.europa.eu/resource/authority/use-context/IMMC> ;
        ns9:authority-code  "LHA" ;
        ns9:deprecated      "false" ;
        ns9:op-code         "LHA" ;
        ns9:op-mapped-code  []  ;
        ns9:op-mapped-code  []  ;
        ns9:start.use       "1988-01-01" ;
        ns5:startDate       "1988-01-01"^^<http://www.w3.org/2001/XMLSchema#date> ;
        ns5:status          <http://publications.europa.eu/resource/authority/concept-status/CURRENT> ;
        ns5:xlDefinition    []  ;
        ns5:xlNotation      []  ;
        ns5:xlNotation      []  ;
        ns5:xlNotation      []  ;
        ns10:op-code        "LHA" ;
        dc:identifier       "LHA" ;
        ns4:created         "2020-05-15"^^<http://www.w3.org/2001/XMLSchema#date> ;
        ns4:dateAccepted    "2020-06-04"^^<http://www.w3.org/2001/XMLSchema#date> ;
        ns4:dateSubmitted   "2020-05-19"^^<http://www.w3.org/2001/XMLSchema#date> ;
        owl:versionInfo     "20200624-0" ;
        skos:definition     "Compressed file produced by LHA, a freeware compression utility."@en ;
        skos:inScheme       ns10:file-type ;
        skos:prefLabel      "LHA"@en ;
        skos:topConceptOf   ns10:file-type ;
        ns7:altLabel        []  ;
        ns7:prefLabel       []  .

<http://publications.europa.eu/resource/authority/file-type/E00>
        a                   ns5:FileType , skos:Concept ;
        ns6:context         <http://publications.europa.eu/resource/authority/use-context/DCAT_AP> , <http://publications.europa.eu/resource/authority/use-context/CELLAR> , <http://publications.europa.eu/resource/authority/use-context/ODP> , <http://publications.europa.eu/resource/authority/use-context/IMMC> ;
        ns9:authority-code  "E00" ;
        ns9:deprecated      "false" ;
        ns9:op-code         "E00" ;
        ns9:op-mapped-code  []  ;
        ns9:start.use       "2013-09-18" ;
        ns5:startDate       "2013-09-18"^^<http://www.w3.org/2001/XMLSchema#date> ;
        ns5:status          <http://publications.europa.eu/resource/authority/concept-status/CURRENT> ;
        ns5:xlDefinition    []  ;
        ns5:xlNotation      []  ;
        ns5:xlNotation      []  ;
        ns10:op-code        "E00" ;
        dc:identifier       "E00" ;
        ns4:created         "2013-09-18"^^<http://www.w3.org/2001/XMLSchema#date> ;
        ns4:dateAccepted    "2013-09-26"^^<http://www.w3.org/2001/XMLSchema#date> ;
        ns4:dateSubmitted   "2013-09-26"^^<http://www.w3.org/2001/XMLSchema#date> ;
        owl:versionInfo     "20200624-0" ;
        skos:definition     "E00 is an ArcInfo interchange file format. ArcInfo is a full-featured geographic information system produced by Esri."@en ;
        skos:inScheme       ns10:file-type ;
        skos:prefLabel      "E00"@en ;
        skos:topConceptOf   ns10:file-type ;
        ns7:altLabel        []  ;
        ns7:prefLabel       []  .

<http://publications.europa.eu/resource/authority/file-type/EPUB>
        a                   ns5:FileType , skos:Concept ;
        ns6:context         <http://publications.europa.eu/resource/authority/use-context/EUDOR> , <http://publications.europa.eu/resource/authority/use-context/PUB> , <http://publications.europa.eu/resource/authority/use-context/ODP> , <http://publications.europa.eu/resource/authority/use-context/CELLAR> , <http://publications.europa.eu/resource/authority/use-context/IMMC> ;
        ns9:authority-code  "EPUB" ;
        ns9:deprecated      "false" ;
        ns9:op-code         "EPUB" ;
        ns9:op-mapped-code  []  ;
        ns9:op-mapped-code  []  ;
        ns9:op-mapped-code  []  ;
        ns9:op-mapped-code  []  ;
        ns9:op-mapped-code  []  ;
        ns9:op-mapped-code  []  ;
        ns9:start.use       "2012-09-01" ;
        ns5:isTextual       false ;
        ns5:order           210 ;
        ns5:startDate       "2012-09-01"^^<http://www.w3.org/2001/XMLSchema#date> ;
        ns5:status          <http://publications.europa.eu/resource/authority/concept-status/CURRENT> ;
        ns5:xlDefinition    []  ;
        ns5:xlNotation      []  ;
        ns5:xlNotation      []  ;
        ns5:xlNotation      []  ;
        ns5:xlNotation      []  ;
        ns5:xlNotation      []  ;
        ns10:op-code        "EPUB" ;
        dc:identifier       "EPUB" ;
        ns4:created         "2012-03-19"^^<http://www.w3.org/2001/XMLSchema#date> ;
        ns4:dateAccepted    "2012-11-27"^^<http://www.w3.org/2001/XMLSchema#date> ;
        ns4:dateSubmitted   "2012-09-27"^^<http://www.w3.org/2001/XMLSchema#date> ;
        owl:versionInfo     "20200624-0" ;
        skos:definition     "EPUB – electronic publication – is an e-book file format that can be downloaded and read on devices like smartphones, tablets, computers or e-readers. It is a technical standard published by the International Digital Publishing Forum (IDPF)."@en ;
        skos:inScheme       ns10:file-type ;
        skos:prefLabel      "EPUB"@en ;
        skos:topConceptOf   ns10:file-type ;
        ns7:altLabel        []  ;
        ns7:prefLabel       []  .

<http://publications.europa.eu/resource/authority/file-type/7Z>
        a                   skos:Concept , ns5:FileType ;
        ns6:context         <http://publications.europa.eu/resource/authority/use-context/DCAT_AP> , <http://publications.europa.eu/resource/authority/use-context/IMMC> ;
        ns9:authority-code  "7Z" ;
        ns9:deprecated      "false" ;
        ns9:op-code         "7Z" ;
        ns9:op-mapped-code  []  ;
        ns9:start.use       "2000-01-01" ;
        ns5:startDate       "2000-01-01"^^<http://www.w3.org/2001/XMLSchema#date> ;
        ns5:status          <http://publications.europa.eu/resource/authority/concept-status/CURRENT> ;
        ns5:xlDefinition    []  ;
        ns5:xlNotation      []  ;
        ns5:xlNotation      []  ;
        ns10:op-code        "7Z" ;
        dc:identifier       "7Z" ;
        ns4:created         "2020-05-15"^^<http://www.w3.org/2001/XMLSchema#date> ;
        ns4:dateAccepted    "2020-06-04"^^<http://www.w3.org/2001/XMLSchema#date> ;
        ns4:dateSubmitted   "2020-05-19"^^<http://www.w3.org/2001/XMLSchema#date> ;
        owl:versionInfo     "20200624-0" ;
        skos:definition     "7z is a compressed archive file format that supports several different data compression, encryption and pre-processing algorithms."@en ;
        skos:inScheme       ns10:file-type ;
        skos:prefLabel      "7z"@en ;
        skos:topConceptOf   ns10:file-type ;
        ns7:altLabel        []  ;
        ns7:prefLabel       []  .

<http://publications.europa.eu/resource/authority/file-type/APK>
        a                   skos:Concept , ns5:FileType ;
        ns6:context         <http://publications.europa.eu/resource/authority/use-context/IMMC> , <http://publications.europa.eu/resource/authority/use-context/DCAT_AP> ;
        ns9:authority-code  "APK" ;
        ns9:deprecated      "false" ;
        ns9:op-code         "APK" ;
        ns9:op-mapped-code  []  ;
        ns9:op-mapped-code  []  ;
        ns9:start.use       "2008-09-23" ;
        ns5:startDate       "2008-09-23"^^<http://www.w3.org/2001/XMLSchema#date> ;
        ns5:status          <http://publications.europa.eu/resource/authority/concept-status/CURRENT> ;
        ns5:xlDefinition    []  ;
        ns5:xlNotation      []  ;
        ns5:xlNotation      []  ;
        ns5:xlNotation      []  ;
        ns10:op-code        "APK" ;
        dc:identifier       "APK" ;
        ns4:created         "2020-05-15"^^<http://www.w3.org/2001/XMLSchema#date> ;
        ns4:dateAccepted    "2020-06-04"^^<http://www.w3.org/2001/XMLSchema#date> ;
        ns4:dateSubmitted   "2020-05-19"^^<http://www.w3.org/2001/XMLSchema#date> ;
        owl:versionInfo     "20200624-0" ;
        skos:definition     "Android Package (APK) is the package file format used by the Android operating system for distribution and installation of mobile apps, mobile games and middleware."@en ;
        skos:inScheme       ns10:file-type ;
        skos:prefLabel      "APK"@en ;
        skos:topConceptOf   ns10:file-type ;
        ns7:altLabel        []  ;
        ns7:prefLabel       []  .

<http://publications.europa.eu/resource/authority/file-type/DTD_SGML>
        a                   skos:Concept , ns5:FileType ;
        ns6:context         <http://publications.europa.eu/resource/authority/use-context/IMMC> , <http://publications.europa.eu/resource/authority/use-context/ODP> , <http://publications.europa.eu/resource/authority/use-context/CELLAR> ;
        ns9:authority-code  "DTD_SGML" ;
        ns9:deprecated      "false" ;
        ns9:op-code         "DTD_SGML" ;
        ns9:op-mapped-code  []  ;
        ns9:op-mapped-code  []  ;
        ns9:start.use       "2012-09-01" ;
        ns5:startDate       "2012-09-01"^^<http://www.w3.org/2001/XMLSchema#date> ;
        ns5:status          <http://publications.europa.eu/resource/authority/concept-status/CURRENT> ;
        ns5:xlDefinition    []  ;
        ns5:xlNotation      []  ;
        ns5:xlNotation      []  ;
        ns5:xlNotation      []  ;
        ns10:op-code        "DTD_SGML" ;
        dc:identifier       "DTD_SGML" ;
        ns4:created         "2012-09-01"^^<http://www.w3.org/2001/XMLSchema#date> ;
        ns4:dateAccepted    "2014-03-12"^^<http://www.w3.org/2001/XMLSchema#date> ;
        ns4:dateSubmitted   "2014-02-19"^^<http://www.w3.org/2001/XMLSchema#date> ;
        owl:versionInfo     "20200624-0" ;
        skos:definition     "SGML – Standard Generalized Markup Language – is a standard for defining generalized markup languages for documents. DTD – document type definition – is a set of markup declarations that define a document type for an SGML-family markup language (SGML, XML, HTML). It defines the legal building blocks of an XML document, the document structure with a list of legal elements and attributes."@en ;
        skos:inScheme       ns10:file-type ;
        skos:prefLabel      "SGML DTD"@en ;
        skos:topConceptOf   ns10:file-type ;
        ns7:altLabel        []  ;
        ns7:prefLabel       []  .

<http://publications.europa.eu/resource/authority/file-type/TSV>
        a                   skos:Concept , ns5:FileType ;
        ns6:context         <http://publications.europa.eu/resource/authority/use-context/ODP> , <http://publications.europa.eu/resource/authority/use-context/CELLAR> , <http://publications.europa.eu/resource/authority/use-context/DCAT_AP> , <http://publications.europa.eu/resource/authority/use-context/IMMC> ;
        ns9:authority-code  "TSV" ;
        ns9:deprecated      "false" ;
        ns9:op-code         "TSV" ;
        ns9:op-mapped-code  []  ;
        ns9:op-mapped-code  []  ;
        ns9:op-mapped-code  []  ;
        ns9:start.use       "2013-10-02" ;
        ns5:nonPropExt      true ;
        ns5:startDate       "2013-10-02"^^<http://www.w3.org/2001/XMLSchema#date> ;
        ns5:status          <http://publications.europa.eu/resource/authority/concept-status/CURRENT> ;
        ns5:xlDefinition    []  ;
        ns5:xlNotation      []  ;
        ns5:xlNotation      []  ;
        ns5:xlNotation      []  ;
        ns10:op-code        "TSV" ;
        dc:identifier       "TSV" ;
        ns4:created         "2013-10-02"^^<http://www.w3.org/2001/XMLSchema#date> ;
        owl:versionInfo     "20200624-0" ;
        skos:definition     "TSV – tab-separated values – files are a simple text format for storing data in a tabular structure, e.g. database table or spreadsheet data, and a way of exchanging information between databases. Each record in the table is one line of the text file. Each field value of a record is separated from the next by a tab character."@en ;
        skos:inScheme       ns10:file-type ;
        skos:prefLabel      "TSV"@en ;
        skos:topConceptOf   ns10:file-type ;
        ns7:altLabel        []  ;
        ns7:prefLabel       []  .

<http://publications.europa.eu/resource/authority/file-type/GDB>
        a                   skos:Concept , ns5:FileType ;
        ns6:context         <http://publications.europa.eu/resource/authority/use-context/CELLAR> , <http://publications.europa.eu/resource/authority/use-context/IMMC> ;
        ns9:authority-code  "GDB" ;
        ns9:deprecated      "false" ;
        ns9:op-code         "GDB" ;
        ns9:op-mapped-code  []  ;
        ns9:start.use       "2008-02-06" ;
        ns5:startDate       "2008-02-06"^^<http://www.w3.org/2001/XMLSchema#date> ;
        ns5:status          <http://publications.europa.eu/resource/authority/concept-status/CURRENT> ;
        ns5:xlDefinition    []  ;
        ns5:xlNotation      []  ;
        ns5:xlNotation      []  ;
        ns10:op-code        "GDB" ;
        dc:identifier       "GDB" ;
        ns4:created         "2015-04-20"^^<http://www.w3.org/2001/XMLSchema#date> ;
        ns4:dateSubmitted   "2015-04-22"^^<http://www.w3.org/2001/XMLSchema#date> ;
        owl:versionInfo     "20200624-0" ;
        skos:definition     "GDB is an Esri's file-based geodatabase format, stored as folders in a file system. It shall be used for Esri file geodatabases. The file is a zip archive that contains the gdb directory."@en ;
        skos:inScheme       ns10:file-type ;
        skos:prefLabel      "Esri File Geodatabase"@en ;
        skos:topConceptOf   ns10:file-type ;
        ns7:altLabel        []  ;
        ns7:prefLabel       []  .

<http://publications.europa.eu/resource/authority/file-type/JPEG2000>
        a                   skos:Concept , ns5:FileType ;
        ns6:context         <http://publications.europa.eu/resource/authority/use-context/IMMC> , <http://publications.europa.eu/resource/authority/use-context/CELLAR> ;
        ns9:authority-code  "JPEG2000" ;
        ns9:deprecated      "false" ;
        ns9:op-code         "JPEG2000" ;
        ns9:op-mapped-code  []  ;
        ns9:op-mapped-code  []  ;
        ns9:op-mapped-code  []  ;
        ns9:start.use       "2000-01-01" ;
        ns5:nonPropExt      true ;
        ns5:startDate       "2000-01-01"^^<http://www.w3.org/2001/XMLSchema#date> ;
        ns5:status          <http://publications.europa.eu/resource/authority/concept-status/CURRENT> ;
        ns5:xlDefinition    []  ;
        ns5:xlNotation      []  ;
        ns5:xlNotation      []  ;
        ns5:xlNotation      []  ;
        ns10:op-code        "JPEG2000" ;
        dc:identifier       "JPEG2000" ;
        ns4:created         "2015-04-20"^^<http://www.w3.org/2001/XMLSchema#date> ;
        ns4:dateSubmitted   "2015-04-22"^^<http://www.w3.org/2001/XMLSchema#date> ;
        owl:versionInfo     "20200624-0" ;
        skos:definition     "JPEG 2000 – Joint Photographic Experts Group 2000 – is an image coding system that uses state-of-the-art compression techniques based on wavelet technology."@en ;
        skos:inScheme       ns10:file-type ;
        skos:prefLabel      "JPEG 2000"@en ;
        skos:topConceptOf   ns10:file-type ;
        ns7:altLabel        []  ;
        ns7:prefLabel       []  .

<http://publications.europa.eu/resource/authority/file-type/WAR>
        a                   skos:Concept , ns5:FileType ;
        ns6:context         <http://publications.europa.eu/resource/authority/use-context/IMMC> , <http://publications.europa.eu/resource/authority/use-context/DCAT_AP> ;
        ns9:authority-code  "WAR" ;
        ns9:deprecated      "false" ;
        ns9:op-code         "WAR" ;
        ns9:op-mapped-code  []  ;
        ns9:start.use       "1999-01-01" ;
        ns5:startDate       "1999-01-01"^^<http://www.w3.org/2001/XMLSchema#date> ;
        ns5:status          <http://publications.europa.eu/resource/authority/concept-status/CURRENT> ;
        ns5:xlDefinition    []  ;
        ns5:xlNotation      []  ;
        ns5:xlNotation      []  ;
        ns10:op-code        "WAR" ;
        dc:identifier       "WAR" ;
        ns4:created         "2020-05-15"^^<http://www.w3.org/2001/XMLSchema#date> ;
        ns4:dateAccepted    "2020-06-04"^^<http://www.w3.org/2001/XMLSchema#date> ;
        ns4:dateSubmitted   "2020-05-19"^^<http://www.w3.org/2001/XMLSchema#date> ;
        owl:versionInfo     "20200624-0" ;
        skos:definition     "A WAR file is used to distribute a collection of JAR-files, JavaServer Pages, Java Servlets, Java classes, XML files, tag libraries, static web pages and other resources that together constitute a web application."@en ;
        skos:inScheme       ns10:file-type ;
        skos:prefLabel      "WAR"@en ;
        skos:topConceptOf   ns10:file-type ;
        ns7:altLabel        []  ;
        ns7:prefLabel       []  .

<http://publications.europa.eu/resource/authority/file-type/JSON>
        a                    ns5:FileType , skos:Concept ;
        ns6:context          <http://publications.europa.eu/resource/authority/use-context/IMMC> , <http://publications.europa.eu/resource/authority/use-context/ODP> , <http://publications.europa.eu/resource/authority/use-context/CELLAR> , <http://publications.europa.eu/resource/authority/use-context/DCAT_AP> ;
        ns9:authority-code   "JSON" ;
        ns9:deprecated       "false" ;
        ns9:op-code          "JSON" ;
        ns9:op-mapped-code   []  ;
        ns9:op-mapped-code   []  ;
        ns9:op-mapped-code   []  ;
        ns9:start.use        "2006-07-01" ;
        ns5:machineReadable  true ;
        ns5:nonPropExt       true ;
        ns5:startDate        "2006-07-01"^^<http://www.w3.org/2001/XMLSchema#date> ;
        ns5:status           <http://publications.europa.eu/resource/authority/concept-status/CURRENT> ;
        ns5:xlDefinition     []  ;
        ns5:xlNotation       []  ;
        ns5:xlNotation       []  ;
        ns10:op-code         "JSON" ;
        dc:identifier        "JSON" ;
        ns4:created          "2013-10-02"^^<http://www.w3.org/2001/XMLSchema#date> ;
        owl:versionInfo      "20200624-0" ;
        skos:definition      "JSON is an open-standard file format that uses human-readable text to transmit data objects consisting of attribute–value pairs and array data types (or any other serializable value). It is a very common data format used for asynchronous browser/server communication."@en ;
        skos:inScheme        ns10:file-type ;
        skos:prefLabel       "JSON"@en ;
        skos:topConceptOf    ns10:file-type ;
        ns7:altLabel         []  ;
        ns7:prefLabel        []  .

<http://publications.europa.eu/resource/authority/file-type/ODT>
        a                   ns5:FileType , skos:Concept ;
        ns6:context         <http://publications.europa.eu/resource/authority/use-context/ODP> , <http://publications.europa.eu/resource/authority/use-context/DCAT_AP> , <http://publications.europa.eu/resource/authority/use-context/IMMC> , <http://publications.europa.eu/resource/authority/use-context/CELLAR> ;
        ns9:authority-code  "ODT" ;
        ns9:deprecated      "false" ;
        ns9:op-code         "ODT" ;
        ns9:op-mapped-code  []  ;
        ns9:op-mapped-code  []  ;
        ns9:start.use       "2012-09-01" ;
        ns5:startDate       "2012-09-01"^^<http://www.w3.org/2001/XMLSchema#date> ;
        ns5:status          <http://publications.europa.eu/resource/authority/concept-status/CURRENT> ;
        ns5:xlDefinition    []  ;
        ns5:xlNotation      []  ;
        ns5:xlNotation      []  ;
        ns5:xlNotation      []  ;
        ns10:op-code        "ODT" ;
        dc:identifier       "ODT" ;
        ns4:created         "2012-09-01"^^<http://www.w3.org/2001/XMLSchema#date> ;
        ns4:dateAccepted    "2014-03-12"^^<http://www.w3.org/2001/XMLSchema#date> ;
        ns4:dateSubmitted   "2014-02-19"^^<http://www.w3.org/2001/XMLSchema#date> ;
        owl:versionInfo     "20200624-0" ;
        skos:definition     "ODT is the word processing file format of OpenDocument, an open standard for electronic documents."@en ;
        skos:inScheme       ns10:file-type ;
        skos:prefLabel      "ODT"@en ;
        skos:topConceptOf   ns10:file-type ;
        ns7:altLabel        []  ;
        ns7:prefLabel       []  .

<http://publications.europa.eu/resource/authority/file-type/MXD>
        a                   skos:Concept , ns5:FileType ;
        ns6:context         <http://publications.europa.eu/resource/authority/use-context/ODP> , <http://publications.europa.eu/resource/authority/use-context/CELLAR> , <http://publications.europa.eu/resource/authority/use-context/IMMC> , <http://publications.europa.eu/resource/authority/use-context/DCAT_AP> ;
        ns9:authority-code  "MXD" ;
        ns9:deprecated      "false" ;
        ns9:op-code         "MXD" ;
        ns9:op-mapped-code  []  ;
        ns9:start.use       "2013-09-18" ;
        ns5:startDate       "2013-09-18"^^<http://www.w3.org/2001/XMLSchema#date> ;
        ns5:status          <http://publications.europa.eu/resource/authority/concept-status/CURRENT> ;
        ns5:xlDefinition    []  ;
        ns5:xlNotation      []  ;
        ns5:xlNotation      []  ;
        ns10:op-code        "MXD" ;
        dc:identifier       "MXD" ;
        ns4:created         "2013-09-18"^^<http://www.w3.org/2001/XMLSchema#date> ;
        ns4:dateAccepted    "2013-09-26"^^<http://www.w3.org/2001/XMLSchema#date> ;
        ns4:dateSubmitted   "2013-09-26"^^<http://www.w3.org/2001/XMLSchema#date> ;
        owl:versionInfo     "20200624-0" ;
        skos:definition     "MXD – Map Exchange Document – is a file format in which the maps created from ArcGIS software can be stored."@en ;
        skos:inScheme       ns10:file-type ;
        skos:prefLabel      "MXD"@en ;
        skos:topConceptOf   ns10:file-type ;
        ns7:altLabel        []  ;
        ns7:prefLabel       []  .

<http://publications.europa.eu/resource/authority/file-type/RDF_N_TRIPLES>
        a                    ns5:FileType , skos:Concept ;
        ns6:context          <http://publications.europa.eu/resource/authority/use-context/IMMC> , <http://publications.europa.eu/resource/authority/use-context/ODP> , <http://publications.europa.eu/resource/authority/use-context/CELLAR> ;
        ns9:authority-code   "RDF_N_TRIPLES" ;
        ns9:deprecated       "false" ;
        ns9:op-code          "RDF_N_TRIPLES" ;
        ns9:op-mapped-code   []  ;
        ns9:op-mapped-code   []  ;
        ns9:op-mapped-code   []  ;
        ns9:op-mapped-code   []  ;
        ns9:op-mapped-code   []  ;
        ns9:op-mapped-code   []  ;
        ns9:op-mapped-code   []  ;
        ns9:start.use        "2008-02-17" ;
        ns5:isTextual        true ;
        ns5:machineReadable  true ;
        ns5:nonPropExt       true ;
        ns5:order            118 ;
        ns5:startDate        "2008-02-17"^^<http://www.w3.org/2001/XMLSchema#date> ;
        ns5:status           <http://publications.europa.eu/resource/authority/concept-status/CURRENT> ;
        ns5:xlDefinition     []  ;
        ns5:xlNotation       []  ;
        ns5:xlNotation       []  ;
        ns5:xlNotation       []  ;
        ns5:xlNotation       []  ;
        ns10:op-code         "RDF_N_TRIPLES" ;
        dc:identifier        "RDF_N_TRIPLES" ;
        ns4:created          "2015-04-07"^^<http://www.w3.org/2001/XMLSchema#date> ;
        ns4:dateSubmitted    "2015-04-22"^^<http://www.w3.org/2001/XMLSchema#date> ;
        owl:versionInfo      "20200624-0" ;
        skos:definition      "RDF N-Tirples is a line-based, plain text format for encoding an RDF graph; a concrete syntax for RDF, an easy to parse line-based subset of Turtle."@en ;
        skos:inScheme        ns10:file-type ;
        skos:prefLabel       "RDF N-Triples"@en ;
        skos:topConceptOf    ns10:file-type ;
        ns7:altLabel         []  ;
        ns7:prefLabel        []  .

<http://publications.europa.eu/resource/authority/file-type/MPEG4>
        a                   ns5:FileType , skos:Concept ;
        ns6:context         <http://publications.europa.eu/resource/authority/use-context/IMMC> ;
        ns9:authority-code  "MPEG4" ;
        ns9:deprecated      "false" ;
        ns9:op-code         "MPEG4" ;
        ns9:op-mapped-code  []  ;
        ns9:op-mapped-code  []  ;
        ns9:op-mapped-code  []  ;
        ns9:start.use       "2001-10-11" ;
        ns5:startDate       "2001-10-11"^^<http://www.w3.org/2001/XMLSchema#date> ;
        ns5:status          <http://publications.europa.eu/resource/authority/concept-status/CURRENT> ;
        ns5:xlDefinition    []  ;
        ns5:xlNotation      []  ;
        ns5:xlNotation      []  ;
        ns5:xlNotation      []  ;
        ns5:xlNotation      []  ;
        ns5:xlNotation      []  ;
        ns5:xlNotation      []  ;
        ns10:op-code        "MPEG4" ;
        dc:identifier       "MPEG4" ;
        ns4:created         "2016-08-18"^^<http://www.w3.org/2001/XMLSchema#date> ;
        ns4:dateAccepted    "2016-09-09"^^<http://www.w3.org/2001/XMLSchema#date> ;
        ns4:dateSubmitted   "2016-08-22"^^<http://www.w3.org/2001/XMLSchema#date> ;
        owl:versionInfo     "20200624-0" ;
        skos:definition     "MPEG-4 – Moving Picture Experts Group – is a method of defining compression of audio and visual (AV) digital data. It was designated a standard for a group of audio and video coding formats and related technology."@en ;
        skos:inScheme       ns10:file-type ;
        skos:prefLabel      "MPEG-4"@en ;
        skos:topConceptOf   ns10:file-type ;
        ns7:altLabel        []  ;
        ns7:prefLabel       []  .

<http://publications.europa.eu/resource/authority/file-type/PSD>
        a                   ns5:FileType , skos:Concept ;
        ns6:context         <http://publications.europa.eu/resource/authority/use-context/IMMC> , <http://publications.europa.eu/resource/authority/use-context/OJEEP> , <http://publications.europa.eu/resource/authority/use-context/CELLAR> ;
        ns9:authority-code  "PSD" ;
        ns9:deprecated      "false" ;
        ns9:op-code         "PSD" ;
        ns9:op-mapped-code  []  ;
        ns9:start.use       "2012-09-01" ;
        ns5:startDate       "2012-09-01"^^<http://www.w3.org/2001/XMLSchema#date> ;
        ns5:status          <http://publications.europa.eu/resource/authority/concept-status/CURRENT> ;
        ns5:xlDefinition    []  ;
        ns5:xlNotation      []  ;
        ns5:xlNotation      []  ;
        ns10:op-code        "PSD" ;
        dc:identifier       "PSD" ;
        ns4:created         "2014-03-04"^^<http://www.w3.org/2001/XMLSchema#date> ;
        ns4:dateAccepted    "2014-03-12"^^<http://www.w3.org/2001/XMLSchema#date> ;
        ns4:dateSubmitted   "2014-02-19"^^<http://www.w3.org/2001/XMLSchema#date> ;
        owl:versionInfo     "20200624-0" ;
        skos:definition     "PSD – Photoshop Document – stores an image with support for most imaging options available in Adobe Photoshop. Photoshop is a raster graphics editor."@en ;
        skos:inScheme       ns10:file-type ;
        skos:prefLabel      "PSD"@en ;
        skos:topConceptOf   ns10:file-type ;
        ns7:altLabel        []  ;
        ns7:prefLabel       []  .

<http://publications.europa.eu/resource/authority/file-type/GML>
        a                   skos:Concept , ns5:FileType ;
        ns6:context         <http://publications.europa.eu/resource/authority/use-context/CELLAR> , <http://publications.europa.eu/resource/authority/use-context/DCAT_AP> , <http://publications.europa.eu/resource/authority/use-context/IMMC> , <http://publications.europa.eu/resource/authority/use-context/ODP> ;
        ns9:authority-code  "GML" ;
        ns9:deprecated      "false" ;
        ns9:op-code         "GML" ;
        ns9:op-mapped-code  []  ;
        ns9:start.use       "2000-05-01" ;
        ns5:startDate       "2000-05-01"^^<http://www.w3.org/2001/XMLSchema#date> ;
        ns5:status          <http://publications.europa.eu/resource/authority/concept-status/CURRENT> ;
        ns5:xlDefinition    []  ;
        ns5:xlNotation      []  ;
        ns5:xlNotation      []  ;
        ns10:op-code        "GML" ;
        dc:identifier       "GML" ;
        ns4:created         "2012-09-01"^^<http://www.w3.org/2001/XMLSchema#date> ;
        ns4:dateAccepted    "2014-03-12"^^<http://www.w3.org/2001/XMLSchema#date> ;
        ns4:dateSubmitted   "2014-02-19"^^<http://www.w3.org/2001/XMLSchema#date> ;
        owl:versionInfo     "20200624-0" ;
        skos:definition     "GML – Geography Markup Language – is the XML grammar defined by the Open Geospatial Consortium (OGC) to express geographical features. GML serves as a modeling language for geographic systems as well as an open interchange format for geographic transactions on the Internet."@en ;
        skos:inScheme       ns10:file-type ;
        skos:prefLabel      "GML"@en ;
        skos:topConceptOf   ns10:file-type ;
        ns7:altLabel        []  ;
        ns7:prefLabel       []  .

<http://publications.europa.eu/resource/authority/file-type/METS>
        a                   ns5:FileType , skos:Concept ;
        ns6:context         <http://publications.europa.eu/resource/authority/use-context/IMMC> , <http://publications.europa.eu/resource/authority/use-context/CELLAR> ;
        ns9:authority-code  "METS" ;
        ns9:deprecated      "false" ;
        ns9:op-code         "METS" ;
        ns9:op-mapped-code  []  ;
        ns9:op-mapped-code  []  ;
        ns9:start.use       "2003-10-27" ;
        ns5:startDate       "2003-10-27"^^<http://www.w3.org/2001/XMLSchema#date> ;
        ns5:status          <http://publications.europa.eu/resource/authority/concept-status/CURRENT> ;
        ns5:xlDefinition    []  ;
        ns5:xlNotation      []  ;
        ns5:xlNotation      []  ;
        ns5:xlNotation      []  ;
        ns10:op-code        "METS" ;
        dc:identifier       "METS" ;
        ns4:created         "2012-03-19"^^<http://www.w3.org/2001/XMLSchema#date> ;
        ns4:dateSubmitted   "2015-04-22"^^<http://www.w3.org/2001/XMLSchema#date> ;
        owl:versionInfo     "20200624-0" ;
        skos:definition     "METS – Metadata Encoding and Transmission Standard – is a metadata standard for encoding descriptive, administrative and structural metadata regarding objects within a digital library, expressed using the XML schema language."@en ;
        skos:inScheme       ns10:file-type ;
        skos:prefLabel      "METS XML"@en ;
        skos:topConceptOf   ns10:file-type ;
        ns7:altLabel        []  ;
        ns7:prefLabel       []  .

<http://publications.europa.eu/resource/authority/file-type/ODG>
        a                   ns5:FileType , skos:Concept ;
        ns6:context         <http://publications.europa.eu/resource/authority/use-context/IMMC> , <http://publications.europa.eu/resource/authority/use-context/CELLAR> , <http://publications.europa.eu/resource/authority/use-context/ODP> ;
        ns9:authority-code  "ODG" ;
        ns9:deprecated      "false" ;
        ns9:op-code         "ODG" ;
        ns9:op-mapped-code  []  ;
        ns9:start.use       "2006-05-31" ;
        ns5:startDate       "2006-05-31"^^<http://www.w3.org/2001/XMLSchema#date> ;
        ns5:status          <http://publications.europa.eu/resource/authority/concept-status/CURRENT> ;
        ns5:xlDefinition    []  ;
        ns5:xlNotation      []  ;
        ns5:xlNotation      []  ;
        ns10:op-code        "ODG" ;
        dc:identifier       "ODG" ;
        ns4:created         "2015-04-21"^^<http://www.w3.org/2001/XMLSchema#date> ;
        ns4:dateSubmitted   "2015-04-22"^^<http://www.w3.org/2001/XMLSchema#date> ;
        owl:versionInfo     "20200624-0" ;
        skos:definition     "OpenDocument is a standardized Open Document Format for Office Applications. Image files are composed of digital data and are used to organize and store digital images."@en ;
        skos:inScheme       ns10:file-type ;
        skos:prefLabel      "OpenDocument Image"@en ;
        skos:topConceptOf   ns10:file-type ;
        ns7:altLabel        []  ;
        ns7:prefLabel       []  .

<http://publications.europa.eu/resource/authority/file-type/ISO>
        a                   ns5:FileType , skos:Concept ;
        ns6:context         <http://publications.europa.eu/resource/authority/use-context/IMMC> ;
        ns9:authority-code  "ISO" ;
        ns9:deprecated      "false" ;
        ns9:op-code         "ISO" ;
        ns9:op-mapped-code  []  ;
        ns9:op-mapped-code  []  ;
        ns9:start.use       "1988-09-01" ;
        ns5:startDate       "1988-09-01"^^<http://www.w3.org/2001/XMLSchema#date> ;
        ns5:status          <http://publications.europa.eu/resource/authority/concept-status/CURRENT> ;
        ns5:xlDefinition    []  ;
        ns5:xlNotation      []  ;
        ns5:xlNotation      []  ;
        ns5:xlNotation      []  ;
        ns10:op-code        "ISO" ;
        dc:identifier       "ISO" ;
        ns4:created         "2018-08-17"^^<http://www.w3.org/2001/XMLSchema#date> ;
        ns4:dateAccepted    "2018-09-12"^^<http://www.w3.org/2001/XMLSchema#date> ;
        ns4:dateSubmitted   "2018-08-29"^^<http://www.w3.org/2001/XMLSchema#date> ;
        owl:versionInfo     "20200624-0" ;
        skos:definition     "Archive file containing the content from (or destined for) an optical disk. Originally it was limited to data formatted to comply with the ISO 9660 standard (1988), hence the format name and the iso file extension. The ISO Disk Image File Format is typically used to package or bundle software, databases, authored DVD video programs, and the like. ISO image files, unlike normal files, are not opened but rather are mounted. ISO image files contain the data contents of every written sector of an optical disc, including the optical disc file system if one is present."@en ;
        skos:inScheme       ns10:file-type ;
        skos:prefLabel      "ISO image"@en ;
        skos:topConceptOf   ns10:file-type ;
        ns7:altLabel        []  ;
        ns7:prefLabel       []  .

<http://publications.europa.eu/resource/authority/file-type/RPM>
        a                   ns5:FileType , skos:Concept ;
        ns6:context         <http://publications.europa.eu/resource/authority/use-context/IMMC> , <http://publications.europa.eu/resource/authority/use-context/DCAT_AP> ;
        ns9:authority-code  "RPM" ;
        ns9:deprecated      "false" ;
        ns9:op-code         "RPM" ;
        ns9:op-mapped-code  []  ;
        ns9:start.use       "1997-01-01" ;
        ns5:startDate       "1997-01-01"^^<http://www.w3.org/2001/XMLSchema#date> ;
        ns5:status          <http://publications.europa.eu/resource/authority/concept-status/CURRENT> ;
        ns5:xlDefinition    []  ;
        ns5:xlNotation      []  ;
        ns5:xlNotation      []  ;
        ns10:op-code        "RPM" ;
        dc:identifier       "RPM" ;
        ns4:created         "2020-05-15"^^<http://www.w3.org/2001/XMLSchema#date> ;
        ns4:dateAccepted    "2020-06-04"^^<http://www.w3.org/2001/XMLSchema#date> ;
        ns4:dateSubmitted   "2020-05-19"^^<http://www.w3.org/2001/XMLSchema#date> ;
        owl:versionInfo     "20200624-0" ;
        skos:definition     "File format for RPM Package Manager (originally Red Hat Package Manager), free and open-source package management system."@en ;
        skos:inScheme       ns10:file-type ;
        skos:prefLabel      "RPM"@en ;
        skos:topConceptOf   ns10:file-type ;
        ns7:altLabel        []  ;
        ns7:prefLabel       []  .

<http://publications.europa.eu/resource/authority/file-type/DMG>
        a                   ns5:FileType , skos:Concept ;
        ns6:context         <http://publications.europa.eu/resource/authority/use-context/DCAT_AP> , <http://publications.europa.eu/resource/authority/use-context/IMMC> ;
        ns9:authority-code  "DMG" ;
        ns9:deprecated      "false" ;
        ns9:op-code         "DMG" ;
        ns9:op-mapped-code  []  ;
        ns9:start.use       "2001-01-01" ;
        ns5:startDate       "2001-01-01"^^<http://www.w3.org/2001/XMLSchema#date> ;
        ns5:status          <http://publications.europa.eu/resource/authority/concept-status/CURRENT> ;
        ns5:xlDefinition    []  ;
        ns5:xlNotation      []  ;
        ns5:xlNotation      []  ;
        ns10:op-code        "DMG" ;
        dc:identifier       "DMG" ;
        ns4:created         "2020-05-15"^^<http://www.w3.org/2001/XMLSchema#date> ;
        ns4:dateAccepted    "2020-06-04"^^<http://www.w3.org/2001/XMLSchema#date> ;
        ns4:dateSubmitted   "2020-05-19"^^<http://www.w3.org/2001/XMLSchema#date> ;
        owl:versionInfo     "20200624-0" ;
        skos:definition     "Apple Disk Image is a disk image format commonly used by the macOS operating system."@en ;
        skos:inScheme       ns10:file-type ;
        skos:prefLabel      "DMG"@en ;
        skos:topConceptOf   ns10:file-type ;
        ns7:altLabel        []  ;
        ns7:prefLabel       []  .

<http://publications.europa.eu/resource/authority/file-type/PDFA1A>
        a                   ns5:FileType , skos:Concept ;
        ns6:context         <http://publications.europa.eu/resource/authority/use-context/PUB> , <http://publications.europa.eu/resource/authority/use-context/CELLAR> , <http://publications.europa.eu/resource/authority/use-context/IMMC> , <http://publications.europa.eu/resource/authority/use-context/EUDOR> ;
        ns9:authority-code  "PDFA1A" ;
        ns9:deprecated      "false" ;
        ns9:op-code         "PDFA1A" ;
        ns9:op-mapped-code  []  ;
        ns9:op-mapped-code  []  ;
        ns9:op-mapped-code  []  ;
        ns9:op-mapped-code  []  ;
        ns9:op-mapped-code  []  ;
        ns9:op-mapped-code  []  ;
        ns9:start.use       "2012-09-01" ;
        ns5:isTextual       false ;
        ns5:order           270 ;
        ns5:startDate       "2012-09-01"^^<http://www.w3.org/2001/XMLSchema#date> ;
        ns5:status          <http://publications.europa.eu/resource/authority/concept-status/CURRENT> ;
        ns5:xlDefinition    []  ;
        ns5:xlNotation      []  ;
        ns5:xlNotation      []  ;
        ns5:xlNotation      []  ;
        ns5:xlNotation      []  ;
        ns5:xlNotation      []  ;
        ns10:op-code        "PDFA1A" ;
        dc:identifier       "PDFA1A" ;
        ns4:created         "2012-03-19"^^<http://www.w3.org/2001/XMLSchema#date> ;
        ns4:dateAccepted    "2012-11-27"^^<http://www.w3.org/2001/XMLSchema#date> ;
        ns4:dateSubmitted   "2012-09-27"^^<http://www.w3.org/2001/XMLSchema#date> ;
        owl:versionInfo     "20200624-0" ;
        skos:definition     "PDF/A-1 is the Part 1 of the PDF standard and specifies two levels of conformance for PDF files. PDF/A-1a – Level A (accessible) conformance was intended to increase the accessibility of conforming files for physically impaired users by allowing assistive software, such as screen readers, to more precisely extract and interpret a file's contents."@en ;
        skos:inScheme       ns10:file-type ;
        skos:prefLabel      "PDF/A-1a"@en ;
        skos:topConceptOf   ns10:file-type ;
        ns7:altLabel        []  ;
        ns7:prefLabel       []  .

<http://publications.europa.eu/resource/authority/file-type/QGS>
        a                   ns5:FileType , skos:Concept ;
        ns6:context         <http://publications.europa.eu/resource/authority/use-context/DCAT_AP> , <http://publications.europa.eu/resource/authority/use-context/IMMC> , <http://publications.europa.eu/resource/authority/use-context/ODP> ;
        ns9:authority-code  "QGS" ;
        ns9:deprecated      "false" ;
        ns9:op-code         "QGS" ;
        ns9:op-mapped-code  []  ;
        ns9:start.use       "2002-07-01" ;
        ns5:startDate       "2002-07-01"^^<http://www.w3.org/2001/XMLSchema#date> ;
        ns5:status          <http://publications.europa.eu/resource/authority/concept-status/CURRENT> ;
        ns5:xlDefinition    []  ;
        ns5:xlNotation      []  ;
        ns5:xlNotation      []  ;
        ns10:op-code        "QGS" ;
        dc:identifier       "QGS" ;
        ns4:created         "2018-11-06"^^<http://www.w3.org/2001/XMLSchema#date> ;
        ns4:dateAccepted    "2018-11-28"^^<http://www.w3.org/2001/XMLSchema#date> ;
        ns4:dateSubmitted   "2018-11-14"^^<http://www.w3.org/2001/XMLSchema#date> ;
        owl:versionInfo     "20200624-0" ;
        skos:definition     "QGS file is a Quantum GIS project. Quantum GIS (QGIS) is a cross-platform free and open source desktop geographic information systems (GIS) application that provides data viewing, editing, and analysis capabilities."@en ;
        skos:inScheme       ns10:file-type ;
        skos:prefLabel      "QGS"@en ;
        skos:topConceptOf   ns10:file-type ;
        ns7:altLabel        []  ;
        ns7:prefLabel       []  .

<http://publications.europa.eu/resource/authority/file-type/RDF_TURTLE>
        a                    skos:Concept , ns5:FileType ;
        ns6:context          <http://publications.europa.eu/resource/authority/use-context/IMMC> , <http://publications.europa.eu/resource/authority/use-context/CELLAR> , <http://publications.europa.eu/resource/authority/use-context/ODP> ;
        ns9:authority-code   "RDF_TURTLE" ;
        ns9:deprecated       "false" ;
        ns9:op-code          "RDF_TURTLE" ;
        ns9:op-mapped-code   []  ;
        ns9:op-mapped-code   []  ;
        ns9:op-mapped-code   []  ;
        ns9:op-mapped-code   []  ;
        ns9:op-mapped-code   []  ;
        ns9:op-mapped-code   []  ;
        ns9:op-mapped-code   []  ;
        ns9:start.use        "2012-09-01" ;
        ns5:isTextual        true ;
        ns5:machineReadable  true ;
        ns5:nonPropExt       true ;
        ns5:order            119 ;
        ns5:startDate        "2012-09-01"^^<http://www.w3.org/2001/XMLSchema#date> ;
        ns5:status           <http://publications.europa.eu/resource/authority/concept-status/CURRENT> ;
        ns5:xlDefinition     []  ;
        ns5:xlNotation       []  ;
        ns5:xlNotation       []  ;
        ns5:xlNotation       []  ;
        ns5:xlNotation       []  ;
        ns10:op-code         "RDF_TURTLE" ;
        dc:identifier        "RDF_TURTLE" ;
        ns4:created          "2012-09-01"^^<http://www.w3.org/2001/XMLSchema#date> ;
        ns4:dateAccepted     "2014-03-12"^^<http://www.w3.org/2001/XMLSchema#date> ;
        ns4:dateSubmitted    "2014-02-19"^^<http://www.w3.org/2001/XMLSchema#date> ;
        owl:versionInfo      "20200624-0" ;
        skos:definition      "Turtle – Terse RDF Triple Language – is a format for expressing data in the Resource Description Framework (RDF) data model with a syntax similar to SPARQL. RDF, in turn, represents information using ‘triples’, each of which consists of a subject, a predicate and an object. Each of those items is expressed as a Web URI."@en ;
        skos:inScheme        ns10:file-type ;
        skos:prefLabel       "RDF Turtle"@en ;
        skos:topConceptOf    ns10:file-type ;
        ns7:altLabel         []  ;
        ns7:prefLabel        []  .

<http://publications.europa.eu/resource/authority/file-type/EPS>
        a                   ns5:FileType , skos:Concept ;
        ns6:context         <http://publications.europa.eu/resource/authority/use-context/CELLAR> , <http://publications.europa.eu/resource/authority/use-context/ODP> , <http://publications.europa.eu/resource/authority/use-context/IMMC> ;
        ns9:authority-code  "EPS" ;
        ns9:deprecated      "false" ;
        ns9:op-code         "EPS" ;
        ns9:op-mapped-code  []  ;
        ns9:op-mapped-code  []  ;
        ns9:start.use       "2012-09-01" ;
        ns5:startDate       "2012-09-01"^^<http://www.w3.org/2001/XMLSchema#date> ;
        ns5:status          <http://publications.europa.eu/resource/authority/concept-status/CURRENT> ;
        ns5:xlDefinition    []  ;
        ns5:xlNotation      []  ;
        ns5:xlNotation      []  ;
        ns5:xlNotation      []  ;
        ns10:op-code        "EPS" ;
        dc:identifier       "EPS" ;
        ns4:created         "2012-09-01"^^<http://www.w3.org/2001/XMLSchema#date> ;
        ns4:dateAccepted    "2014-03-12"^^<http://www.w3.org/2001/XMLSchema#date> ;
        ns4:dateSubmitted   "2014-02-19"^^<http://www.w3.org/2001/XMLSchema#date> ;
        owl:versionInfo     "20200624-0" ;
        skos:definition     "EPS – Encapsulated PostScript – files are more-or-less self-contained, reasonably predictable PostScript documents that describe an image or drawing and can be placed within another PostScript document."@en ;
        skos:inScheme       ns10:file-type ;
        skos:prefLabel      "Encapsulated Postscript"@en ;
        skos:topConceptOf   ns10:file-type ;
        ns7:altLabel        []  ;
        ns7:prefLabel       []  .

<http://publications.europa.eu/resource/authority/file-type/XLSB>
        a                   skos:Concept , ns5:FileType ;
        ns6:context         <http://publications.europa.eu/resource/authority/use-context/IMMC> , <http://publications.europa.eu/resource/authority/use-context/ODP> ;
        ns9:authority-code  "XLSB" ;
        ns9:deprecated      "false" ;
        ns9:op-code         "XLSB" ;
        ns9:op-mapped-code  []  ;
        ns9:start.use       "2007-01-30" ;
        ns5:startDate       "2007-01-30"^^<http://www.w3.org/2001/XMLSchema#date> ;
        ns5:status          <http://publications.europa.eu/resource/authority/concept-status/CURRENT> ;
        ns5:xlDefinition    []  ;
        ns5:xlNotation      []  ;
        ns5:xlNotation      []  ;
        ns10:op-code        "XLSB" ;
        dc:identifier       "XLSB" ;
        ns4:created         "2019-08-05"^^<http://www.w3.org/2001/XMLSchema#date> ;
        ns4:dateAccepted    "2019-08-27"^^<http://www.w3.org/2001/XMLSchema#date> ;
        ns4:dateSubmitted   "2019-08-13"^^<http://www.w3.org/2001/XMLSchema#date> ;
        owl:versionInfo     "20200624-0" ;
        skos:definition     "A file with the XLSB file extension is an Excel Binary Workbook file. They store information in binary format instead of XML like with most other Excel files (like XLSX). Since XLSB files are binary, they can be read from and written to much faster, making them extremely useful for very large spreadsheets."@en ;
        skos:inScheme       ns10:file-type ;
        skos:prefLabel      "XLSB"@en ;
        skos:topConceptOf   ns10:file-type ;
        ns7:altLabel        []  ;
        ns7:prefLabel       []  .

<http://publications.europa.eu/resource/authority/file-type/GZIP>
        a                   ns5:FileType , skos:Concept ;
        ns6:context         <http://publications.europa.eu/resource/authority/use-context/ODP> , <http://publications.europa.eu/resource/authority/use-context/IMMC> , <http://publications.europa.eu/resource/authority/use-context/DCAT_AP> , <http://publications.europa.eu/resource/authority/use-context/CELLAR> ;
        ns9:authority-code  "GZIP" ;
        ns9:deprecated      "false" ;
        ns9:op-code         "GZIP" ;
        ns9:op-mapped-code  []  ;
        ns9:op-mapped-code  []  ;
        ns9:op-mapped-code  []  ;
        ns9:op-mapped-code  []  ;
        ns9:start.use       "2012-09-01" ;
        ns5:nonPropExt      true ;
        ns5:startDate       "2012-09-01"^^<http://www.w3.org/2001/XMLSchema#date> ;
        ns5:status          <http://publications.europa.eu/resource/authority/concept-status/CURRENT> ;
        ns5:xlDefinition    []  ;
        ns5:xlNotation      []  ;
        ns5:xlNotation      []  ;
        ns5:xlNotation      []  ;
        ns5:xlNotation      []  ;
        ns5:xlNotation      []  ;
        ns10:op-code        "GZIP" ;
        dc:identifier       "GZIP" ;
        ns4:created         "2012-03-19"^^<http://www.w3.org/2001/XMLSchema#date> ;
        ns4:dateAccepted    "2013-09-26"^^<http://www.w3.org/2001/XMLSchema#date> ;
        ns4:dateSubmitted   "2013-09-26"^^<http://www.w3.org/2001/XMLSchema#date> ;
        owl:versionInfo     "20200624-0" ;
        skos:definition     "GZIP – GNU zip – is a file format and a software application used for file compression and decompression."@en ;
        skos:inScheme       ns10:file-type ;
        skos:prefLabel      "GNU zip"@en ;
        skos:topConceptOf   ns10:file-type ;
        ns7:altLabel        []  ;
        ns7:prefLabel       []  .

<http://publications.europa.eu/resource/authority/file-type/MDB>
        a                   skos:Concept , ns5:FileType ;
        ns6:context         <http://publications.europa.eu/resource/authority/use-context/CELLAR> , <http://publications.europa.eu/resource/authority/use-context/IMMC> , <http://publications.europa.eu/resource/authority/use-context/DCAT_AP> , <http://publications.europa.eu/resource/authority/use-context/ODP> ;
        ns9:authority-code  "MDB" ;
        ns9:deprecated      "false" ;
        ns9:op-code         "MDB" ;
        ns9:op-mapped-code  []  ;
        ns9:start.use       "2013-09-18" ;
        ns5:startDate       "2013-09-18"^^<http://www.w3.org/2001/XMLSchema#date> ;
        ns5:status          <http://publications.europa.eu/resource/authority/concept-status/CURRENT> ;
        ns5:xlDefinition    []  ;
        ns5:xlNotation      []  ;
        ns5:xlNotation      []  ;
        ns5:xlNotation      []  ;
        ns10:op-code        "MDB" ;
        dc:identifier       "MDB" ;
        ns4:created         "2013-09-18"^^<http://www.w3.org/2001/XMLSchema#date> ;
        ns4:dateAccepted    "2013-09-26"^^<http://www.w3.org/2001/XMLSchema#date> ;
        ns4:dateSubmitted   "2013-09-26"^^<http://www.w3.org/2001/XMLSchema#date> ;
        owl:versionInfo     "20200624-0" ;
        skos:definition     "MDB – Microsoft Database – is a proprietary file format used by 2003 and earlier versions of Microsoft Access. Microsoft Access is a database management system."@en ;
        skos:inScheme       ns10:file-type ;
        skos:prefLabel      "MDB"@en ;
        skos:topConceptOf   ns10:file-type ;
        ns7:altLabel        []  ;
        ns7:prefLabel       []  .

<http://publications.europa.eu/resource/authority/file-type/DOCX>
        a                   skos:Concept , ns5:FileType ;
        ns6:context         <http://publications.europa.eu/resource/authority/use-context/DCAT_AP> , <http://publications.europa.eu/resource/authority/use-context/EUDOR> , <http://publications.europa.eu/resource/authority/use-context/ODP> , <http://publications.europa.eu/resource/authority/use-context/CELLAR> , <http://publications.europa.eu/resource/authority/use-context/OJEEP> , <http://publications.europa.eu/resource/authority/use-context/IMMC> ;
        ns9:authority-code  "DOCX" ;
        ns9:deprecated      "false" ;
        ns9:op-code         "DOCX" ;
        ns9:op-mapped-code  []  ;
        ns9:op-mapped-code  []  ;
        ns9:op-mapped-code  []  ;
        ns9:op-mapped-code  []  ;
        ns9:op-mapped-code  []  ;
        ns9:op-mapped-code  []  ;
        ns9:start.use       "2012-09-01" ;
        ns5:isTextual       false ;
        ns5:order           220 ;
        ns5:startDate       "2012-09-01"^^<http://www.w3.org/2001/XMLSchema#date> ;
        ns5:status          <http://publications.europa.eu/resource/authority/concept-status/CURRENT> ;
        ns5:xlDefinition    []  ;
        ns5:xlNotation      []  ;
        ns5:xlNotation      []  ;
        ns5:xlNotation      []  ;
        ns5:xlNotation      []  ;
        ns5:xlNotation      []  ;
        ns10:op-code        "DOCX" ;
        dc:identifier       "DOCX" ;
        ns4:created         "2012-03-19"^^<http://www.w3.org/2001/XMLSchema#date> ;
        ns4:dateAccepted    "2012-11-27"^^<http://www.w3.org/2001/XMLSchema#date> ;
        ns4:dateSubmitted   "2012-09-27"^^<http://www.w3.org/2001/XMLSchema#date> ;
        owl:versionInfo     "20200624-0" ;
        skos:definition     "DOCX is an Office Open XML international standard for Office documents. It is used by Microsoft Word and by a growing number of applications from other vendors in word processing programs."@en ;
        skos:inScheme       ns10:file-type ;
        skos:prefLabel      "Word DOCX"@en ;
        skos:topConceptOf   ns10:file-type ;
        ns7:altLabel        []  ;
        ns7:prefLabel       []  .

<http://publications.europa.eu/resource/authority/file-type/ECW>
        a                   ns5:FileType , skos:Concept ;
        ns6:context         <http://publications.europa.eu/resource/authority/use-context/IMMC> , <http://publications.europa.eu/resource/authority/use-context/CELLAR> ;
        ns9:authority-code  "ECW" ;
        ns9:deprecated      "false" ;
        ns9:op-code         "ECW" ;
        ns9:op-mapped-code  []  ;
        ns9:start.use       "1998-01-01" ;
        ns5:startDate       "1998-01-01"^^<http://www.w3.org/2001/XMLSchema#date> ;
        ns5:status          <http://publications.europa.eu/resource/authority/concept-status/CURRENT> ;
        ns5:xlDefinition    []  ;
        ns5:xlNotation      []  ;
        ns5:xlNotation      []  ;
        ns10:op-code        "ECW" ;
        dc:identifier       "ECW" ;
        ns4:created         "2015-04-20"^^<http://www.w3.org/2001/XMLSchema#date> ;
        ns4:dateSubmitted   "2015-04-22"^^<http://www.w3.org/2001/XMLSchema#date> ;
        owl:versionInfo     "20200624-0" ;
        skos:definition     "ECW – Enhanced Compressed Wavelet – is the media type which shall be used for a proprietary wavelet compression image format optimized for aerial and satellite imagery."@en ;
        skos:inScheme       ns10:file-type ;
        skos:prefLabel      "ECW"@en ;
        skos:topConceptOf   ns10:file-type ;
        ns7:altLabel        []  ;
        ns7:prefLabel       []  .

<http://publications.europa.eu/resource/authority/file-type/KML>
        a                    ns5:FileType , skos:Concept ;
        ns6:context          <http://publications.europa.eu/resource/authority/use-context/DCAT_AP> , <http://publications.europa.eu/resource/authority/use-context/ODP> , <http://publications.europa.eu/resource/authority/use-context/CELLAR> , <http://publications.europa.eu/resource/authority/use-context/IMMC> ;
        ns9:authority-code   "KML" ;
        ns9:deprecated       "false" ;
        ns9:op-code          "KML" ;
        ns9:op-mapped-code   []  ;
        ns9:op-mapped-code   []  ;
        ns9:op-mapped-code   []  ;
        ns9:start.use        "2013-09-18" ;
        ns5:machineReadable  true ;
        ns5:nonPropExt       true ;
        ns5:startDate        "2013-09-18"^^<http://www.w3.org/2001/XMLSchema#date> ;
        ns5:status           <http://publications.europa.eu/resource/authority/concept-status/CURRENT> ;
        ns5:xlDefinition     []  ;
        ns5:xlNotation       []  ;
        ns5:xlNotation       []  ;
        ns10:op-code         "KML" ;
        dc:identifier        "KML" ;
        ns4:created          "2013-09-18"^^<http://www.w3.org/2001/XMLSchema#date> ;
        ns4:dateAccepted     "2013-09-26"^^<http://www.w3.org/2001/XMLSchema#date> ;
        ns4:dateSubmitted    "2013-09-26"^^<http://www.w3.org/2001/XMLSchema#date> ;
        owl:versionInfo      "20200624-0" ;
        skos:definition      "KML – Keyhole Markup Language – is an XML notation for expressing geographic annotation and visualization within Internet-based, two-dimensional maps and three-dimensional Earth browsers. KML was developed for use with Google Earth and became an international standard."@en ;
        skos:inScheme        ns10:file-type ;
        skos:prefLabel       "KML"@en ;
        skos:topConceptOf    ns10:file-type ;
        ns7:altLabel         []  ;
        ns7:prefLabel        []  .

<http://publications.europa.eu/resource/authority/file-type/LAS>
        a                   skos:Concept , ns5:FileType ;
        ns6:context         <http://publications.europa.eu/resource/authority/use-context/IMMC> , <http://publications.europa.eu/resource/authority/use-context/CELLAR> ;
        ns9:authority-code  "LAS" ;
        ns9:deprecated      "false" ;
        ns9:op-code         "LAS" ;
        ns9:op-mapped-code  []  ;
        ns9:start.use       "2003-05-09" ;
        ns5:startDate       "2003-05-09"^^<http://www.w3.org/2001/XMLSchema#date> ;
        ns5:status          <http://publications.europa.eu/resource/authority/concept-status/CURRENT> ;
        ns5:xlDefinition    []  ;
        ns5:xlNotation      []  ;
        ns5:xlNotation      []  ;
        ns10:op-code        "LAS" ;
        dc:identifier       "LAS" ;
        ns4:created         "2015-04-20"^^<http://www.w3.org/2001/XMLSchema#date> ;
        ns4:dateSubmitted   "2015-04-22"^^<http://www.w3.org/2001/XMLSchema#date> ;
        owl:versionInfo     "20200624-0" ;
        skos:definition     "LAS – LASer file format – is the media type which shall be used for a public file format for the interchange of 3-dimensional point cloud data data between data users."@en ;
        skos:inScheme       ns10:file-type ;
        skos:prefLabel      "LASer file"@en ;
        skos:topConceptOf   ns10:file-type ;
        ns7:altLabel        []  ;
        ns7:prefLabel       []  .

<http://publications.europa.eu/resource/authority/file-type/RDFA>
        a                    skos:Concept , ns5:FileType ;
        ns6:context          <http://publications.europa.eu/resource/authority/use-context/IMMC> , <http://publications.europa.eu/resource/authority/use-context/CELLAR> , <http://publications.europa.eu/resource/authority/use-context/ODP> ;
        ns9:authority-code   "RDFA" ;
        ns9:deprecated       "false" ;
        ns9:op-code          "RDFA" ;
        ns9:op-mapped-code   []  ;
        ns9:op-mapped-code   []  ;
        ns9:start.use        "2006-03-10" ;
        ns5:machineReadable  true ;
        ns5:startDate        "2006-03-10"^^<http://www.w3.org/2001/XMLSchema#date> ;
        ns5:status           <http://publications.europa.eu/resource/authority/concept-status/CURRENT> ;
        ns5:xlDefinition     []  ;
        ns5:xlNotation       []  ;
        ns5:xlNotation       []  ;
        ns10:op-code         "RDFA" ;
        dc:identifier        "RDFA" ;
        ns4:created          "2016-02-10"^^<http://www.w3.org/2001/XMLSchema#date> ;
        ns4:dateAccepted     "2016-03-02"^^<http://www.w3.org/2001/XMLSchema#date> ;
        ns4:dateSubmitted    "2016-02-16"^^<http://www.w3.org/2001/XMLSchema#date> ;
        owl:versionInfo      "20200624-0" ;
        skos:definition      "RDFa is a technique that provides a set of markup attributes to augment the visual information on the Web with machine-readable hints."@en ;
        skos:inScheme        ns10:file-type ;
        skos:prefLabel       "RDFa"@en ;
        skos:topConceptOf    ns10:file-type ;
        ns7:altLabel         []  ;
        ns7:prefLabel        []  .

<http://publications.europa.eu/resource/authority/file-type/TIFF_FX>
        a                   ns5:FileType , skos:Concept ;
        ns6:context         <http://publications.europa.eu/resource/authority/use-context/IMMC> , <http://publications.europa.eu/resource/authority/use-context/CELLAR> ;
        ns9:authority-code  "TIFF_FX" ;
        ns9:deprecated      "false" ;
        ns9:op-code         "TIFF_FX" ;
        ns9:op-mapped-code  []  ;
        ns9:op-mapped-code  []  ;
        ns9:op-mapped-code  []  ;
        ns9:start.use       "2005-02-01" ;
        ns5:startDate       "2005-02-01"^^<http://www.w3.org/2001/XMLSchema#date> ;
        ns5:status          <http://publications.europa.eu/resource/authority/concept-status/CURRENT> ;
        ns5:xlDefinition    []  ;
        ns5:xlNotation      []  ;
        ns5:xlNotation      []  ;
        ns5:xlNotation      []  ;
        ns5:xlNotation      []  ;
        ns10:op-code        "TIFF_FX" ;
        dc:identifier       "TIFF_FX" ;
        ns4:created         "2015-12-03"^^<http://www.w3.org/2001/XMLSchema#date> ;
        ns4:dateAccepted    "2016-01-20"^^<http://www.w3.org/2001/XMLSchema#date> ;
        ns4:dateSubmitted   "2016-01-06"^^<http://www.w3.org/2001/XMLSchema#date> ;
        owl:versionInfo     "20200624-0" ;
        skos:definition     "TIFF-FX is a TIFF-based file format created for fax sendings over the Internet."@en ;
        skos:inScheme       ns10:file-type ;
        skos:prefLabel      "TIFF FX"@en ;
        skos:topConceptOf   ns10:file-type ;
        ns7:altLabel        []  ;
        ns7:prefLabel       []  .

<http://publications.europa.eu/resource/authority/file-type/NETCDF>
        a                    ns5:FileType , skos:Concept ;
        ns6:context          <http://publications.europa.eu/resource/authority/use-context/ODP> , <http://publications.europa.eu/resource/authority/use-context/IMMC> , <http://publications.europa.eu/resource/authority/use-context/CELLAR> ;
        ns9:authority-code   "NETCDF" ;
        ns9:deprecated       "false" ;
        ns9:op-code          "NETCDF" ;
        ns9:op-mapped-code   []  ;
        ns9:op-mapped-code   []  ;
        ns9:op-mapped-code   []  ;
        ns9:op-mapped-code   []  ;
        ns9:op-mapped-code   []  ;
        ns9:start.use        "1990-01-01" ;
        ns5:machineReadable  true ;
        ns5:nonPropExt       true ;
        ns5:startDate        "1990-01-01"^^<http://www.w3.org/2001/XMLSchema#date> ;
        ns5:status           <http://publications.europa.eu/resource/authority/concept-status/CURRENT> ;
        ns5:xlDefinition     []  ;
        ns5:xlNotation       []  ;
        ns5:xlNotation       []  ;
        ns5:xlNotation       []  ;
        ns5:xlNotation       []  ;
        ns10:op-code         "NETCDF" ;
        dc:identifier        "NETCDF" ;
        ns4:created          "2015-04-07"^^<http://www.w3.org/2001/XMLSchema#date> ;
        ns4:dateSubmitted    "2015-04-22"^^<http://www.w3.org/2001/XMLSchema#date> ;
        owl:versionInfo      "20200624-0" ;
        skos:definition      "NetCDF is a set of software libraries and self-describing, machine-independent data formats that support the creation, access and sharing of array-oriented scientific data."@en ;
        skos:inScheme        ns10:file-type ;
        skos:prefLabel       "NetCDF"@en ;
        skos:topConceptOf    ns10:file-type ;
        ns7:altLabel         []  ;
        ns7:prefLabel        []  .

<http://publications.europa.eu/resource/authority/file-type/PNG>
        a                   ns5:FileType , skos:Concept ;
        ns6:context         <http://publications.europa.eu/resource/authority/use-context/IMMC> , <http://publications.europa.eu/resource/authority/use-context/ODP> , <http://publications.europa.eu/resource/authority/use-context/DCAT_AP> , <http://publications.europa.eu/resource/authority/use-context/CELLAR> ;
        ns9:authority-code  "PNG" ;
        ns9:deprecated      "false" ;
        ns9:op-code         "PNG" ;
        ns9:op-mapped-code  []  ;
        ns9:op-mapped-code  []  ;
        ns9:op-mapped-code  []  ;
        ns9:op-mapped-code  []  ;
        ns9:op-mapped-code  []  ;
        ns9:op-mapped-code  []  ;
        ns9:op-mapped-code  []  ;
        ns9:start.use       "2012-09-01" ;
        ns5:isTextual       false ;
        ns5:nonPropExt      true ;
        ns5:order           10 ;
        ns5:startDate       "2012-09-01"^^<http://www.w3.org/2001/XMLSchema#date> ;
        ns5:status          <http://publications.europa.eu/resource/authority/concept-status/CURRENT> ;
        ns5:xlDefinition    []  ;
        ns5:xlNotation      []  ;
        ns5:xlNotation      []  ;
        ns5:xlNotation      []  ;
        ns5:xlNotation      []  ;
        ns5:xlNotation      []  ;
        ns10:op-code        "PNG" ;
        dc:identifier       "PNG" ;
        ns4:created         "2012-03-19"^^<http://www.w3.org/2001/XMLSchema#date> ;
        ns4:dateAccepted    "2012-11-27"^^<http://www.w3.org/2001/XMLSchema#date> ;
        ns4:dateSubmitted   "2012-09-27"^^<http://www.w3.org/2001/XMLSchema#date> ;
        owl:versionInfo     "20200624-0" ;
        skos:definition     "PNG – Portable Network Graphics – is a raster graphics file format that supports lossless data compression. PNG was created as an improved, non-patented replacement for Graphics Interchange Format (GIF), and is the most widely used lossless image compression format on the Internet."@en ;
        skos:inScheme       ns10:file-type ;
        skos:prefLabel      "PNG"@en ;
        skos:topConceptOf   ns10:file-type ;
        ns7:altLabel        []  ;
        ns7:prefLabel       []  .

<http://publications.europa.eu/resource/authority/file-type/PPTX>
        a                   skos:Concept , ns5:FileType ;
        ns6:context         <http://publications.europa.eu/resource/authority/use-context/ODP> , <http://publications.europa.eu/resource/authority/use-context/IMMC> , <http://publications.europa.eu/resource/authority/use-context/OJEEP> , <http://publications.europa.eu/resource/authority/use-context/DCAT_AP> , <http://publications.europa.eu/resource/authority/use-context/CELLAR> ;
        ns9:authority-code  "PPTX" ;
        ns9:deprecated      "false" ;
        ns9:op-code         "PPTX" ;
        ns9:op-mapped-code  []  ;
        ns9:op-mapped-code  []  ;
        ns9:op-mapped-code  []  ;
        ns9:op-mapped-code  []  ;
        ns9:op-mapped-code  []  ;
        ns9:op-mapped-code  []  ;
        ns9:start.use       "2012-09-01" ;
        ns5:isTextual       false ;
        ns5:order           130 ;
        ns5:startDate       "2012-09-01"^^<http://www.w3.org/2001/XMLSchema#date> ;
        ns5:status          <http://publications.europa.eu/resource/authority/concept-status/CURRENT> ;
        ns5:xlDefinition    []  ;
        ns5:xlNotation      []  ;
        ns5:xlNotation      []  ;
        ns5:xlNotation      []  ;
        ns5:xlNotation      []  ;
        ns5:xlNotation      []  ;
        ns10:op-code        "PPTX" ;
        dc:identifier       "PPTX" ;
        ns4:created         "2012-03-19"^^<http://www.w3.org/2001/XMLSchema#date> ;
        ns4:dateAccepted    "2012-11-27"^^<http://www.w3.org/2001/XMLSchema#date> ;
        ns4:dateSubmitted   "2012-09-27"^^<http://www.w3.org/2001/XMLSchema#date> ;
        owl:versionInfo     "20200624-0" ;
        skos:definition     "PPTX – PowerPoint 2007 XML presentation – is an XML filename extension of Office Open XML version of Microsoft PowerPoint presentation program. PowerPoint was originally designed to provide visuals for group presentations within business organizations, but has come to be very widely used in many other communication situations, both in business and beyond."@en ;
        skos:inScheme       ns10:file-type ;
        skos:prefLabel      "PowerPoint PPTX"@en ;
        skos:topConceptOf   ns10:file-type ;
        ns7:altLabel        []  ;
        ns7:prefLabel       []  .

<http://publications.europa.eu/resource/authority/file-type/ODB>
        a                   ns5:FileType , skos:Concept ;
        ns6:context         <http://publications.europa.eu/resource/authority/use-context/IMMC> , <http://publications.europa.eu/resource/authority/use-context/ODP> , <http://publications.europa.eu/resource/authority/use-context/CELLAR> ;
        ns9:authority-code  "ODB" ;
        ns9:deprecated      "false" ;
        ns9:op-code         "ODB" ;
        ns9:op-mapped-code  []  ;
        ns9:start.use       "2009-01-16" ;
        ns5:startDate       "2009-01-16"^^<http://www.w3.org/2001/XMLSchema#date> ;
        ns5:status          <http://publications.europa.eu/resource/authority/concept-status/CURRENT> ;
        ns5:xlDefinition    []  ;
        ns5:xlNotation      []  ;
        ns5:xlNotation      []  ;
        ns10:op-code        "ODB" ;
        dc:identifier       "ODB" ;
        ns4:created         "2015-04-21"^^<http://www.w3.org/2001/XMLSchema#date> ;
        ns4:dateSubmitted   "2015-04-22"^^<http://www.w3.org/2001/XMLSchema#date> ;
        owl:versionInfo     "20200624-0" ;
        skos:definition     "OpenDocument is a standardized Open Document Format for Office Applications. Databases are organized collections of data."@en ;
        skos:inScheme       ns10:file-type ;
        skos:prefLabel      "OpenDocument Database"@en ;
        skos:topConceptOf   ns10:file-type ;
        ns7:altLabel        []  ;
        ns7:prefLabel       []  .

<http://publications.europa.eu/resource/authority/file-type/DOC>
        a                   ns5:FileType , skos:Concept ;
        ns6:context         <http://publications.europa.eu/resource/authority/use-context/OJEEP> , <http://publications.europa.eu/resource/authority/use-context/ODP> , <http://publications.europa.eu/resource/authority/use-context/EUDOR> , <http://publications.europa.eu/resource/authority/use-context/IMMC> , <http://publications.europa.eu/resource/authority/use-context/DCAT_AP> , <http://publications.europa.eu/resource/authority/use-context/CELLAR> ;
        ns9:authority-code  "DOC" ;
        ns9:deprecated      "false" ;
        ns9:op-code         "DOC" ;
        ns9:op-mapped-code  []  ;
        ns9:op-mapped-code  []  ;
        ns9:op-mapped-code  []  ;
        ns9:op-mapped-code  []  ;
        ns9:op-mapped-code  []  ;
        ns9:op-mapped-code  []  ;
        ns9:start.use       "2012-09-01" ;
        ns5:isTextual       false ;
        ns5:order           290 ;
        ns5:startDate       "2012-09-01"^^<http://www.w3.org/2001/XMLSchema#date> ;
        ns5:status          <http://publications.europa.eu/resource/authority/concept-status/CURRENT> ;
        ns5:xlDefinition    []  ;
        ns5:xlNotation      []  ;
        ns5:xlNotation      []  ;
        ns5:xlNotation      []  ;
        ns5:xlNotation      []  ;
        ns5:xlNotation      []  ;
        ns10:op-code        "DOC" ;
        dc:identifier       "DOC" ;
        ns4:created         "2012-03-19"^^<http://www.w3.org/2001/XMLSchema#date> ;
        ns4:dateAccepted    "2012-11-27"^^<http://www.w3.org/2001/XMLSchema#date> ;
        ns4:dateSubmitted   "2012-09-27"^^<http://www.w3.org/2001/XMLSchema#date> ;
        owl:versionInfo     "20200624-0" ;
        skos:definition     "DOC is a proprietary binary Word document format used by Microsoft Word word processor."@en ;
        skos:inScheme       ns10:file-type ;
        skos:prefLabel      "Word DOC"@en ;
        skos:topConceptOf   ns10:file-type ;
        ns7:altLabel        []  ;
        ns7:prefLabel       []  .

<http://publications.europa.eu/resource/authority/file-type/SPARQLQRES>
        a                   ns5:FileType , skos:Concept ;
        ns6:context         <http://publications.europa.eu/resource/authority/use-context/CELLAR> , <http://publications.europa.eu/resource/authority/use-context/IMMC> , <http://publications.europa.eu/resource/authority/use-context/ODP> ;
        ns9:authority-code  "SPARQLQRES" ;
        ns9:deprecated      "false" ;
        ns9:op-code         "SPARQLQRES" ;
        ns9:op-mapped-code  []  ;
        ns9:op-mapped-code  []  ;
        ns9:op-mapped-code  []  ;
        ns9:op-mapped-code  []  ;
        ns9:op-mapped-code  []  ;
        ns9:op-mapped-code  []  ;
        ns9:op-mapped-code  []  ;
        ns9:start.use       "2012-09-01" ;
        ns5:isTextual       true ;
        ns5:order           80 ;
        ns5:startDate       "2012-09-01"^^<http://www.w3.org/2001/XMLSchema#date> ;
        ns5:status          <http://publications.europa.eu/resource/authority/concept-status/CURRENT> ;
        ns5:xlDefinition    []  ;
        ns5:xlNotation      []  ;
        ns5:xlNotation      []  ;
        ns5:xlNotation      []  ;
        ns5:xlNotation      []  ;
        ns5:xlNotation      []  ;
        ns5:xlNotation      []  ;
        ns10:op-code        "SPARQLQRES" ;
        dc:identifier       "SPARQLQRES" ;
        ns4:created         "2012-03-19"^^<http://www.w3.org/2001/XMLSchema#date> ;
        ns4:dateAccepted    "2012-11-27"^^<http://www.w3.org/2001/XMLSchema#date> ;
        ns4:dateSubmitted   "2012-09-27"^^<http://www.w3.org/2001/XMLSchema#date> ;
        owl:versionInfo     "20200624-0" ;
        skos:definition     "Results of a SPARQL query. SPARQL – SPARQL Protocol and RDF Query Language – is an RDF query language, that is, a semantic query language for databases, able to retrieve and manipulate data stored in Resource Description Framework (RDF) format."@en ;
        skos:inScheme       ns10:file-type ;
        skos:prefLabel      "SPARQL results"@en ;
        skos:topConceptOf   ns10:file-type ;
        ns7:altLabel        []  ;
        ns7:prefLabel       []  .

<http://publications.europa.eu/resource/authority/file-type/RDF_TRIG>
        a                    ns5:FileType , skos:Concept ;
        ns6:context          <http://publications.europa.eu/resource/authority/use-context/IMMC> , <http://publications.europa.eu/resource/authority/use-context/CELLAR> , <http://publications.europa.eu/resource/authority/use-context/ODP> ;
        ns9:authority-code   "RDF_TRIG" ;
        ns9:deprecated       "false" ;
        ns9:op-code          "RDF_TRIG" ;
        ns9:op-mapped-code   []  ;
        ns9:op-mapped-code   []  ;
        ns9:op-mapped-code   []  ;
        ns9:start.use        "2013-04-09" ;
        ns5:machineReadable  true ;
        ns5:nonPropExt       true ;
        ns5:startDate        "2013-04-09"^^<http://www.w3.org/2001/XMLSchema#date> ;
        ns5:status           <http://publications.europa.eu/resource/authority/concept-status/CURRENT> ;
        ns5:xlDefinition     []  ;
        ns5:xlNotation       []  ;
        ns5:xlNotation       []  ;
        ns10:op-code         "RDF_TRIG" ;
        dc:identifier        "RDF_TRIG" ;
        ns4:created          "2016-02-10"^^<http://www.w3.org/2001/XMLSchema#date> ;
        ns4:dateAccepted     "2016-03-02"^^<http://www.w3.org/2001/XMLSchema#date> ;
        ns4:dateSubmitted    "2016-02-16"^^<http://www.w3.org/2001/XMLSchema#date> ;
        owl:versionInfo      "20200624-0" ;
        skos:definition      "TriG allows an RDF dataset to be completely written in a compact and natural text form, with abbreviations for common usage patterns and datatypes. TriG is an extension of the Turtle format."@en ;
        skos:inScheme        ns10:file-type ;
        skos:prefLabel       "RDF TriG"@en ;
        skos:topConceptOf    ns10:file-type ;
        ns7:altLabel         []  ;
        ns7:prefLabel        []  .

<http://publications.europa.eu/resource/authority/file-type/JPEG>
        a                   ns5:FileType , skos:Concept ;
        ns6:context         <http://publications.europa.eu/resource/authority/use-context/EUDOR> , <http://publications.europa.eu/resource/authority/use-context/CELLAR> , <http://publications.europa.eu/resource/authority/use-context/IMMC> , <http://publications.europa.eu/resource/authority/use-context/DCAT_AP> , <http://publications.europa.eu/resource/authority/use-context/OJEEP> , <http://publications.europa.eu/resource/authority/use-context/ODP> , <http://publications.europa.eu/resource/authority/use-context/PUB> ;
        ns9:authority-code  "JPEG" ;
        ns9:deprecated      "false" ;
        ns9:op-code         "JPEG" ;
        ns9:op-mapped-code  []  ;
        ns9:op-mapped-code  []  ;
        ns9:op-mapped-code  []  ;
        ns9:op-mapped-code  []  ;
        ns9:op-mapped-code  []  ;
        ns9:op-mapped-code  []  ;
        ns9:op-mapped-code  []  ;
        ns9:start.use       "2012-09-01" ;
        ns5:isTextual       false ;
        ns5:order           170 ;
        ns5:startDate       "2012-09-01"^^<http://www.w3.org/2001/XMLSchema#date> ;
        ns5:status          <http://publications.europa.eu/resource/authority/concept-status/CURRENT> ;
        ns5:xlDefinition    []  ;
        ns5:xlNotation      []  ;
        ns5:xlNotation      []  ;
        ns5:xlNotation      []  ;
        ns5:xlNotation      []  ;
        ns5:xlNotation      []  ;
        ns5:xlNotation      []  ;
        ns10:op-code        "JPEG" ;
        dc:identifier       "JPEG" ;
        ns4:created         "2012-03-19"^^<http://www.w3.org/2001/XMLSchema#date> ;
        ns4:dateAccepted    "2012-11-27"^^<http://www.w3.org/2001/XMLSchema#date> ;
        ns4:dateSubmitted   "2012-09-27"^^<http://www.w3.org/2001/XMLSchema#date> ;
        owl:versionInfo     "20200624-0" ;
        skos:definition     "JPEG – Joint Photographic Experts Group – is a commonly used method of lossy compression for digital images, particularly for those images produced by digital photography. The degree of compression can be adjusted, allowing a selectable tradeoff between storage size and image quality."@en ;
        skos:inScheme       ns10:file-type ;
        skos:prefLabel      "JPEG"@en ;
        skos:topConceptOf   ns10:file-type ;
        ns7:altLabel        []  ;
        ns7:prefLabel       []  .

<http://publications.europa.eu/resource/authority/file-type/SKOS_XML>
        a                   skos:Concept , ns5:FileType ;
        ns6:context         <http://publications.europa.eu/resource/authority/use-context/IMMC> , <http://publications.europa.eu/resource/authority/use-context/ODP> , <http://publications.europa.eu/resource/authority/use-context/DCAT_AP> , <http://publications.europa.eu/resource/authority/use-context/CELLAR> ;
        ns9:authority-code  "SKOS_XML" ;
        ns9:deprecated      "false" ;
        ns9:op-code         "SKOS_XML" ;
        ns9:op-mapped-code  []  ;
        ns9:op-mapped-code  []  ;
        ns9:start.use       "2012-09-01" ;
        ns5:startDate       "2012-09-01"^^<http://www.w3.org/2001/XMLSchema#date> ;
        ns5:status          <http://publications.europa.eu/resource/authority/concept-status/CURRENT> ;
        ns5:xlDefinition    []  ;
        ns5:xlNotation      []  ;
        ns5:xlNotation      []  ;
        ns5:xlNotation      []  ;
        ns10:op-code        "SKOS_XML" ;
        dc:identifier       "SKOS_XML" ;
        ns4:created         "2012-03-19"^^<http://www.w3.org/2001/XMLSchema#date> ;
        ns4:dateAccepted    "2012-11-27"^^<http://www.w3.org/2001/XMLSchema#date> ;
        ns4:dateSubmitted   "2012-09-27"^^<http://www.w3.org/2001/XMLSchema#date> ;
        owl:versionInfo     "20200624-0" ;
        skos:definition     "SKOS – Simple Knowledge Organization System – is a W3C recommendation designed for representation of thesauri, classification schemes, taxonomies, subject-heading systems or any other type of structured controlled vocabulary. XML – Extensible Markup Language – is a markup language that defines a set of rules for encoding documents in a format that is both human-readable and machine-readable."@en ;
        skos:inScheme       ns10:file-type ;
        skos:prefLabel      "SKOS"@en ;
        skos:topConceptOf   ns10:file-type ;
        ns7:altLabel        []  ;
        ns7:prefLabel       []  .

<http://publications.europa.eu/resource/authority/file-type/ARJ>
        a                   ns5:FileType , skos:Concept ;
        ns6:context         <http://publications.europa.eu/resource/authority/use-context/DCAT_AP> , <http://publications.europa.eu/resource/authority/use-context/IMMC> ;
        ns9:authority-code  "ARJ" ;
        ns9:deprecated      "false" ;
        ns9:op-code         "ARJ" ;
        ns9:op-mapped-code  []  ;
        ns9:start.use       "1990-01-01" ;
        ns5:startDate       "1990-01-01"^^<http://www.w3.org/2001/XMLSchema#date> ;
        ns5:status          <http://publications.europa.eu/resource/authority/concept-status/CURRENT> ;
        ns5:xlDefinition    []  ;
        ns5:xlNotation      []  ;
        ns5:xlNotation      []  ;
        ns10:op-code        "ARJ" ;
        dc:identifier       "ARJ" ;
        ns4:created         "2020-05-15"^^<http://www.w3.org/2001/XMLSchema#date> ;
        ns4:dateAccepted    "2020-06-04"^^<http://www.w3.org/2001/XMLSchema#date> ;
        ns4:dateSubmitted   "2020-05-19"^^<http://www.w3.org/2001/XMLSchema#date> ;
        owl:versionInfo     "20200624-0" ;
        skos:definition     "Compressed archive file produced by ARJ software. ARJ (Archived by Robert Jung) is a software tool designed by Robert K. Jung for creating high-efficiency compressed file archives."@en ;
        skos:inScheme       ns10:file-type ;
        skos:prefLabel      "ARJ"@en ;
        skos:topConceptOf   ns10:file-type ;
        ns7:altLabel        []  ;
        ns7:prefLabel       []  .

<http://publications.europa.eu/resource/authority/file-type/OVF>
        a                   ns5:FileType , skos:Concept ;
        ns6:context         <http://publications.europa.eu/resource/authority/use-context/CELLAR> , <http://publications.europa.eu/resource/authority/use-context/IMMC> ;
        ns9:authority-code  "OVF" ;
        ns9:deprecated      "false" ;
        ns9:op-code         "OVF" ;
        ns9:op-mapped-code  []  ;
        ns9:start.use       "2007-09-10" ;
        ns5:startDate       "2007-09-10"^^<http://www.w3.org/2001/XMLSchema#date> ;
        ns5:status          <http://publications.europa.eu/resource/authority/concept-status/CURRENT> ;
        ns5:xlDefinition    []  ;
        ns5:xlNotation      []  ;
        ns5:xlNotation      []  ;
        ns10:op-code        "OVF" ;
        dc:identifier       "OVF" ;
        ns4:created         "2015-03-30"^^<http://www.w3.org/2001/XMLSchema#date> ;
        ns4:dateSubmitted   "2015-04-22"^^<http://www.w3.org/2001/XMLSchema#date> ;
        owl:versionInfo     "20200624-0" ;
        skos:definition     "OVF – Open Virtualization Format – is an open standard for packaging and distributing virtual appliances or more generally software to be run in virtual machines."@en ;
        skos:inScheme       ns10:file-type ;
        skos:prefLabel      "OVF"@en ;
        skos:topConceptOf   ns10:file-type ;
        ns7:altLabel        []  ;
        ns7:prefLabel       []  .

<http://publications.europa.eu/resource/authority/file-type/SDMX>
        a                   skos:Concept , ns5:FileType ;
        ns6:context         <http://publications.europa.eu/resource/authority/use-context/IMMC> , <http://publications.europa.eu/resource/authority/use-context/CELLAR> , <http://publications.europa.eu/resource/authority/use-context/ODP> ;
        ns9:authority-code  "SDMX" ;
        ns9:deprecated      "false" ;
        ns9:op-code         "SDMX" ;
        ns9:op-mapped-code  []  ;
        ns9:op-mapped-code  []  ;
        ns9:start.use       "2001-01-01" ;
        ns5:startDate       "2001-01-01"^^<http://www.w3.org/2001/XMLSchema#date> ;
        ns5:status          <http://publications.europa.eu/resource/authority/concept-status/CURRENT> ;
        ns5:xlDefinition    []  ;
        ns5:xlNotation      []  ;
        ns5:xlNotation      []  ;
        ns5:xlNotation      []  ;
        ns5:xlNotation      []  ;
        ns10:op-code        "SDMX" ;
        dc:identifier       "SDMX" ;
        ns4:created         "2015-04-07"^^<http://www.w3.org/2001/XMLSchema#date> ;
        ns4:dateSubmitted   "2015-04-22"^^<http://www.w3.org/2001/XMLSchema#date> ;
        owl:versionInfo     "20200624-0" ;
        skos:definition     "SDMX is an initiative to foster standards for the exchange of statistical information. The SDMX message formats have two basic expressions, SDMX-ML (using XML syntax) and SDMX-EDI (using EDIFACT syntax and based on the GESMES/TS statistical message)."@en ;
        skos:inScheme       ns10:file-type ;
        skos:prefLabel      "SDMX"@en ;
        skos:topConceptOf   ns10:file-type ;
        ns7:altLabel        []  ;
        ns7:prefLabel       []  .

<http://publications.europa.eu/resource/authority/file-type/DCR>
        a                   skos:Concept , ns5:FileType ;
        ns6:context         <http://publications.europa.eu/resource/authority/use-context/CELLAR> , <http://publications.europa.eu/resource/authority/use-context/ODP> , <http://publications.europa.eu/resource/authority/use-context/IMMC> ;
        ns9:authority-code  "DCR" ;
        ns9:deprecated      "false" ;
        ns9:op-code         "DCR" ;
        ns9:op-mapped-code  []  ;
        ns9:op-mapped-code  []  ;
        ns9:start.use       "1988-01-01" ;
        ns5:startDate       "1988-01-01"^^<http://www.w3.org/2001/XMLSchema#date> ;
        ns5:status          <http://publications.europa.eu/resource/authority/concept-status/CURRENT> ;
        ns5:xlDefinition    []  ;
        ns5:xlNotation      []  ;
        ns5:xlNotation      []  ;
        ns5:xlNotation      []  ;
        ns10:op-code        "DCR" ;
        dc:identifier       "DCR" ;
        ns4:created         "2015-04-21"^^<http://www.w3.org/2001/XMLSchema#date> ;
        ns4:dateSubmitted   "2015-04-22"^^<http://www.w3.org/2001/XMLSchema#date> ;
        owl:versionInfo     "20200624-0" ;
        skos:definition     "DCR is a file type for Adobe Shockwave Media files. DCR files are used to create games and other highly interactive content."@en ;
        skos:inScheme       ns10:file-type ;
        skos:prefLabel      "DCR File"@en ;
        skos:topConceptOf   ns10:file-type ;
        ns7:altLabel        []  ;
        ns7:prefLabel       []  .

<http://publications.europa.eu/resource/authority/file-type/ARC_GZ>
        a                   skos:Concept , ns5:FileType ;
        ns6:context         <http://publications.europa.eu/resource/authority/use-context/IMMC> , <http://publications.europa.eu/resource/authority/use-context/ODP> , <http://publications.europa.eu/resource/authority/use-context/CELLAR> ;
        ns9:authority-code  "ARC_GZ" ;
        ns9:deprecated      "false" ;
        ns9:op-code         "ARC_GZ" ;
        ns9:op-mapped-code  []  ;
        ns9:start.use       "2012-09-01" ;
        ns5:startDate       "2012-09-01"^^<http://www.w3.org/2001/XMLSchema#date> ;
        ns5:status          <http://publications.europa.eu/resource/authority/concept-status/CURRENT> ;
        ns5:xlDefinition    []  ;
        ns5:xlNotation      []  ;
        ns5:xlNotation      []  ;
        ns10:op-code        "ARC_GZ" ;
        dc:identifier       "ARC_GZ" ;
        ns4:created         "2017-05-19"^^<http://www.w3.org/2001/XMLSchema#date> ;
        ns4:dateAccepted    "2017-06-08"^^<http://www.w3.org/2001/XMLSchema#date> ;
        ns4:dateSubmitted   "2017-05-22"^^<http://www.w3.org/2001/XMLSchema#date> ;
        owl:versionInfo     "20200624-0" ;
        skos:definition     "ARC is the archive file format of Internet Archive. ARC files are large aggregate files. ARC GZ is ARC compressed by GZIP."@en ;
        skos:inScheme       ns10:file-type ;
        skos:prefLabel      "ARC GZ"@en ;
        skos:topConceptOf   ns10:file-type ;
        ns7:altLabel        []  ;
        ns7:prefLabel       []  .
